<?xml version="1.0"?>
<rdf:RDF xmlns="http://performedmusicontology.org/ontology/"
     xml:base="http://performedmusicontology.org/ontology/"
     xmlns:rdakit="http://metadataregistry.org/uri/profile/rdakit/"
     xmlns:rdf="http://www.w3.org/1999/02/22-rdf-syntax-ns#"
     xmlns:terms="http://purl.org/dc/terms/"
     xmlns:owl="http://www.w3.org/2002/07/owl#"
     xmlns:xml="http://www.w3.org/XML/1998/namespace"
     xmlns:regap="http://metadataregistry.org/uri/profile/regap/"
     xmlns:xsd="http://www.w3.org/2001/XMLSchema#"
     xmlns:skos="http://www.w3.org/2004/02/skos/core#"
     xmlns:rdfs="http://www.w3.org/2000/01/rdf-schema#"
     xmlns:vann="http://purl.org/vocab/vann/"
     xmlns:dc="http://purl.org/dc/elements/1.1/">
    <owl:Ontology rdf:about="http://performedmusicontology.org/ontology/">
        <owl:versionIRI rdf:resource="http://performedmusicontology.org/ontology/"/>
        <owl:imports rdf:resource="http://id.loc.gov/ontologies/bibframe/"/>
    </owl:Ontology>
    


    <!-- 
    ///////////////////////////////////////////////////////////////////////////////////////
    //
    // Annotation properties
    //
    ///////////////////////////////////////////////////////////////////////////////////////
     -->

    


    <!-- http://metadataregistry.org/uri/profile/rdakit/toolkitDefinition -->

    <owl:AnnotationProperty rdf:about="http://metadataregistry.org/uri/profile/rdakit/toolkitDefinition"/>
    


    <!-- http://metadataregistry.org/uri/profile/rdakit/toolkitLabel -->

    <owl:AnnotationProperty rdf:about="http://metadataregistry.org/uri/profile/rdakit/toolkitLabel"/>
    


    <!-- http://metadataregistry.org/uri/profile/regap/identifier -->

    <owl:AnnotationProperty rdf:about="http://metadataregistry.org/uri/profile/regap/identifier"/>
    


    <!-- http://metadataregistry.org/uri/profile/regap/status -->

    <owl:AnnotationProperty rdf:about="http://metadataregistry.org/uri/profile/regap/status"/>
    


    <!-- http://purl.org/dc/elements/1.1/title -->

    <owl:AnnotationProperty rdf:about="http://purl.org/dc/elements/1.1/title"/>
    


    <!-- http://purl.org/dc/terms/description -->

    <owl:AnnotationProperty rdf:about="http://purl.org/dc/terms/description"/>
    


    <!-- http://www.w3.org/2004/02/skos/core#altLabel -->

    <owl:AnnotationProperty rdf:about="http://www.w3.org/2004/02/skos/core#altLabel"/>
    


    <!-- http://www.w3.org/2004/02/skos/core#broader -->

    <owl:AnnotationProperty rdf:about="http://www.w3.org/2004/02/skos/core#broader"/>
    


    <!-- http://www.w3.org/2004/02/skos/core#definition -->

    <owl:AnnotationProperty rdf:about="http://www.w3.org/2004/02/skos/core#definition"/>
    


    <!-- http://www.w3.org/2004/02/skos/core#narrower -->

    <owl:AnnotationProperty rdf:about="http://www.w3.org/2004/02/skos/core#narrower"/>
    


    <!-- http://www.w3.org/2004/02/skos/core#prefLabel -->

    <owl:AnnotationProperty rdf:about="http://www.w3.org/2004/02/skos/core#prefLabel"/>
    


    <!-- http://www.w3.org/2004/02/skos/core#scopeNote -->

    <owl:AnnotationProperty rdf:about="http://www.w3.org/2004/02/skos/core#scopeNote"/>
    


    <!-- 
    ///////////////////////////////////////////////////////////////////////////////////////
    //
    // Object Properties
    //
    ///////////////////////////////////////////////////////////////////////////////////////
     -->

    


    <!-- http://id.loc.gov/ontologies/bibframe/eventContent -->

    <owl:ObjectProperty rdf:about="http://id.loc.gov/ontologies/bibframe/eventContent"/>
    


    <!-- http://id.loc.gov/ontologies/bibframe/eventContentOf -->

    <owl:ObjectProperty rdf:about="http://id.loc.gov/ontologies/bibframe/eventContentOf"/>
    


    <!-- http://id.loc.gov/ontologies/bibframe/relatedTo -->

    <owl:ObjectProperty rdf:about="http://id.loc.gov/ontologies/bibframe/relatedTo"/>
    


    <!-- http://performedmusicontology.org/ontology/alternateOf -->

    <owl:ObjectProperty rdf:about="http://performedmusicontology.org/ontology/alternateOf">
        <skos:definition>Declared medium part that is an alternate for another declared medium part</skos:definition>
    </owl:ObjectProperty>
    


    <!-- http://performedmusicontology.org/ontology/associatedWith -->

    <owl:ObjectProperty rdf:about="http://performedmusicontology.org/ontology/associatedWith">
        <rdfs:subPropertyOf rdf:resource="http://id.loc.gov/ontologies/bibframe/relatedTo"/>
        <rdf:type rdf:resource="http://www.w3.org/2002/07/owl#InverseFunctionalProperty"/>
        <rdfs:range rdf:resource="http://id.loc.gov/ontologies/bibframe/Event"/>
        <skos:definition>Event a work, instance, or item is created for, e.g., a motet created for the inauguration of Pope Clement VI.</skos:definition>
    </owl:ObjectProperty>
    


    <!-- http://performedmusicontology.org/ontology/createdFor -->

    <owl:ObjectProperty rdf:about="http://performedmusicontology.org/ontology/createdFor">
        <rdfs:subPropertyOf rdf:resource="http://id.loc.gov/ontologies/bibframe/relatedTo"/>
        <rdfs:domain rdf:resource="http://id.loc.gov/ontologies/bibframe/Work"/>
        <rdfs:range rdf:resource="http://id.loc.gov/ontologies/bibframe/Event"/>
        <skos:definition>Event a work is created for, e.g., a motet celebrating the inauguration of a pope.</skos:definition>
    </owl:ObjectProperty>
    


    <!-- http://performedmusicontology.org/ontology/eventNameOf -->

    <owl:ObjectProperty rdf:about="http://performedmusicontology.org/ontology/eventNameOf">
        <owl:inverseOf rdf:resource="http://performedmusicontology.org/ontology/hasEventName"/>
        <rdfs:range rdf:resource="http://id.loc.gov/ontologies/bibframe/Event"/>
    </owl:ObjectProperty>
    


    <!-- http://performedmusicontology.org/ontology/hasDoublingMediumofPerformance -->

    <owl:ObjectProperty rdf:about="http://performedmusicontology.org/ontology/hasDoublingMediumofPerformance">
        <skos:definition>2 (or more) mediums of performance intended to be performed alternately by a single performer</skos:definition>
    </owl:ObjectProperty>
    


    <!-- http://performedmusicontology.org/ontology/hasDramaticRole -->

    <owl:ObjectProperty rdf:about="http://performedmusicontology.org/ontology/hasDramaticRole"/>
    


    <!-- http://performedmusicontology.org/ontology/hasEventName -->

    <owl:ObjectProperty rdf:about="http://performedmusicontology.org/ontology/hasEventName">
        <rdfs:domain rdf:resource="http://id.loc.gov/ontologies/bibframe/Event"/>
    </owl:ObjectProperty>
    


    <!-- http://performedmusicontology.org/ontology/hasInspiration -->

    <owl:ObjectProperty rdf:about="http://performedmusicontology.org/ontology/hasInspiration">
        <rdfs:subPropertyOf rdf:resource="http://id.loc.gov/ontologies/bibframe/relatedTo"/>
        <owl:inverseOf rdf:resource="http://performedmusicontology.org/ontology/inspirationFor"/>
    </owl:ObjectProperty>
    


    <!-- http://performedmusicontology.org/ontology/hasMedium -->

    <owl:ObjectProperty rdf:about="http://performedmusicontology.org/ontology/hasMedium">
        <skos:definition>The declared or performed medium as a whole.</skos:definition>
    </owl:ObjectProperty>
    


    <!-- http://performedmusicontology.org/ontology/hasMediumOfPerformance -->

    <owl:ObjectProperty rdf:about="http://performedmusicontology.org/ontology/hasMediumOfPerformance">
        <skos:definition>Specific medium of performance, e.g., bass guitar.</skos:definition>
    </owl:ObjectProperty>
    


    <!-- http://performedmusicontology.org/ontology/hasMediumPart -->

    <owl:ObjectProperty rdf:about="http://performedmusicontology.org/ontology/hasMediumPart">
        <rdfs:comment>Use with: pmo:DeclaredMedium, pmo:PerformedMedium, pmo:AlternateMedium
bf:Contribution</rdfs:comment>
        <skos:definition>Specific element within an overall declared or performed medium</skos:definition>
    </owl:ObjectProperty>
    


    <!-- http://performedmusicontology.org/ontology/hasMediumPartType -->

    <owl:ObjectProperty rdf:about="http://performedmusicontology.org/ontology/hasMediumPartType">
        <skos:definition>Specific role or type of a medium part, e.g., solo, ad lib, optional, offstage.</skos:definition>
    </owl:ObjectProperty>
    


    <!-- http://performedmusicontology.org/ontology/hasMusicPart -->

    <owl:ObjectProperty rdf:about="http://performedmusicontology.org/ontology/hasMusicPart"/>
    


    <!-- http://performedmusicontology.org/ontology/hasPerformance -->

    <owl:ObjectProperty rdf:about="http://performedmusicontology.org/ontology/hasPerformance">
        <rdfs:subPropertyOf rdf:resource="http://id.loc.gov/ontologies/bibframe/eventContentOf"/>
        <owl:inverseOf rdf:resource="http://performedmusicontology.org/ontology/performanceOf"/>
        <rdfs:domain rdf:resource="http://id.loc.gov/ontologies/bibframe/Work"/>
        <rdfs:range rdf:resource="http://performedmusicontology.org/ontology/Performance"/>
    </owl:ObjectProperty>
    


    <!-- http://performedmusicontology.org/ontology/hasProxyWork -->

    <owl:ObjectProperty rdf:about="http://performedmusicontology.org/ontology/hasProxyWork">
        <rdfs:comment>Work that is a duplicate of another work, except that it is included as part of an aggregation/compilation or a work component in multiples works. The proxy work permits numbering within the aggregate or work.</rdfs:comment>
    </owl:ObjectProperty>
    


    <!-- http://performedmusicontology.org/ontology/hasRecording -->

    <owl:ObjectProperty rdf:about="http://performedmusicontology.org/ontology/hasRecording">
        <rdfs:subPropertyOf rdf:resource="http://id.loc.gov/ontologies/bibframe/eventContent"/>
        <owl:inverseOf rdf:resource="http://performedmusicontology.org/ontology/recordingOf"/>
        <rdfs:domain rdf:resource="http://id.loc.gov/ontologies/bibframe/Event"/>
        <rdfs:range rdf:resource="http://id.loc.gov/ontologies/bibframe/Work"/>
        <skos:definition>Audio or video recording of an event.</skos:definition>
    </owl:ObjectProperty>
    


    <!-- http://performedmusicontology.org/ontology/inspirationFor -->

    <owl:ObjectProperty rdf:about="http://performedmusicontology.org/ontology/inspirationFor">
        <rdfs:subPropertyOf rdf:resource="http://id.loc.gov/ontologies/bibframe/relatedTo"/>
    </owl:ObjectProperty>
    


    <!-- http://performedmusicontology.org/ontology/performanceOf -->

    <owl:ObjectProperty rdf:about="http://performedmusicontology.org/ontology/performanceOf">
        <rdfs:subPropertyOf rdf:resource="http://id.loc.gov/ontologies/bibframe/eventContent"/>
        <rdfs:domain rdf:resource="http://id.loc.gov/ontologies/bibframe/Event"/>
        <rdfs:range rdf:resource="http://performedmusicontology.org/ontology/Performance"/>
    </owl:ObjectProperty>
    


    <!-- http://performedmusicontology.org/ontology/playsDramaticRole -->

    <owl:ObjectProperty rdf:about="http://performedmusicontology.org/ontology/playsDramaticRole"/>
    


    <!-- http://performedmusicontology.org/ontology/recordingOf -->

    <owl:ObjectProperty rdf:about="http://performedmusicontology.org/ontology/recordingOf">
        <rdfs:subPropertyOf rdf:resource="http://id.loc.gov/ontologies/bibframe/eventContentOf"/>
        <rdfs:domain rdf:resource="http://id.loc.gov/ontologies/bibframe/Work"/>
        <rdfs:range rdf:resource="http://id.loc.gov/ontologies/bibframe/Event"/>
    </owl:ObjectProperty>
    


    <!-- http://www.w3.org/2004/02/skos/core#hasTopConcept -->

    <owl:ObjectProperty rdf:about="http://www.w3.org/2004/02/skos/core#hasTopConcept"/>
    


    <!-- http://www.w3.org/2004/02/skos/core#inScheme -->

    <owl:ObjectProperty rdf:about="http://www.w3.org/2004/02/skos/core#inScheme"/>
    


    <!-- http://www.w3.org/2004/02/skos/core#related -->

    <owl:ObjectProperty rdf:about="http://www.w3.org/2004/02/skos/core#related"/>
    


    <!-- http://www.w3.org/2004/02/skos/core#topConceptOf -->

    <owl:ObjectProperty rdf:about="http://www.w3.org/2004/02/skos/core#topConceptOf"/>
    


    <!-- 
    ///////////////////////////////////////////////////////////////////////////////////////
    //
    // Data properties
    //
    ///////////////////////////////////////////////////////////////////////////////////////
     -->

    


    <!-- http://id.loc.gov/ontologies/bibframe/date -->

    <owl:DatatypeProperty rdf:about="http://id.loc.gov/ontologies/bibframe/date"/>
    


    <!-- http://performedmusicontology.org/ontology/hasDistinctMusicPartCount -->

    <owl:DatatypeProperty rdf:about="http://performedmusicontology.org/ontology/hasDistinctMusicPartCount"/>
    


    <!-- http://performedmusicontology.org/ontology/hasMusicPart -->

    <owl:DatatypeProperty rdf:about="http://performedmusicontology.org/ontology/hasMusicPart"/>
    


    <!-- http://performedmusicontology.org/ontology/hasOrder -->

    <owl:DatatypeProperty rdf:about="http://performedmusicontology.org/ontology/hasOrder"/>
    


    <!-- http://performedmusicontology.org/ontology/hasRequiredPerformersCount -->

    <owl:DatatypeProperty rdf:about="http://performedmusicontology.org/ontology/hasRequiredPerformersCount"/>
    


    <!-- http://performedmusicontology.org/ontology/phonogramCopyrightDate -->

    <owl:DatatypeProperty rdf:about="http://performedmusicontology.org/ontology/phonogramCopyrightDate">
        <rdfs:subPropertyOf rdf:resource="http://id.loc.gov/ontologies/bibframe/date"/>
    </owl:DatatypeProperty>
    


    <!-- 
    ///////////////////////////////////////////////////////////////////////////////////////
    //
    // Classes
    //
    ///////////////////////////////////////////////////////////////////////////////////////
     -->

    


    <!-- http://erlangen-crm.org/efrbroo/F31_Performance -->

    <owl:Class rdf:about="http://erlangen-crm.org/efrbroo/F31_Performance"/>
    


    <!-- http://id.loc.gov/ontologies/bibframe/Agent -->

    <owl:Class rdf:about="http://id.loc.gov/ontologies/bibframe/Agent"/>
    


    <!-- http://id.loc.gov/ontologies/bibframe/Carrier -->

    <owl:Class rdf:about="http://id.loc.gov/ontologies/bibframe/Carrier"/>
    


    <!-- http://id.loc.gov/ontologies/bibframe/Contribution -->

    <owl:Class rdf:about="http://id.loc.gov/ontologies/bibframe/Contribution"/>
    


    <!-- http://id.loc.gov/ontologies/bibframe/EncodingFormat -->

    <owl:Class rdf:about="http://id.loc.gov/ontologies/bibframe/EncodingFormat"/>
    


    <!-- http://id.loc.gov/ontologies/bibframe/Event -->

    <owl:Class rdf:about="http://id.loc.gov/ontologies/bibframe/Event"/>
    


    <!-- http://id.loc.gov/ontologies/bibframe/Identifier -->

    <owl:Class rdf:about="http://id.loc.gov/ontologies/bibframe/Identifier"/>
    


    <!-- http://id.loc.gov/ontologies/bibframe/Person -->

    <owl:Class rdf:about="http://id.loc.gov/ontologies/bibframe/Person"/>
    


    <!-- http://id.loc.gov/ontologies/bibframe/PlayingSpeed -->

    <owl:Class rdf:about="http://id.loc.gov/ontologies/bibframe/PlayingSpeed"/>
    


    <!-- http://id.loc.gov/ontologies/bibframe/Role -->

    <owl:Class rdf:about="http://id.loc.gov/ontologies/bibframe/Role"/>
    


    <!-- http://id.loc.gov/ontologies/bibframe/SoundCharacteristic -->

    <owl:Class rdf:about="http://id.loc.gov/ontologies/bibframe/SoundCharacteristic"/>
    


    <!-- http://id.loc.gov/ontologies/bibframe/TapeConfig -->

    <owl:Class rdf:about="http://id.loc.gov/ontologies/bibframe/TapeConfig"/>
    


    <!-- http://id.loc.gov/ontologies/bibframe/Work -->

    <owl:Class rdf:about="http://id.loc.gov/ontologies/bibframe/Work"/>
    


    <!-- http://performedmusicontology.org/ontology/Audition -->

    <owl:Class rdf:about="http://performedmusicontology.org/ontology/Audition">
        <rdfs:subClassOf rdf:resource="http://id.loc.gov/ontologies/bibframe/Event"/>
        <skos:definition>Event in which a performer or actor is applying for a position in an ensemble, cast, film, etc.</skos:definition>
    </owl:Class>
    


    <!-- http://performedmusicontology.org/ontology/BenefitConcert -->

    <owl:Class rdf:about="http://performedmusicontology.org/ontology/BenefitConcert">
        <rdfs:subClassOf rdf:resource="http://performedmusicontology.org/ontology/Concert"/>
        <skos:definition>Concert held for charitable purposes, i.e., to raise funds or awareness</skos:definition>
    </owl:Class>
    


    <!-- http://performedmusicontology.org/ontology/Ceremony -->

    <owl:Class rdf:about="http://performedmusicontology.org/ontology/Ceremony">
        <rdfs:subClassOf rdf:resource="http://id.loc.gov/ontologies/bibframe/Event"/>
        <skos:definition>Ritual event, performed on special occasions (e.g., death, baptism, wedding, graduation, equinox, coronation, victory)</skos:definition>
    </owl:Class>
    


    <!-- http://performedmusicontology.org/ontology/CommandPerformance -->

    <owl:Class rdf:about="http://performedmusicontology.org/ontology/CommandPerformance">
        <rdfs:subClassOf rdf:resource="http://performedmusicontology.org/ontology/Concert"/>
        <skos:definition>Performance done at the request of a monarch or other head of state.</skos:definition>
    </owl:Class>
    


    <!-- http://performedmusicontology.org/ontology/Concert -->

    <owl:Class rdf:about="http://performedmusicontology.org/ontology/Concert">
        <rdfs:subClassOf rdf:resource="http://id.loc.gov/ontologies/bibframe/Event"/>
        <skos:definition>Live musical performance of one or more works in front of an audience</skos:definition>
    </owl:Class>
    


    <!-- http://performedmusicontology.org/ontology/ConcertSeries -->

    <owl:Class rdf:about="http://performedmusicontology.org/ontology/ConcertSeries">
        <rdfs:subClassOf rdf:resource="http://id.loc.gov/ontologies/bibframe/Event"/>
        <skos:definition>Group of concerts in the same geographic area by a single performer or brought together by a common theme, usually available for sale as a package. e.g., an orchestra concert season, a series featuring chamber ensembles.</skos:definition>
    </owl:Class>
    


    <!-- http://performedmusicontology.org/ontology/ConcertTour -->

    <owl:Class rdf:about="http://performedmusicontology.org/ontology/ConcertTour">
        <rdfs:subClassOf rdf:resource="http://id.loc.gov/ontologies/bibframe/Event"/>
        <skos:definition>Series of concerts by a performer or group of performers in different cities, countries, or locations.</skos:definition>
    </owl:Class>
    


    <!-- http://performedmusicontology.org/ontology/DeclaredMedium -->

    <owl:Class rdf:about="http://performedmusicontology.org/ontology/DeclaredMedium">
        <skos:definition>Intended overall medium of performance of a musical work, as declared by the composer, a reference source, or an instance of the work.</skos:definition>
    </owl:Class>
    


    <!-- http://performedmusicontology.org/ontology/DiscCutting -->

    <owl:Class rdf:about="http://performedmusicontology.org/ontology/DiscCutting">
        <rdfs:subClassOf rdf:resource="http://id.loc.gov/ontologies/bibframe/SoundCharacteristic"/>
        <skos:definition>Recording process in which a stylus cuts a vertical or lateral groove into an audio disc.</skos:definition>
    </owl:Class>
    


    <!-- http://performedmusicontology.org/ontology/DramaticRole -->

    <owl:Class rdf:about="http://performedmusicontology.org/ontology/DramaticRole"/>
    


    <!-- http://performedmusicontology.org/ontology/EventName -->

    <owl:Class rdf:about="http://performedmusicontology.org/ontology/EventName">
        <skos:definition>Name given to an event.</skos:definition>
    </owl:Class>
    


    <!-- http://performedmusicontology.org/ontology/FirstPerformance -->

    <owl:Class rdf:about="http://performedmusicontology.org/ontology/FirstPerformance">
        <rdfs:subClassOf rdf:resource="http://performedmusicontology.org/ontology/Performance"/>
        <skos:definition>The world premiere performance of a work.</skos:definition>
    </owl:Class>
    


    <!-- http://performedmusicontology.org/ontology/IndividualInstrument -->

    <owl:Class rdf:about="http://performedmusicontology.org/ontology/IndividualInstrument">
        <rdfs:subClassOf rdf:resource="http://performedmusicontology.org/ontology/MusicalInstrument"/>
        <skos:definition>Single musical instrument, e.g., bassoon, bass guitar, synthesizer or group of instruments, e.g., percussion, intended to be played by a single performer.</skos:definition>
    </owl:Class>
    


    <!-- http://performedmusicontology.org/ontology/IndividualVoice -->

    <owl:Class rdf:about="http://performedmusicontology.org/ontology/IndividualVoice">
        <rdfs:subClassOf rdf:resource="http://performedmusicontology.org/ontology/Voice"/>
        <rdfs:comment>Single voice, i.e., soprano, male voice, alto.</rdfs:comment>
    </owl:Class>
    


    <!-- http://performedmusicontology.org/ontology/InstrumentEnsemble -->

    <owl:Class rdf:about="http://performedmusicontology.org/ontology/InstrumentEnsemble">
        <rdfs:subClassOf rdf:resource="http://performedmusicontology.org/ontology/MusicalInstrument"/>
        <skos:definition>Group of like or unlike musical instruments intended to be played by multiple performers.</skos:definition>
    </owl:Class>
    


    <!-- http://performedmusicontology.org/ontology/LivePerformance -->

    <owl:Class rdf:about="http://performedmusicontology.org/ontology/LivePerformance">
        <rdfs:subClassOf rdf:resource="http://performedmusicontology.org/ontology/Performance"/>
        <skos:definition>Performance that is recorded at a concert.</skos:definition>
    </owl:Class>
    


    <!-- http://performedmusicontology.org/ontology/MasterClass -->

    <owl:Class rdf:about="http://performedmusicontology.org/ontology/MasterClass">
        <rdfs:subClassOf rdf:resource="http://id.loc.gov/ontologies/bibframe/Event"/>
        <skos:definition>Event in which a recognized performer critiques the performances of one or more other performers.</skos:definition>
    </owl:Class>
    


    <!-- http://performedmusicontology.org/ontology/MediumOfPerformance -->

    <owl:Class rdf:about="http://performedmusicontology.org/ontology/MediumOfPerformance">
        <skos:definition>Instruments, voices, ensembles, choruses, and other participants (actors, dancers, etc.) required or used for an event or work, including electronics, computers, installations, etc.</skos:definition>
    </owl:Class>
    


    <!-- http://performedmusicontology.org/ontology/MediumPart -->

    <owl:Class rdf:about="http://performedmusicontology.org/ontology/MediumPart">
        <skos:definition>Medium of performance, type, etc., of a specific part of the declared or performed medium.</skos:definition>
    </owl:Class>
    


    <!-- http://performedmusicontology.org/ontology/MediumPartType -->

    <owl:Class rdf:about="http://performedmusicontology.org/ontology/MediumPartType">
        <rdfs:label>Medium type</rdfs:label>
        <skos:definition>The type of pmo:PerformedMediumPart, e.g., solo, ad lib, optional</skos:definition>
    </owl:Class>
    


    <!-- http://performedmusicontology.org/ontology/MusicalInstrument -->

    <owl:Class rdf:about="http://performedmusicontology.org/ontology/MusicalInstrument">
        <rdfs:subClassOf rdf:resource="http://performedmusicontology.org/ontology/MediumOfPerformance"/>
        <skos:definition>Musical instrument(s) or object(s) used as a musical instrument (e.g., drinking glasses, leaves, typewriters).</skos:definition>
    </owl:Class>
    


    <!-- http://performedmusicontology.org/ontology/OpenMicPerformance -->

    <owl:Class rdf:about="http://performedmusicontology.org/ontology/OpenMicPerformance">
        <rdfs:subClassOf rdf:resource="http://performedmusicontology.org/ontology/Performance"/>
        <skos:definition>Live performance at a coffee house, night club, or other venue by amateur performers.</skos:definition>
    </owl:Class>
    


    <!-- http://performedmusicontology.org/ontology/Performance -->

    <owl:Class rdf:about="http://performedmusicontology.org/ontology/Performance">
        <rdfs:subClassOf rdf:resource="http://erlangen-crm.org/efrbroo/F31_Performance"/>
        <rdfs:subClassOf rdf:resource="http://id.loc.gov/ontologies/bibframe/Event"/>
        <skos:definition>Event in which a performer or group of performers present a work to an audience or in a recording studio.</skos:definition>
    </owl:Class>
    


    <!-- http://performedmusicontology.org/ontology/PerformedMedium -->

    <owl:Class rdf:about="http://performedmusicontology.org/ontology/PerformedMedium">
        <skos:definition>The overall medium of performance used in the performance of a musical work. This may or may not be the same as the declared medium of performance.</skos:definition>
    </owl:Class>
    


    <!-- http://performedmusicontology.org/ontology/ProxyWork -->

    <owl:Class rdf:about="http://performedmusicontology.org/ontology/ProxyWork">
        <rdfs:subClassOf rdf:resource="http://id.loc.gov/ontologies/bibframe/Work"/>
        <skos:definition>A work that is aggregated into a compilation or other type of aggregating work. Ordering of the work within the aggregating work is put here.</skos:definition>
    </owl:Class>
    


    <!-- http://performedmusicontology.org/ontology/RecordingSession -->

    <owl:Class rdf:about="http://performedmusicontology.org/ontology/RecordingSession">
        <rdfs:subClassOf rdf:resource="http://id.loc.gov/ontologies/bibframe/Event"/>
        <skos:definition>Event in which one or more performances are recorded with the aim of producing a recording for issue.</skos:definition>
    </owl:Class>
    


    <!-- http://performedmusicontology.org/ontology/Rehearsal -->

    <owl:Class rdf:about="http://performedmusicontology.org/ontology/Rehearsal">
        <rdfs:subClassOf rdf:resource="http://id.loc.gov/ontologies/bibframe/Event"/>
        <skos:definition>Event in which a performer or group of performers prepare for a performance in a concert.</skos:definition>
    </owl:Class>
    


    <!-- http://performedmusicontology.org/ontology/Tempo -->

    <owl:Class rdf:about="http://performedmusicontology.org/ontology/Tempo">
        <rdfs:isDefinedBy>The speed or pace of a music work, whether declared (in a score) or performed.</rdfs:isDefinedBy>
    </owl:Class>
    


    <!-- http://performedmusicontology.org/ontology/VideogamePlatformIdentifier -->

    <owl:Class rdf:about="http://performedmusicontology.org/ontology/VideogamePlatformIdentifier">
        <rdfs:subClassOf rdf:resource="http://id.loc.gov/ontologies/bibframe/Identifier"/>
        <skos:definition>Identifier assigned to a video game platform, e.g., CUSA 54321 (a PlayStation 4 number).</skos:definition>
    </owl:Class>
    


    <!-- http://performedmusicontology.org/ontology/Voice -->

    <owl:Class rdf:about="http://performedmusicontology.org/ontology/Voice">
        <rdfs:subClassOf rdf:resource="http://performedmusicontology.org/ontology/MediumOfPerformance"/>
        <skos:definition>Human voice as a medium of performance, whether singing, speaking, or making sounds</skos:definition>
    </owl:Class>
    


    <!-- http://performedmusicontology.org/ontology/VoiceEnsemble -->

    <owl:Class rdf:about="http://performedmusicontology.org/ontology/VoiceEnsemble">
        <rdfs:subClassOf rdf:resource="http://performedmusicontology.org/ontology/Voice"/>
        <rdfs:comment>Group of like or unlike voices, e.g., children’s chorus.</rdfs:comment>
    </owl:Class>
    


    <!-- http://performedmusicontology.org/ontology/WorkComponent -->

    <owl:Class rdf:about="http://performedmusicontology.org/ontology/WorkComponent">
        <rdfs:subClassOf rdf:resource="http://id.loc.gov/ontologies/bibframe/Work"/>
        <rdfs:isDefinedBy>A work that is an integral part of another work, even when separated from it, e.g., a movement of a symphony, a chapter of a novel.</rdfs:isDefinedBy>
    </owl:Class>
    


    <!-- http://www.w3.org/2004/02/skos/core#Concept -->

    <owl:Class rdf:about="http://www.w3.org/2004/02/skos/core#Concept"/>
    


    <!-- http://www.w3.org/2004/02/skos/core#ConceptScheme -->

    <owl:Class rdf:about="http://www.w3.org/2004/02/skos/core#ConceptScheme"/>
    


    <!-- 
    ///////////////////////////////////////////////////////////////////////////////////////
    //
    // Individuals
    //
    ///////////////////////////////////////////////////////////////////////////////////////
     -->

    


    <!-- http://performedmusicontology.org/FPM12 -->

    <owl:NamedIndividual rdf:about="http://performedmusicontology.org/FPM12">
        <rdf:type rdf:resource="http://id.loc.gov/ontologies/bibframe/PlayingSpeed"/>
        <rdfs:comment>Traditional way of describing the speed of audio cylinders.</rdfs:comment>
        <rdfs:label rdf:datatype="http://www.w3.org/2001/XMLSchema#integer">120</rdfs:label>
        <skos:definition>Playing speed of 12 feet per minute x 10.</skos:definition>
    </owl:NamedIndividual>
    


    <!-- http://performedmusicontology.org/Laserdisc -->

    <owl:NamedIndividual rdf:about="http://performedmusicontology.org/Laserdisc">
        <rdf:type rdf:resource="http://id.loc.gov/ontologies/bibframe/Carrier"/>
        <rdfs:label>Laser disc</rdfs:label>
        <skos:broader rdf:resource="http://rdaregistry.info/termList/RDACarrierType/1060"/>
        <skos:definition>Optical video disc, 30 cm (12 in.) in diameter. It was the first commercial optical disc storage medium.</skos:definition>
    </owl:NamedIndividual>
    


    <!-- http://performedmusicontology.org/adLib -->

    <owl:NamedIndividual rdf:about="http://performedmusicontology.org/adLib">
        <rdf:type rdf:resource="http://performedmusicontology.org/ontology/MediumPartType"/>
        <rdfs:comment>For mediums of performance marked &quot;ad lib&quot; or &quot;ad libitum&quot; in a score or otherwise.</rdfs:comment>
        <rdfs:label>ad lib</rdfs:label>
        <skos:altLabel>ad libitum</skos:altLabel>
    </owl:NamedIndividual>
    


    <!-- http://performedmusicontology.org/offstage -->

    <owl:NamedIndividual rdf:about="http://performedmusicontology.org/offstage">
        <rdf:type rdf:resource="http://performedmusicontology.org/ontology/MediumPartType"/>
        <rdfs:label>offstage</rdfs:label>
        <skos:definition>A declared or performed medium that is to be performed or is performed offstage, i.e., out of sight of the audience.</skos:definition>
    </owl:NamedIndividual>
    


    <!-- http://performedmusicontology.org/optional -->

    <owl:NamedIndividual rdf:about="http://performedmusicontology.org/optional">
        <rdf:type rdf:resource="http://performedmusicontology.org/ontology/MediumPartType"/>
        <rdfs:label>optional</rdfs:label>
        <skos:definition>For mediums of performance marked &quot;optional&quot; in a score or otherwise.</skos:definition>
    </owl:NamedIndividual>
    


    <!-- http://performedmusicontology.org/solo -->

    <owl:NamedIndividual rdf:about="http://performedmusicontology.org/solo">
        <rdf:type rdf:resource="http://performedmusicontology.org/ontology/MediumPartType"/>
        <rdfs:label>solo</rdfs:label>
        <skos:definition>For mediums of performance marked &quot;solo&quot; in a score or otherwise.</skos:definition>
    </owl:NamedIndividual>
    


    <!-- http://performedmusicontology.org/45 -->

    <owl:NamedIndividual rdf:about="http://performedmusicontology.org/45">
        <rdf:type rdf:resource="http://id.loc.gov/ontologies/bibframe/Carrier"/>
        <rdfs:label>45 recording</rdfs:label>
        <skos:definition>Colloquial term representing 7&quot; diameter vinyl audio discs with a playing speed of 45 rpm. The term does not necessarily accurately describe the carrier.</skos:definition>
    </owl:NamedIndividual>
    


    <!-- http://performedmusicontology.org/78recording -->

    <owl:NamedIndividual rdf:about="http://performedmusicontology.org/78recording">
        <rdf:type rdf:resource="http://id.loc.gov/ontologies/bibframe/Carrier"/>
        <rdfs:label>78 recording</rdfs:label>
        <skos:definition>Colloquial term representing audio discs from the 78 rpm disc era, with actual playing speeds ranging from around 60 rpm to 130 rpm.The term does not necessarily accurately describe the carrier.</skos:definition>
    </owl:NamedIndividual>
    


    <!-- http://performedmusicontology.org/ontology/AAC -->

    <owl:NamedIndividual rdf:about="http://performedmusicontology.org/ontology/AAC">
        <rdf:type rdf:resource="http://id.loc.gov/ontologies/bibframe/EncodingFormat"/>
        <skos:definition>Advanced Audio Coding format, a proprietary audio coding standard for lossy digital audio compression.</skos:definition>
    </owl:NamedIndividual>
    


    <!-- http://performedmusicontology.org/ontology/AIFF -->

    <owl:NamedIndividual rdf:about="http://performedmusicontology.org/ontology/AIFF">
        <rdf:type rdf:resource="http://id.loc.gov/ontologies/bibframe/EncodingFormat"/>
        <skos:definition>Standard audio file format used by Apple.</skos:definition>
    </owl:NamedIndividual>
    


    <!-- http://performedmusicontology.org/ontology/CdAudio -->

    <owl:NamedIndividual rdf:about="http://performedmusicontology.org/ontology/CdAudio">
        <rdf:type rdf:resource="http://id.loc.gov/ontologies/bibframe/Carrier"/>
        <rdfs:label>CD Audio</rdfs:label>
        <skos:broader rdf:resource="http://rdaregistry.info/termList/RDACarrierType/1004"/>
        <skos:definition>Optical discs that use the standard compact disc format for audio. They are 12 cm (4 3/4 in.) in diameter, and encoded as 2-channel signed 16-bit Linear PCM sampled at 44,100 Hz.</skos:definition>
    </owl:NamedIndividual>
    


    <!-- http://performedmusicontology.org/ontology/DAT -->

    <owl:NamedIndividual rdf:about="http://performedmusicontology.org/ontology/DAT">
        <rdf:type rdf:resource="http://id.loc.gov/ontologies/bibframe/Carrier"/>
        <rdfs:label>DAT (Digital Audio Tape)</rdfs:label>
        <skos:broader rdf:resource="http://rdaregistry.info/termList/RDACarrierType/1007"/>
        <skos:definition>Sony&apos;s proprietary Digital Audio Tape format, characterized by magnetic media enclosed in a protective shell, with the dimensions of 8 x 6 cm, 4 mm tape or 2 7/8 x 2 1/8 in., 1/8 in. tape</skos:definition>
    </owl:NamedIndividual>
    


    <!-- http://performedmusicontology.org/ontology/DvdAudio -->

    <owl:NamedIndividual rdf:about="http://performedmusicontology.org/ontology/DvdAudio">
        <rdf:type rdf:resource="http://id.loc.gov/ontologies/bibframe/Carrier"/>
        <rdfs:label>DVD Audio</rdfs:label>
        <skos:altLabel>DVD-A</skos:altLabel>
        <skos:broader rdf:resource="http://rdaregistry.info/termList/RDACarrierType/1004"/>
        <skos:definition>DVD optical discs that use the the DVD audio format. Different bit depth/sampling rate/channel combinations can be used on a single disc.</skos:definition>
    </owl:NamedIndividual>
    


    <!-- http://performedmusicontology.org/ontology/DvdVideo -->

    <owl:NamedIndividual rdf:about="http://performedmusicontology.org/ontology/DvdVideo">
        <rdf:type rdf:resource="http://id.loc.gov/ontologies/bibframe/Carrier"/>
        <rdfs:label>DVD Video</rdfs:label>
        <skos:broader rdf:resource="http://rdaregistry.info/termList/RDACarrierType/1060"/>
        <skos:definition>DVD optical discs that use the DVD format to store digital video. From 2003, it has been the dominant consumer video format.</skos:definition>
    </owl:NamedIndividual>
    


    <!-- http://performedmusicontology.org/ontology/EightTrack -->

    <owl:NamedIndividual rdf:about="http://performedmusicontology.org/ontology/EightTrack">
        <rdf:type rdf:resource="http://id.loc.gov/ontologies/bibframe/TapeConfig"/>
        <rdfs:label>8-track</rdfs:label>
        <skos:definition>Magnetic tape divided into 8 audio tracks that run parallel with each other, on which sound and other electro-acoustic signals are captured.</skos:definition>
    </owl:NamedIndividual>
    


    <!-- http://performedmusicontology.org/ontology/EnhancedCdAudio -->

    <owl:NamedIndividual rdf:about="http://performedmusicontology.org/ontology/EnhancedCdAudio">
        <rdf:type rdf:resource="http://id.loc.gov/ontologies/bibframe/Carrier"/>
        <rdfs:label>Enhanced CD Audio</rdfs:label>
        <skos:broader rdf:resource="http://rdaregistry.info/termList/RDACarrierType/1004"/>
        <skos:definition>An optical disc containing a combination of audio and computer data for use in both CD and CD-ROM players. Usually music CDs combined with short videos or other content.</skos:definition>
    </owl:NamedIndividual>
    


    <!-- http://performedmusicontology.org/ontology/EpRecord -->

    <owl:NamedIndividual rdf:about="http://performedmusicontology.org/ontology/EpRecord">
        <rdf:type rdf:resource="http://id.loc.gov/ontologies/bibframe/Carrier"/>
        <rdfs:label>EP (Extended play)</rdfs:label>
        <skos:broader rdf:resource="http://rdaregistry.info/termList/RDACarrierType/1004"/>
        <skos:definition>A music disc that contains more tracks than a single but not as many as on a typical album/LP/disc.</skos:definition>
    </owl:NamedIndividual>
    


    <!-- http://performedmusicontology.org/ontology/FLAC -->

    <owl:NamedIndividual rdf:about="http://performedmusicontology.org/ontology/FLAC">
        <rdf:type rdf:resource="http://id.loc.gov/ontologies/bibframe/EncodingFormat"/>
        <skos:definition>Free Lossless Audio Codec, an open audio coding format for lossless compression of digital audio.</skos:definition>
    </owl:NamedIndividual>
    


    <!-- http://performedmusicontology.org/ontology/FullTrack -->

    <owl:NamedIndividual rdf:about="http://performedmusicontology.org/ontology/FullTrack">
        <rdf:type rdf:resource="http://id.loc.gov/ontologies/bibframe/TapeConfig"/>
        <rdfs:label>full track</rdfs:label>
        <skos:definition>Magnetic tape with 1 audio track on which sound and other electro-acoustic signals are captured.</skos:definition>
    </owl:NamedIndividual>
    


    <!-- http://performedmusicontology.org/ontology/HalfTrack -->

    <owl:NamedIndividual rdf:about="http://performedmusicontology.org/ontology/HalfTrack">
        <rdf:type rdf:resource="http://id.loc.gov/ontologies/bibframe/TapeConfig"/>
        <rdfs:label>half track</rdfs:label>
        <skos:definition>Magnetic tape divided into 2 audio tracks that run parallel with each other, on which sound and other electro-acoustic signals are captured.</skos:definition>
    </owl:NamedIndividual>
    


    <!-- http://performedmusicontology.org/ontology/HybridSacd -->

    <owl:NamedIndividual rdf:about="http://performedmusicontology.org/ontology/HybridSacd">
        <rdf:type rdf:resource="http://id.loc.gov/ontologies/bibframe/Carrier"/>
        <rdfs:label>Hybrid SACD</rdfs:label>
        <skos:broader rdf:resource="http://rdaregistry.info/termList/RDACarrierType/1004"/>
        <skos:definition>An SACD that also is also encoded with a PCM audio layer readable by compact disc players.</skos:definition>
    </owl:NamedIndividual>
    


    <!-- http://performedmusicontology.org/ontology/IPS.9 -->

    <owl:NamedIndividual rdf:about="http://performedmusicontology.org/ontology/IPS.9">
        <rdf:type rdf:resource="http://id.loc.gov/ontologies/bibframe/PlayingSpeed"/>
        <rdfs:comment>Speed occurs on half-speed mini-cassettes used in small portable recorders.</rdfs:comment>
        <rdfs:label>15/16 ips</rdfs:label>
        <skos:definition>Playing speed of 15/16 inches per second.</skos:definition>
    </owl:NamedIndividual>
    


    <!-- http://performedmusicontology.org/ontology/IPS1.8 -->

    <owl:NamedIndividual rdf:about="http://performedmusicontology.org/ontology/IPS1.8">
        <rdf:type rdf:resource="http://id.loc.gov/ontologies/bibframe/PlayingSpeed"/>
        <rdfs:comment>Speed occurs on standard audiocassettes.</rdfs:comment>
        <rdfs:label>1 7/8 ips</rdfs:label>
        <skos:definition>Playing speed of 1 7/8 inches per second.</skos:definition>
    </owl:NamedIndividual>
    


    <!-- http://performedmusicontology.org/ontology/IPS15 -->

    <owl:NamedIndividual rdf:about="http://performedmusicontology.org/ontology/IPS15">
        <rdf:type rdf:resource="http://id.loc.gov/ontologies/bibframe/PlayingSpeed"/>
        <rdfs:comment>Occcurs on reel-to-reel, studio tapes.</rdfs:comment>
        <rdfs:label>15 ips</rdfs:label>
        <skos:definition>Playing speed of 15 inches per second.</skos:definition>
    </owl:NamedIndividual>
    


    <!-- http://performedmusicontology.org/ontology/IPS3.75 -->

    <owl:NamedIndividual rdf:about="http://performedmusicontology.org/ontology/IPS3.75">
        <rdf:type rdf:resource="http://id.loc.gov/ontologies/bibframe/PlayingSpeed"/>
        <rdfs:comment>Speed occurs on consumer and nonprofessional reel-to-reel tapes, cartridges and very unusual cassette tapes.</rdfs:comment>
        <rdfs:label>3.75 ips</rdfs:label>
        <skos:definition>Playing speed of 3.75 inches per second</skos:definition>
    </owl:NamedIndividual>
    


    <!-- http://performedmusicontology.org/ontology/IPS30 -->

    <owl:NamedIndividual rdf:about="http://performedmusicontology.org/ontology/IPS30">
        <rdf:type rdf:resource="http://id.loc.gov/ontologies/bibframe/PlayingSpeed"/>
        <rdfs:comment>Occurs on reel-to-reel, studio tapes, but is rarely used.</rdfs:comment>
        <rdfs:label>30 ips</rdfs:label>
        <skos:definition>Playing speed of 30 inches per second.</skos:definition>
    </owl:NamedIndividual>
    


    <!-- http://performedmusicontology.org/ontology/IPS7.5 -->

    <owl:NamedIndividual rdf:about="http://performedmusicontology.org/ontology/IPS7.5">
        <rdf:type rdf:resource="http://id.loc.gov/ontologies/bibframe/PlayingSpeed"/>
        <rdfs:comment>Speed occurs in reel-to-reel, nonprofessional, and studio tapes.</rdfs:comment>
        <rdfs:label>7.5 ips</rdfs:label>
        <skos:definition>Playing speed of 7.5 inches per second.</skos:definition>
    </owl:NamedIndividual>
    


    <!-- http://performedmusicontology.org/ontology/LP -->

    <owl:NamedIndividual rdf:about="http://performedmusicontology.org/ontology/LP">
        <rdf:type rdf:resource="http://id.loc.gov/ontologies/bibframe/Carrier"/>
        <rdfs:label>LP/Vinyl</rdfs:label>
        <skos:broader rdf:resource="http://rdaregistry.info/termList/RDACarrierType/1004"/>
        <skos:definition>Colloquial term representing 12&quot; diameter vinyl audio discs with a playing speed of 33 1/3 rpm. The term does not necessarily accurately describe the carrier.</skos:definition>
    </owl:NamedIndividual>
    


    <!-- http://performedmusicontology.org/ontology/LateralCut -->

    <owl:NamedIndividual rdf:about="http://performedmusicontology.org/ontology/LateralCut">
        <rdf:type rdf:resource="http://performedmusicontology.org/ontology/DiscCutting"/>
        <rdfs:label>Lateral cut</rdfs:label>
        <skos:definition>Recording process in which a stylus cuts a side-to-side groove into a phonograph record.</skos:definition>
    </owl:NamedIndividual>
    


    <!-- http://performedmusicontology.org/ontology/MP3 -->

    <owl:NamedIndividual rdf:about="http://performedmusicontology.org/ontology/MP3">
        <rdf:type rdf:resource="http://id.loc.gov/ontologies/bibframe/EncodingFormat"/>
        <rdfs:comment>MPEG Layer III Audio, and audio encoding format for digital audio.</rdfs:comment>
    </owl:NamedIndividual>
    


    <!-- http://performedmusicontology.org/ontology/MPS1.4 -->

    <owl:NamedIndividual rdf:about="http://performedmusicontology.org/ontology/MPS1.4">
        <rdf:type rdf:resource="http://id.loc.gov/ontologies/bibframe/PlayingSpeed"/>
        <rdfs:comment>Speed is calculated from the distance the playback mechanism covers on the surface of the disc per second, and not the number of revolutions of the disc. It is associated with compact discs (CDs)</rdfs:comment>
        <rdfs:label>1.4 mps</rdfs:label>
        <skos:definition>Playing speed of 1.4 meters per second.</skos:definition>
    </owl:NamedIndividual>
    


    <!-- http://performedmusicontology.org/ontology/OrganRoll -->

    <owl:NamedIndividual rdf:about="http://performedmusicontology.org/ontology/OrganRoll">
        <rdf:type rdf:resource="http://id.loc.gov/ontologies/bibframe/Carrier"/>
        <rdfs:label>Organ roll</rdfs:label>
        <skos:broader rdf:resource="http://rdaregistry.info/termList/RDACarrierType/1006"/>
        <skos:definition>An audio roll used to operate a player piano or reproducing organ.</skos:definition>
    </owl:NamedIndividual>
    


    <!-- http://performedmusicontology.org/ontology/PianoRoll -->

    <owl:NamedIndividual rdf:about="http://performedmusicontology.org/ontology/PianoRoll">
        <rdf:type rdf:resource="http://id.loc.gov/ontologies/bibframe/Carrier"/>
        <rdfs:label>Piano roll</rdfs:label>
        <skos:broader rdf:resource="http://rdaregistry.info/termList/RDACarrierType/1006"/>
        <skos:definition>Audio roll used to operate a player piano or reproducing piano.</skos:definition>
    </owl:NamedIndividual>
    


    <!-- http://performedmusicontology.org/ontology/QuarterTrack -->

    <owl:NamedIndividual rdf:about="http://performedmusicontology.org/ontology/QuarterTrack">
        <rdf:type rdf:resource="http://id.loc.gov/ontologies/bibframe/TapeConfig"/>
        <rdfs:label>quarter track</rdfs:label>
        <skos:definition>Magnetic tape divided into 4 audio tracks that run parallel with each other, in which sound and other electro-acoustic signals are captured.</skos:definition>
    </owl:NamedIndividual>
    


    <!-- http://performedmusicontology.org/ontology/RPM16 -->

    <owl:NamedIndividual rdf:about="http://performedmusicontology.org/ontology/RPM16">
        <rdf:type rdf:resource="http://id.loc.gov/ontologies/bibframe/PlayingSpeed"/>
        <rdfs:comment>For audio discs</rdfs:comment>
        <rdfs:label>16 rpm</rdfs:label>
        <skos:definition>Playing speed of 16 revolutions per minute.</skos:definition>
    </owl:NamedIndividual>
    


    <!-- http://performedmusicontology.org/ontology/RPM33 -->

    <owl:NamedIndividual rdf:about="http://performedmusicontology.org/ontology/RPM33">
        <rdf:type rdf:resource="http://id.loc.gov/ontologies/bibframe/PlayingSpeed"/>
        <rdfs:comment>For audio discs.</rdfs:comment>
        <rdfs:label>33 1/3 rpm</rdfs:label>
        <skos:definition>Playing speed of 33 1/3 revolutions per minute. Often shortened to &quot;33&quot;.</skos:definition>
    </owl:NamedIndividual>
    


    <!-- http://performedmusicontology.org/ontology/RPM45 -->

    <owl:NamedIndividual rdf:about="http://performedmusicontology.org/ontology/RPM45">
        <rdf:type rdf:resource="http://id.loc.gov/ontologies/bibframe/PlayingSpeed"/>
        <rdfs:comment>For audio discs.</rdfs:comment>
        <rdfs:label>45 rpm</rdfs:label>
        <skos:definition>Playing speed of 45 revolutions per minute.</skos:definition>
    </owl:NamedIndividual>
    


    <!-- http://performedmusicontology.org/ontology/RPM78 -->

    <owl:NamedIndividual rdf:about="http://performedmusicontology.org/ontology/RPM78">
        <rdf:type rdf:resource="http://id.loc.gov/ontologies/bibframe/PlayingSpeed"/>
        <rdfs:comment>For audio discs</rdfs:comment>
        <rdfs:label>78 rpm</rdfs:label>
        <skos:definition>Playing speed of 78 revolutions per minute.</skos:definition>
    </owl:NamedIndividual>
    


    <!-- http://performedmusicontology.org/ontology/RPM8 -->

    <owl:NamedIndividual rdf:about="http://performedmusicontology.org/ontology/RPM8">
        <rdf:type rdf:resource="http://id.loc.gov/ontologies/bibframe/PlayingSpeed"/>
        <rdfs:comment>For audio discs</rdfs:comment>
        <rdfs:label>8 rpm</rdfs:label>
        <skos:definition>Playing speed of 8 revolutions per minute.</skos:definition>
    </owl:NamedIndividual>
    


    <!-- http://performedmusicontology.org/ontology/Sacd -->

    <owl:NamedIndividual rdf:about="http://performedmusicontology.org/ontology/Sacd">
        <rdf:type rdf:resource="http://id.loc.gov/ontologies/bibframe/Carrier"/>
        <rdfs:label>SACD</rdfs:label>
        <skos:altLabel>Super audio compact disc</skos:altLabel>
        <skos:broader rdf:resource="http://rdaregistry.info/termList/RDACarrierType/1004"/>
        <skos:definition>Optical audio disc with more channels and longer playing time than a conventional CD.</skos:definition>
    </owl:NamedIndividual>
    


    <!-- http://performedmusicontology.org/ontology/SixteenTrack -->

    <owl:NamedIndividual rdf:about="http://performedmusicontology.org/ontology/SixteenTrack">
        <rdf:type rdf:resource="http://id.loc.gov/ontologies/bibframe/TapeConfig"/>
        <rdfs:label>16-track</rdfs:label>
        <skos:definition>Magnetic tape divided into 16 audio tracks that run parallel with each other, on which sound and other electro-acoustic signals are captured.</skos:definition>
    </owl:NamedIndividual>
    


    <!-- http://performedmusicontology.org/ontology/TwelveTrack -->

    <owl:NamedIndividual rdf:about="http://performedmusicontology.org/ontology/TwelveTrack">
        <rdf:type rdf:resource="http://id.loc.gov/ontologies/bibframe/TapeConfig"/>
        <rdfs:label>12-track</rdfs:label>
        <skos:definition>Magnetic tape divided into 12 audio tracks that run parallel with each other, on which sound and other electro-acoustic signals are captured.</skos:definition>
    </owl:NamedIndividual>
    


    <!-- http://performedmusicontology.org/ontology/Vertical -->

    <owl:NamedIndividual rdf:about="http://performedmusicontology.org/ontology/Vertical">
        <rdf:type rdf:resource="http://performedmusicontology.org/ontology/DiscCutting"/>
        <rdfs:label>Vertical cut</rdfs:label>
        <skos:altLabel>Hill and dale</skos:altLabel>
        <skos:definition>Recording process in which a stylus cuts a vertical groove into a phonograph record.</skos:definition>
    </owl:NamedIndividual>
    


    <!-- http://rdaregistry.info/termList/RDACarrierType -->

    <owl:NamedIndividual rdf:about="http://rdaregistry.info/termList/RDACarrierType">
        <rdf:type rdf:resource="http://www.w3.org/2004/02/skos/core#ConceptScheme"/>
        <dc:title>RDA Carrier Type</dc:title>
    </owl:NamedIndividual>
    


    <!-- http://rdaregistry.info/termList/RDACarrierType/1004 -->

    <owl:NamedIndividual rdf:about="http://rdaregistry.info/termList/RDACarrierType/1004">
        <rdf:type rdf:resource="http://id.loc.gov/ontologies/bibframe/Carrier"/>
        <rdf:type rdf:resource="http://www.w3.org/2004/02/skos/core#Concept"/>
        <skos:inScheme rdf:resource="http://rdaregistry.info/termList/RDACarrierType"/>
        <rdakit:toolkitDefinition xml:lang="en">A carrier type consisting of a disc on which sound waves, recorded as modulations, pulses, etc., are incised or indented in a continuous spiral groove.</rdakit:toolkitDefinition>
        <rdakit:toolkitDefinition xml:lang="es">Disco en el que las ondas sonoras, registradas como modulaciones, pulsos, etc., se registraron mediante incisiones o muescas en un surco en espiral continua.</rdakit:toolkitDefinition>
        <rdakit:toolkitDefinition xml:lang="fr">Disque sur lequel les ondulations sonores, enregistrées sous forme de modulations, impulsions, etc. ont été gravées au moyen d’une entaille ou d’empreintes en créant un sillon continu en spirale.</rdakit:toolkitDefinition>
        <rdakit:toolkitDefinition xml:lang="nl">Een disc waarop geluidsgolven, opgeslagen als modulaties, pulsen etc., ingesneden of ingesprongen zijn in een continue spiraalvormige groef.</rdakit:toolkitDefinition>
        <rdakit:toolkitDefinition xml:lang="de">Ein Datenträgertyp, der aus einer Disk besteht, auf der als Modulation, Pulse usw. aufgenommene Schallwellen in einer fortlaufend gewundenen Rille graviert oder eingeprägt sind.</rdakit:toolkitDefinition>
        <rdakit:toolkitDefinition xml:lang="vi">Loại hộp chứa gồm có đĩa trên đó sóng âm ghi lại như là chuyển giọng, nhịp điệu, vv... được vạch hoặc rập trong đường rãnh xoắn ốc liên tục.</rdakit:toolkitDefinition>
        <rdakit:toolkitDefinition xml:lang="ca">Tipus de suport físic que consisteix en un disc en el qual s’han gravat ones sonores, enregistrades com a modulacions, impulsos, etc., per mitjà d’incisions o marques en un solc continu en espiral.</rdakit:toolkitDefinition>
        <rdakit:toolkitDefinition xml:lang="zh">通过刻痕或连续的螺旋式纹槽在其上将声波记录为音调、节奏等的盘片。</rdakit:toolkitDefinition>
        <rdakit:toolkitLabel xml:lang="de">Audiodisk</rdakit:toolkitLabel>
        <rdakit:toolkitLabel xml:lang="en">audio disc</rdakit:toolkitLabel>
        <rdakit:toolkitLabel xml:lang="nl">audiodisc</rdakit:toolkitLabel>
        <rdakit:toolkitLabel xml:lang="ca">disc àudio</rdakit:toolkitLabel>
        <rdakit:toolkitLabel xml:lang="it">disco audio</rdakit:toolkitLabel>
        <rdakit:toolkitLabel xml:lang="es">disco sonoro</rdakit:toolkitLabel>
        <rdakit:toolkitLabel xml:lang="fr">disque audio</rdakit:toolkitLabel>
        <rdakit:toolkitLabel xml:lang="sv">ljudskiva</rdakit:toolkitLabel>
        <rdakit:toolkitLabel xml:lang="fi">äänilevy</rdakit:toolkitLabel>
        <rdakit:toolkitLabel xml:lang="vi">đĩa audio</rdakit:toolkitLabel>
        <rdakit:toolkitLabel xml:lang="zh">录音盘</rdakit:toolkitLabel>
        <regap:identifier rdf:resource="http://metadataregistry.org/concepts/536"/>
        <rdfs:label>Audio disc</rdfs:label>
        <skos:altLabel xml:lang="ca">disc sonor</skos:altLabel>
        <skos:altLabel xml:lang="es">disco de audio</skos:altLabel>
        <skos:altLabel xml:lang="en">sound disc</skos:altLabel>
        <skos:altLabel xml:lang="vi">đĩa âm thanh</skos:altLabel>
        <skos:altLabel xml:lang="zh">声音盘</skos:altLabel>
        <skos:definition xml:lang="en">A carrier type consisting of a disc on which sound waves, recorded as modulations, pulses, etc., are incised or indented in a continuous spiral groove.</skos:definition>
        <skos:definition xml:lang="es">Disco en el que las ondas sonoras, registradas como modulaciones, pulsos, etc., se registraron mediante incisiones o muescas en un surco en espiral continua.</skos:definition>
        <skos:definition xml:lang="fr">Disque sur lequel les ondulations sonores, enregistrées sous forme de modulations, impulsions, etc. ont été gravées au moyen d’une entaille ou d’empreintes en créant un sillon continu en spirale.</skos:definition>
        <skos:definition xml:lang="nl">Een disc waarop geluidsgolven, opgeslagen als modulaties, pulsen etc., ingesneden of ingesprongen zijn in een continue spiraalvormige groef.</skos:definition>
        <skos:definition xml:lang="de">Ein Datenträgertyp, der aus einer Disk besteht, auf der als Modulation, Pulse usw. aufgenommene Schallwellen in einer fortlaufend gewundenen Rille graviert oder eingeprägt sind.</skos:definition>
        <skos:definition xml:lang="vi">Loại hộp chứa gồm có đĩa trên đó sóng âm ghi lại như là chuyển giọng, nhịp điệu, vv... được vạch hoặc rập trong đường rãnh xoắn ốc liên tục.</skos:definition>
        <skos:definition xml:lang="ca">Tipus de suport físic que consisteix en un disc en el qual s’han gravat ones sonores, enregistrades com a modulacions, impulsos, etc., per mitjà d’incisions o marques en un solc continu en espiral.</skos:definition>
        <skos:definition xml:lang="zh">通过刻痕或连续的螺旋式纹槽在其上将声波记录为音调、节奏等的盘片。</skos:definition>
        <skos:narrower rdf:resource="http://performedmusicontology.org/45"/>
        <skos:narrower rdf:resource="http://performedmusicontology.org/78recording"/>
        <skos:narrower rdf:resource="http://performedmusicontology.org/ontology/DvdAudio"/>
        <skos:narrower rdf:resource="http://performedmusicontology.org/ontology/EnhancedCdAudio"/>
        <skos:narrower rdf:resource="http://performedmusicontology.org/ontology/EpRecord"/>
        <skos:narrower rdf:resource="http://performedmusicontology.org/ontology/HybridSacd"/>
        <skos:narrower rdf:resource="http://performedmusicontology.org/ontology/LP"/>
        <skos:narrower rdf:resource="http://performedmusicontology.org/ontology/RPM33"/>
        <skos:narrower rdf:resource="http://performedmusicontology.org/ontology/Sacd"/>
        <skos:prefLabel xml:lang="de">Audiodisk</skos:prefLabel>
        <skos:prefLabel xml:lang="en">audio disc</skos:prefLabel>
        <skos:prefLabel xml:lang="nl">audiodisc</skos:prefLabel>
        <skos:prefLabel xml:lang="ca">disc àudio</skos:prefLabel>
        <skos:prefLabel xml:lang="it">disco audio</skos:prefLabel>
        <skos:prefLabel xml:lang="es">disco sonoro</skos:prefLabel>
        <skos:prefLabel xml:lang="fr">disque audio</skos:prefLabel>
        <skos:prefLabel xml:lang="sv">ljudskiva</skos:prefLabel>
        <skos:prefLabel xml:lang="fi">äänilevy</skos:prefLabel>
        <skos:prefLabel xml:lang="vi">đĩa audio</skos:prefLabel>
        <skos:prefLabel xml:lang="ar">قرص صوتي</skos:prefLabel>
        <skos:prefLabel xml:lang="zh">录音盘</skos:prefLabel>
    </owl:NamedIndividual>
    


    <!-- http://rdaregistry.info/termList/RDACarrierType/1006 -->

    <owl:NamedIndividual rdf:about="http://rdaregistry.info/termList/RDACarrierType/1006">
        <rdf:type rdf:resource="http://id.loc.gov/ontologies/bibframe/Carrier"/>
        <rdf:type rdf:resource="http://www.w3.org/2004/02/skos/core#Concept"/>
        <skos:inScheme rdf:resource="http://rdaregistry.info/termList/RDACarrierType"/>
        <rdakit:toolkitDefinition xml:lang="en">A carrier type consisting of a roll of paper on which musical notes are represented by perforations, designed to mechanically reproduce the music when used in a player piano, player organ, etc.</rdakit:toolkitDefinition>
        <rdakit:toolkitDefinition xml:lang="nl">Een rol papier waarop muzieknoten voorgesteld worden door perforaties, ontworpen om mechanisch de muziek weer te geven wanneer deze gebruikt wordt in een pianola e.d.</rdakit:toolkitDefinition>
        <rdakit:toolkitDefinition xml:lang="de">Ein Datenträgertyp, der aus einer Papierrolle besteht, auf der Musiknoten in Form von Perforationen repräsentiert werden und die konzipiert ist, um Musik in einem mechanischen Klavier, einer mechanischen Orgel usw. wiederzugeben.</rdakit:toolkitDefinition>
        <rdakit:toolkitDefinition xml:lang="vi">Loại hộp chứa gồm có cuốn giấy trên đó nốt nhạc được trình bày bởi các lỗ răng cưa để tái tạo một cách cơ học âm nhạc khi dùng với piano tự động, organ tự động, vv...</rdakit:toolkitDefinition>
        <rdakit:toolkitDefinition xml:lang="es">Rollo de papel en el que las notas musicales están representadas mediante perforaciones, diseñado para reproducir en forma mecánica la música cuando se utiliza en una pianola, órgano mecánico, etc.</rdakit:toolkitDefinition>
        <rdakit:toolkitDefinition xml:lang="fr">Rouleau de papier sur lequel les notes de musique sont représentées par des perforations, destiné à reproduire mécaniquement la musique lorsqu’il est utilisé avec un piano mécanique, un orgue mécanique, etc.</rdakit:toolkitDefinition>
        <rdakit:toolkitDefinition xml:lang="ca">Tipus de suport físic que consisteix en un rotlle de paper sobre el qual es representen les notes musicals amb perforacions, concebut per reproduir la música mecànicament quan s’usa en una pianola, un orgue mecànic, etc.</rdakit:toolkitDefinition>
        <rdakit:toolkitDefinition xml:lang="zh">通过穿孔方式表示音符的纸卷，用于钢琴、风琴等时，以机械方式重现音乐。</rdakit:toolkitDefinition>
        <rdakit:toolkitLabel xml:lang="de">Notenrolle</rdakit:toolkitLabel>
        <rdakit:toolkitLabel xml:lang="en">audio roll</rdakit:toolkitLabel>
        <rdakit:toolkitLabel xml:lang="nl">audiorol</rdakit:toolkitLabel>
        <rdakit:toolkitLabel xml:lang="vi">cuốn audio</rdakit:toolkitLabel>
        <rdakit:toolkitLabel xml:lang="sv">ljudrulle</rdakit:toolkitLabel>
        <rdakit:toolkitLabel xml:lang="fi">pianorulla</rdakit:toolkitLabel>
        <rdakit:toolkitLabel xml:lang="es">rollo sonoro</rdakit:toolkitLabel>
        <rdakit:toolkitLabel xml:lang="ca">rotlle àudio</rdakit:toolkitLabel>
        <rdakit:toolkitLabel xml:lang="fr">rouleau audio</rdakit:toolkitLabel>
        <rdakit:toolkitLabel xml:lang="it">rullo audio</rdakit:toolkitLabel>
        <rdakit:toolkitLabel xml:lang="zh">录音卷</rdakit:toolkitLabel>
        <regap:identifier rdf:resource="http://metadataregistry.org/concepts/538"/>
        <rdfs:label>Audio roll</rdfs:label>
        <skos:altLabel xml:lang="vi">cuốn piano</skos:altLabel>
        <skos:altLabel xml:lang="en">piano roll</skos:altLabel>
        <skos:altLabel xml:lang="es">rollo de piano</skos:altLabel>
        <skos:altLabel xml:lang="zh">钢琴滚筒</skos:altLabel>
        <skos:definition xml:lang="en">A carrier type consisting of a roll of paper on which musical notes are represented by perforations, designed to mechanically reproduce the music when used in a player piano, player organ, etc.</skos:definition>
        <skos:definition xml:lang="nl">Een rol papier waarop muzieknoten voorgesteld worden door perforaties, ontworpen om mechanisch de muziek weer te geven wanneer deze gebruikt wordt in een pianola e.d.</skos:definition>
        <skos:definition xml:lang="de">Ein Datenträgertyp, der aus einer Papierrolle besteht, auf der Musiknoten in Form von Perforationen repräsentiert werden und die konzipiert ist, um Musik in einem mechanischen Klavier, einer mechanischen Orgel usw. wiederzugeben.</skos:definition>
        <skos:definition xml:lang="vi">Loại hộp chứa gồm có cuốn giấy trên đó nốt nhạc được trình bày bởi các lỗ răng cưa để tái tạo một cách cơ học âm nhạc khi dùng với piano tự động, organ tự động, vv...</skos:definition>
        <skos:definition xml:lang="es">Rollo de papel en el que las notas musicales están representadas mediante perforaciones, diseñado para reproducir en forma mecánica la música cuando se utiliza en una pianola, órgano mecánico, etc.</skos:definition>
        <skos:definition xml:lang="fr">Rouleau de papier sur lequel les notes de musique sont représentées par des perforations, destiné à reproduire mécaniquement la musique lorsqu’il est utilisé avec un piano mécanique, un orgue mécanique, etc.</skos:definition>
        <skos:definition xml:lang="ca">Tipus de suport físic que consisteix en un rotlle de paper sobre el qual es representen les notes musicals amb perforacions, concebut per reproduir la música mecànicament quan s’usa en una pianola, un orgue mecànic, etc.</skos:definition>
        <skos:definition xml:lang="zh">通过穿孔方式表示音符的纸卷，用于钢琴、风琴等时，以机械方式重现音乐。</skos:definition>
        <skos:narrower rdf:resource="http://performedmusicontology.org/ontology/OrganRoll"/>
        <skos:narrower rdf:resource="http://performedmusicontology.org/ontology/PianoRoll"/>
        <skos:prefLabel xml:lang="de">Notenrolle</skos:prefLabel>
        <skos:prefLabel xml:lang="en">audio roll</skos:prefLabel>
        <skos:prefLabel xml:lang="nl">audiorol</skos:prefLabel>
        <skos:prefLabel xml:lang="vi">cuốn audio</skos:prefLabel>
        <skos:prefLabel xml:lang="sv">ljudrulle</skos:prefLabel>
        <skos:prefLabel xml:lang="fi">pianorulla</skos:prefLabel>
        <skos:prefLabel xml:lang="es">rollo sonoro</skos:prefLabel>
        <skos:prefLabel xml:lang="ca">rotlle àudio</skos:prefLabel>
        <skos:prefLabel xml:lang="fr">rouleau audio</skos:prefLabel>
        <skos:prefLabel xml:lang="it">rullo audio</skos:prefLabel>
        <skos:prefLabel xml:lang="ar">لفافة سمعية</skos:prefLabel>
        <skos:prefLabel xml:lang="zh">录音卷</skos:prefLabel>
        <skos:scopeNote xml:lang="fr">Comprend les rouleaux pour piano, etc.</skos:scopeNote>
        <skos:scopeNote xml:lang="es">Incluye rollos de pianola, etc.</skos:scopeNote>
        <skos:scopeNote xml:lang="zh">用于钢琴滚筒等。</skos:scopeNote>
    </owl:NamedIndividual>
    


    <!-- http://rdaregistry.info/termList/RDACarrierType/1007 -->

    <owl:NamedIndividual rdf:about="http://rdaregistry.info/termList/RDACarrierType/1007">
        <rdf:type rdf:resource="http://id.loc.gov/ontologies/bibframe/Carrier"/>
        <rdf:type rdf:resource="http://www.w3.org/2004/02/skos/core#Concept"/>
        <skos:inScheme rdf:resource="http://rdaregistry.info/termList/RDACarrierType"/>
        <rdakit:toolkitDefinition xml:lang="en">A carrier type consisting of a cassette containing an audiotape.</rdakit:toolkitDefinition>
        <rdakit:toolkitDefinition xml:lang="es">Casete que contiene una cinta de audio.</rdakit:toolkitDefinition>
        <rdakit:toolkitDefinition xml:lang="fr">Cassette contenant une bande audio.</rdakit:toolkitDefinition>
        <rdakit:toolkitDefinition xml:lang="nl">Een cassette die een audiotape bevat.</rdakit:toolkitDefinition>
        <rdakit:toolkitDefinition xml:lang="de">Ein Datenträgertyp, der aus einer Kassette besteht, die ein Tonband enthält.</rdakit:toolkitDefinition>
        <rdakit:toolkitDefinition xml:lang="vi">Loại hộp chứa gồm có cassette chứa một băng audio.</rdakit:toolkitDefinition>
        <rdakit:toolkitDefinition xml:lang="ca">Tipus de suport físic que consisteix en una casset que conté una cinta àudio.</rdakit:toolkitDefinition>
        <rdakit:toolkitDefinition xml:lang="zh">装在双轴盒中的录音带。</rdakit:toolkitDefinition>
        <rdakit:toolkitLabel xml:lang="de">Audiokassette</rdakit:toolkitLabel>
        <rdakit:toolkitLabel xml:lang="es">audiocasete</rdakit:toolkitLabel>
        <rdakit:toolkitLabel xml:lang="it">audiocassetta</rdakit:toolkitLabel>
        <rdakit:toolkitLabel xml:lang="en">audiocassette</rdakit:toolkitLabel>
        <rdakit:toolkitLabel xml:lang="nl">audiocassette</rdakit:toolkitLabel>
        <rdakit:toolkitLabel xml:lang="vi">audiocassette</rdakit:toolkitLabel>
        <rdakit:toolkitLabel xml:lang="ca">casset àudio</rdakit:toolkitLabel>
        <rdakit:toolkitLabel xml:lang="fr">cassette audio</rdakit:toolkitLabel>
        <rdakit:toolkitLabel xml:lang="sv">ljudkassett</rdakit:toolkitLabel>
        <rdakit:toolkitLabel xml:lang="fi">äänikasetti</rdakit:toolkitLabel>
        <rdakit:toolkitLabel xml:lang="zh">卡式录音带</rdakit:toolkitLabel>
        <regap:identifier rdf:resource="http://metadataregistry.org/concepts/539"/>
        <rdfs:label>Audiocassette</rdfs:label>
        <skos:definition xml:lang="en">A carrier type consisting of a cassette containing an audiotape.</skos:definition>
        <skos:definition xml:lang="es">Casete que contiene una cinta de audio.</skos:definition>
        <skos:definition xml:lang="fr">Cassette contenant une bande audio.</skos:definition>
        <skos:definition xml:lang="nl">Een cassette die een audiotape bevat.</skos:definition>
        <skos:definition xml:lang="de">Ein Datenträgertyp, der aus einer Kassette besteht, die ein Tonband enthält.</skos:definition>
        <skos:definition xml:lang="vi">Loại hộp chứa gồm có cassette chứa một băng audio.</skos:definition>
        <skos:definition xml:lang="ca">Tipus de suport físic que consisteix en una casset que conté una cinta àudio.</skos:definition>
        <skos:definition xml:lang="zh">装在双轴盒中的录音带。</skos:definition>
        <skos:narrower rdf:resource="http://performedmusicontology.org/ontology/DAT"/>
        <skos:narrower></skos:narrower>
        <skos:prefLabel xml:lang="de">Audiokassette</skos:prefLabel>
        <skos:prefLabel xml:lang="es">audiocasete</skos:prefLabel>
        <skos:prefLabel xml:lang="it">audiocassetta</skos:prefLabel>
        <skos:prefLabel xml:lang="en">audiocassette</skos:prefLabel>
        <skos:prefLabel xml:lang="nl">audiocassette</skos:prefLabel>
        <skos:prefLabel xml:lang="vi">audiocassette</skos:prefLabel>
        <skos:prefLabel xml:lang="ca">casset àudio</skos:prefLabel>
        <skos:prefLabel xml:lang="fr">cassette audio</skos:prefLabel>
        <skos:prefLabel xml:lang="sv">ljudkassett</skos:prefLabel>
        <skos:prefLabel xml:lang="fi">äänikasetti</skos:prefLabel>
        <skos:prefLabel xml:lang="ar">كاسيت صوتي</skos:prefLabel>
        <skos:prefLabel xml:lang="zh">卡式录音带</skos:prefLabel>
    </owl:NamedIndividual>
    


    <!-- http://rdaregistry.info/termList/RDACarrierType/1060 -->

    <owl:NamedIndividual rdf:about="http://rdaregistry.info/termList/RDACarrierType/1060">
        <rdf:type rdf:resource="http://id.loc.gov/ontologies/bibframe/Carrier"/>
        <rdf:type rdf:resource="http://www.w3.org/2004/02/skos/core#Concept"/>
        <skos:inScheme rdf:resource="http://rdaregistry.info/termList/RDACarrierType"/>
        <rdakit:toolkitDefinition xml:lang="en">A carrier type consisting of a disc on which video signals, with or without sound, are recorded.</rdakit:toolkitDefinition>
        <rdakit:toolkitDefinition xml:lang="es">Disco sobre el que se han grabado señales de video, con o sin sonido.</rdakit:toolkitDefinition>
        <rdakit:toolkitDefinition xml:lang="fr">Disque sur lequel des signaux vidéo, accompagnés de son ou non, sont enregistrés.</rdakit:toolkitDefinition>
        <rdakit:toolkitDefinition xml:lang="nl">Een disc waarop videosignalen, met of zonder geluid, worden opgenomen.</rdakit:toolkitDefinition>
        <rdakit:toolkitDefinition xml:lang="de">Ein Datenträgertyp, der aus eine Disk besteht, auf der Video-Signale mit oder ohne Ton aufgezeichnet sind.</rdakit:toolkitDefinition>
        <rdakit:toolkitDefinition xml:lang="vi">Loại hộp chứa gồm có đĩa trên đó tín hiệu video, có hoặc không có âm thanh, được ghi lại.</rdakit:toolkitDefinition>
        <rdakit:toolkitDefinition xml:lang="ca">Tipus de suport físic que consisteix en un disc en el qual hi ha enregistrats senyals de vídeo, amb o sense so.</rdakit:toolkitDefinition>
        <rdakit:toolkitDefinition xml:lang="zh">记录视频信号的盘片，有无声音均可。</rdakit:toolkitDefinition>
        <rdakit:toolkitLabel xml:lang="de">Videodisk</rdakit:toolkitLabel>
        <rdakit:toolkitLabel xml:lang="ca">videodisc</rdakit:toolkitLabel>
        <rdakit:toolkitLabel xml:lang="en">videodisc</rdakit:toolkitLabel>
        <rdakit:toolkitLabel xml:lang="nl">videodisc</rdakit:toolkitLabel>
        <rdakit:toolkitLabel xml:lang="es">videodisco</rdakit:toolkitLabel>
        <rdakit:toolkitLabel xml:lang="it">videodisco</rdakit:toolkitLabel>
        <rdakit:toolkitLabel xml:lang="fi">videolevy</rdakit:toolkitLabel>
        <rdakit:toolkitLabel xml:lang="sv">videoskiva</rdakit:toolkitLabel>
        <rdakit:toolkitLabel xml:lang="fr">vidéodisque</rdakit:toolkitLabel>
        <rdakit:toolkitLabel xml:lang="vi">đĩa video</rdakit:toolkitLabel>
        <rdakit:toolkitLabel xml:lang="zh">视盘</rdakit:toolkitLabel>
        <regap:identifier rdf:resource="http://metadataregistry.org/concepts/1113"/>
        <rdfs:label>Videodisc</rdfs:label>
        <skos:definition xml:lang="en">A carrier type consisting of a disc on which video signals, with or without sound, are recorded.</skos:definition>
        <skos:definition xml:lang="es">Disco sobre el que se han grabado señales de video, con o sin sonido.</skos:definition>
        <skos:definition xml:lang="fr">Disque sur lequel des signaux vidéo, accompagnés de son ou non, sont enregistrés.</skos:definition>
        <skos:definition xml:lang="nl">Een disc waarop videosignalen, met of zonder geluid, worden opgenomen.</skos:definition>
        <skos:definition xml:lang="de">Ein Datenträgertyp, der aus eine Disk besteht, auf der Video-Signale mit oder ohne Ton aufgezeichnet sind.</skos:definition>
        <skos:definition xml:lang="vi">Loại hộp chứa gồm có đĩa trên đó tín hiệu video, có hoặc không có âm thanh, được ghi lại.</skos:definition>
        <skos:definition xml:lang="ca">Tipus de suport físic que consisteix en un disc en el qual hi ha enregistrats senyals de vídeo, amb o sense so.</skos:definition>
        <skos:definition xml:lang="zh">记录视频信号的盘片，有无声音均可。</skos:definition>
        <skos:narrower rdf:resource="http://performedmusicontology.org/Laserdisc"/>
        <skos:narrower rdf:resource="http://performedmusicontology.org/ontology/DvdVideo"/>
        <skos:prefLabel xml:lang="de">Videodisk</skos:prefLabel>
        <skos:prefLabel xml:lang="ca">videodisc</skos:prefLabel>
        <skos:prefLabel xml:lang="en">videodisc</skos:prefLabel>
        <skos:prefLabel xml:lang="nl">videodisc</skos:prefLabel>
        <skos:prefLabel xml:lang="es">videodisco</skos:prefLabel>
        <skos:prefLabel xml:lang="it">videodisco</skos:prefLabel>
        <skos:prefLabel xml:lang="fi">videolevy</skos:prefLabel>
        <skos:prefLabel xml:lang="sv">videoskiva</skos:prefLabel>
        <skos:prefLabel xml:lang="fr">vidéodisque</skos:prefLabel>
        <skos:prefLabel xml:lang="vi">đĩa video</skos:prefLabel>
        <skos:prefLabel xml:lang="ar">قرص فيديو</skos:prefLabel>
        <skos:prefLabel xml:lang="zh">视盘</skos:prefLabel>
    </owl:NamedIndividual>
    


    <!-- 
    ///////////////////////////////////////////////////////////////////////////////////////
    //
    // Annotations
    //
    ///////////////////////////////////////////////////////////////////////////////////////
     -->

    <rdf:Description rdf:about="http://performedmusicontology.org/ontology/hasMusicPart">
        <skos:definition>Specific role or type of a medium part, e.g., solo, ad lib, optional, offstage.</skos:definition>
    </rdf:Description>
</rdf:RDF>



<!-- Generated by the OWL API (version 4.2.8.20170104-2310) https://github.com/owlcs/owlapi -->

