@prefix : <http://performedmusicontology.org/ontology/> .
@prefix ns: <http://creativecommons.org/ns#> .
@prefix owl: <http://www.w3.org/2002/07/owl#> .
@prefix rdf: <http://www.w3.org/1999/02/22-rdf-syntax-ns#> .
@prefix xml: <http://www.w3.org/XML/1998/namespace> .
@prefix xsd: <http://www.w3.org/2001/XMLSchema#> .
@prefix rdfs: <http://www.w3.org/2000/01/rdf-schema#> .
@prefix skos: <http://www.w3.org/2004/02/skos/core#> .
@prefix terms: <http://purl.org/dc/terms/> .
@base <http://performedmusicontology.org/ontology/> .

<http://performedmusicontology.org/ontology/> rdf:type owl:Ontology ;
                                               owl:versionIRI <http://performedmusicontology.org/ontology/2.0> ;
                                               owl:imports <http://id.loc.gov/ontologies/bibframe-2-0-1/> .

#################################################################
#    Annotation properties
#################################################################

###  http://www.w3.org/2004/02/skos/core#definition
skos:definition rdf:type owl:AnnotationProperty .


###  http://www.w3.org/2004/02/skos/core#example
skos:example rdf:type owl:AnnotationProperty .


#################################################################
#    Object Properties
#################################################################

###  http://performedmusicontology.org/ontology/aggregatedIn
:aggregatedIn rdf:type owl:ObjectProperty ;
              owl:inverseOf :aggregates ;
              rdfs:domain <http://id.loc.gov/ontologies/bibframe/Work> ;
              rdfs:range <http://id.loc.gov/ontologies/bibframe/Work> ;
              rdfs:label "Aggregated in"^^xsd:string ;
              skos:definition "Relates a work to a work in which it is aggregated."^^xsd:string .


###  http://performedmusicontology.org/ontology/aggregates
:aggregates rdf:type owl:ObjectProperty ;
            rdfs:domain <http://id.loc.gov/ontologies/bibframe/Work> ;
            rdfs:range <http://id.loc.gov/ontologies/bibframe/Work> ;
            rdfs:label "Aggregates"^^xsd:string ;
            skos:definition "Relates a work to a work that it aggregates."^^xsd:string .


###  http://performedmusicontology.org/ontology/asMemberOf
:asMemberOf rdf:type owl:ObjectProperty ;
            rdfs:domain <http://id.loc.gov/ontologies/bibframe/Contribution> ;
            rdfs:range <http://id.loc.gov/ontologies/bibframe/Organization> ;
            rdfs:label "As member of"^^xsd:string ;
            skos:definition "Relates a contribution that is a person to an organization through which a person makes a contribution to the resource."^^xsd:string .


###  http://performedmusicontology.org/ontology/associatedWith
:associatedWith rdf:type owl:ObjectProperty ;
                rdfs:subPropertyOf <http://id.loc.gov/ontologies/bibframe/relatedTo> ;
                rdf:type owl:SymmetricProperty ;
                rdfs:comment "Sugested use - With any resource (event, work, instance, item, agent)"^^xsd:string ;
                rdfs:label "Associated with"^^xsd:string ;
                skos:definition "Relates a resource to another resource with which it is associated in a general way."^^xsd:string ;
                skos:example "The musical work \"1812\" is associated with the event \"French invasion of Russia\""^^xsd:string .


###  http://performedmusicontology.org/ontology/createdFor
:createdFor rdf:type owl:ObjectProperty ;
            rdfs:subPropertyOf <http://id.loc.gov/ontologies/bibframe/relatedTo> ;
            rdfs:comment "Suggested use - With Agent, Event" ;
            rdfs:label "Created for"^^xsd:string ;
            skos:definition "Relates a resource to a resource for which it was created"^^xsd:string .


###  http://performedmusicontology.org/ontology/hasDramaticRole
:hasDramaticRole rdf:type owl:ObjectProperty ;
                 rdfs:domain <http://id.loc.gov/ontologies/bibframe/Contribution> ;
                 rdfs:range :DramaticRole ;
                 rdfs:label "Has dramatic role"^^xsd:string ;
                 skos:definition "Relates a contribution to a dramatic role."^^xsd:string .


###  http://performedmusicontology.org/ontology/hasEnsembleSize
:hasEnsembleSize rdf:type owl:ObjectProperty ;
                 rdfs:domain <http://id.loc.gov/ontologies/bibframe/Work> ;
                 rdfs:range :EnsembleSize ;
                 rdfs:label "Has ensemble size"^^xsd:string ;
                 skos:definition "Relates a work to an individual ensemble size."^^xsd:string .


###  http://performedmusicontology.org/ontology/hasEventName
:hasEventName rdf:type owl:ObjectProperty ;
              rdfs:domain <http://id.loc.gov/ontologies/bibframe/Event> ;
              rdfs:range :EventName ;
              rdfs:label "Has event name"^^xsd:string ;
              skos:definition "Relates an event to a name or title for the event."^^xsd:string .


###  http://performedmusicontology.org/ontology/hasInspiration
:hasInspiration rdf:type owl:ObjectProperty ;
                rdfs:subPropertyOf <http://id.loc.gov/ontologies/bibframe/relatedTo> ;
                owl:inverseOf :inspirationFor ;
                rdfs:domain <http://id.loc.gov/ontologies/bibframe/Work> ;
                rdfs:comment "Suggested use - Work, Event, Agent, Place, Item" ;
                rdfs:label "Inspired by"^^xsd:string ;
                skos:definition "Relates a work to a resource that inspired the creation of the work"^^xsd:string .


###  http://performedmusicontology.org/ontology/hasKeyMode
:hasKeyMode rdf:type owl:ObjectProperty ;
            rdfs:domain <http://id.loc.gov/ontologies/bibframe/Work> ;
            rdfs:range :KeyMode ;
            rdfs:comment "A key and mode may not be present for some works, or a key may be present without a mode. For individual named modes, use hasMode."^^xsd:string ;
            rdfs:label "Has key and mode"^^xsd:string ;
            skos:definition "Relates a work to a key and mode."^^xsd:string .


###  http://performedmusicontology.org/ontology/hasMediumComponent
:hasMediumComponent rdf:type owl:ObjectProperty ;
                    rdfs:domain <http://id.loc.gov/ontologies/bibframe/Work> ;
                    rdfs:range :MediumComponent ;
                    rdfs:label "has Medium component"^^xsd:string ;
                    skos:definition "Relates a work to a medium component."^^xsd:string .


###  http://performedmusicontology.org/ontology/hasMediumComponentQualifier
:hasMediumComponentQualifier rdf:type owl:ObjectProperty ;
                             rdfs:domain :MediumComponent ;
                             rdfs:range :MediumComponentQualifier ;
                             rdfs:label "Has medium component qualifier"^^xsd:string ;
                             skos:definition "Relates a medium component to a medium component qualifier that affects the medium component."^^xsd:string .


###  http://performedmusicontology.org/ontology/hasMediumOfPerformance
:hasMediumOfPerformance rdf:type owl:ObjectProperty ;
                        rdfs:domain :MediumComponent ;
                        rdfs:label "Has medium of performance"^^xsd:string ;
                        skos:definition "Relates a work to a medium of performance."^^xsd:string .


###  http://performedmusicontology.org/ontology/hasMode
:hasMode rdf:type owl:ObjectProperty ;
         rdfs:domain <http://id.loc.gov/ontologies/bibframe/Work> ;
         rdfs:range :Mode ;
         rdfs:label "Has mode"^^xsd:string ;
         skos:definition "Relates a work to a mode."^^xsd:string .


###  http://performedmusicontology.org/ontology/hasPerformance
:hasPerformance rdf:type owl:ObjectProperty ;
                rdfs:subPropertyOf <http://id.loc.gov/ontologies/bibframe/eventContentOf> ;
                owl:inverseOf :performanceOf ;
                rdfs:domain <http://id.loc.gov/ontologies/bibframe/Work> ;
                rdfs:range <http://id.loc.gov/ontologies/bibframe/Event> ;
                rdfs:label "Has performance"^^xsd:string ;
                skos:definition "Relates a work to an event that is a performance."^^xsd:string .


###  http://performedmusicontology.org/ontology/hasRecording
:hasRecording rdf:type owl:ObjectProperty ;
              rdfs:subPropertyOf <http://id.loc.gov/ontologies/bibframe/eventContent> ;
              owl:inverseOf :recordingOf ;
              rdfs:domain <http://id.loc.gov/ontologies/bibframe/Event> ;
              rdfs:range <http://id.loc.gov/ontologies/bibframe/Work> ;
              rdfs:label "Has recording"^^xsd:string ;
              skos:definition "Relates an event to an audio or video work that is created by recording the event."^^xsd:string .


###  http://performedmusicontology.org/ontology/hasTempo
:hasTempo rdf:type owl:ObjectProperty ;
          rdfs:domain <http://id.loc.gov/ontologies/bibframe/Work> ;
          rdfs:range :Tempo ;
          rdfs:label "Has tempo"^^xsd:string ;
          skos:definition "Relates a work to a tempo."^^xsd:string .


###  http://performedmusicontology.org/ontology/inspirationFor
:inspirationFor rdf:type owl:ObjectProperty ;
                rdfs:subPropertyOf <http://id.loc.gov/ontologies/bibframe/relatedTo> ;
                rdfs:domain <http://id.loc.gov/ontologies/bibframe/Event> ;
                rdfs:range <http://id.loc.gov/ontologies/bibframe/Work> ;
                rdfs:label "Inspiration for"^^xsd:string ;
                skos:definition "Relates an event to a work that is inspired by an event."^^xsd:string .


###  http://performedmusicontology.org/ontology/performanceOf
:performanceOf rdf:type owl:ObjectProperty ;
               rdfs:subPropertyOf <http://id.loc.gov/ontologies/bibframe/eventContent> ;
               rdfs:domain <http://id.loc.gov/ontologies/bibframe/Event> ;
               rdfs:range <http://id.loc.gov/ontologies/bibframe/Work> ;
               rdfs:label "Performance of"^^xsd:string ;
               skos:definition "Relates an event to a work that is performed at an event."^^xsd:string .


###  http://performedmusicontology.org/ontology/recordingOf
:recordingOf rdf:type owl:ObjectProperty ;
             rdfs:subPropertyOf <http://id.loc.gov/ontologies/bibframe/eventContentOf> ;
             rdfs:domain <http://id.loc.gov/ontologies/bibframe/Work> ;
             rdfs:range <http://id.loc.gov/ontologies/bibframe/Event> ;
             rdfs:label "Recording of"^^xsd:string ;
             skos:definition "Relates a work to an event that is recorded to create an audio or video work."^^xsd:string .


###  http://performedmusicontology.org/ontology/remixOf
:remixOf rdf:type owl:ObjectProperty ;
         rdfs:subPropertyOf <http://id.loc.gov/ontologies/bibframe/derivativeOf> ;
         rdfs:comment "Suggested use - with Audio" ;
         rdfs:label "Remix of" ;
         skos:definition "Relates an audio work created by substantial editing of the audio of a work to the original work" .


###  http://performedmusicontology.org/ontology/remixedIn
:remixedIn rdf:type owl:ObjectProperty ;
           rdfs:subPropertyOf <http://id.loc.gov/ontologies/bibframe/hasDerivative> ;
           rdfs:label "Remixed in" ;
           skos:definition "Relates an audio work to a work created by the substantial editing of the audio of that work" .


###  http://performedmusicontology.org/ontology/sampledBy
:sampledBy rdf:type owl:ObjectProperty ;
           rdfs:subPropertyOf <http://id.loc.gov/ontologies/bibframe/referencedBy> ;
           owl:inverseOf :samplesFrom ;
           rdfs:label "Sampled by" ;
           skos:definition "Relates an audio work from which audio clips are sampled to the new audio work using those samples.." .


###  http://performedmusicontology.org/ontology/samplesFrom
:samplesFrom rdf:type owl:ObjectProperty ;
             rdfs:subPropertyOf <http://id.loc.gov/ontologies/bibframe/references> ;
             rdfs:label "Samples from" ;
             skos:definition "Relates an audio work that makes use of audio clips (samples) from another work to the work it samples from. The sample may or may not be manipulated in the new work." .


###  http://performedmusicontology.org/ontology/usesMediumOfPerformance
:usesMediumOfPerformance rdf:type owl:ObjectProperty ;
                         rdfs:domain <http://id.loc.gov/ontologies/bibframe/Contribution> ;
                         rdfs:range :MediumOfPerformance ;
                         rdfs:label "Uses medium of performance"^^xsd:string ;
                         skos:definition "Relates a contribution to a medium of performance."^^xsd:string .


#################################################################
#    Data properties
#################################################################

###  http://performedmusicontology.org/ontology/hasMediumCount
:hasMediumCount rdf:type owl:DatatypeProperty ;
                rdfs:domain :MediumComponent ;
                rdfs:label "Has medium count"^^rdfs:Literal ;
                skos:definition "Relates a medium component to the count of that medium component."^^xsd:string .


###  http://performedmusicontology.org/ontology/hasNumberOfHands
:hasNumberOfHands rdf:type owl:DatatypeProperty ;
                  rdfs:domain :MediumComponent ;
                  rdfs:comment "Examples include works in which more than one performer shares an instrument or works in which an atypical number of hand is specified for the instrument."^^xsd:string ;
                  rdfs:label "Number of hands"^^xsd:string ;
                  skos:definition "Relates a medium component to the number of hands required for performance."^^xsd:string .


###  http://performedmusicontology.org/ontology/phonogramCopyrightDate
:phonogramCopyrightDate rdf:type owl:DatatypeProperty ;
                        rdfs:subPropertyOf <http://id.loc.gov/ontologies/bibframe/date> ;
                        rdfs:domain <http://id.loc.gov/ontologies/bibframe/Work> ;
                        rdfs:label "Phonogram copyright date"^^xsd:string ;
                        skos:definition "Relates a work to a phonogram copyright date for a work that is a audio recording."^^xsd:string .


#################################################################
#    Classes
#################################################################

###  http://performedmusicontology.org/ontology/AllMusicId
:AllMusicId rdf:type owl:Class ;
            rdfs:subClassOf <http://id.loc.gov/ontologies/bibframe/Identifier> ;
            rdfs:label "AllMusic ID"^^xsd:string ;
            skos:definition "An identifier from AllMusic"^^xsd:string .


###  http://performedmusicontology.org/ontology/DiscogsId
:DiscogsId rdf:type owl:Class ;
           rdfs:subClassOf <http://id.loc.gov/ontologies/bibframe/Identifier> ;
           rdfs:label "Discogs ID"^^xsd:string ;
           skos:definition "An identifier from Discogs."^^xsd:string .


###  http://performedmusicontology.org/ontology/DramaticRole
:DramaticRole rdf:type owl:Class ;
              rdfs:label "Dramatic role"^^xsd:string ;
              skos:definition "A dramatic role performed by a contributing agent."^^xsd:string ;
              skos:example "Role of \"Carmen\" in the opera Carmen."^^xsd:string .


###  http://performedmusicontology.org/ontology/EnsembleSize
:EnsembleSize rdf:type owl:Class ;
              rdfs:comment "A vocabulary is provided"^^xsd:string ;
              rdfs:label "Ensemble size"^^xsd:string ;
              skos:definition "A designation of the size of an individual ensemble."^^xsd:string ;
              skos:example "trio (3 performers); individual or solo performer; large ensemble"^^xsd:string .


###  http://performedmusicontology.org/ontology/EventName
:EventName rdf:type owl:Class ;
           rdfs:label "Event name"^^xsd:string ;
           skos:definition "A name or title given to an event, whether formally stated or created for metadata purposes."^^xsd:string .


###  http://performedmusicontology.org/ontology/KeyMode
:KeyMode rdf:type owl:Class ;
         rdfs:label "Music key"^^xsd:string ;
         skos:definition "Key and mode, or key only if no mode is present, of a music work."^^xsd:string ;
         skos:example "C major; B-flat minor; D"^^xsd:string .


###  http://performedmusicontology.org/ontology/MediumComponent
:MediumComponent rdf:type owl:Class ;
                 rdfs:comment "A medium component may gather together a medium of performance, medium count, number of hands, and/or medium component qualifier."^^xsd:string ;
                 rdfs:label "Medium component"^^xsd:string ;
                 skos:definition "An individual component of an overall medium of performance of a work."^^xsd:string .


###  http://performedmusicontology.org/ontology/MediumComponentQualifier
:MediumComponentQualifier rdf:type owl:Class ;
                          rdfs:comment "A vocabulary is provided."^^xsd:string ;
                          rdfs:label "Medium component qualifier"^^xsd:string ;
                          skos:definition "A qualifier that affects the medium component."^^xsd:string ;
                          skos:example "offstage, amplified, optional"^^xsd:string .


###  http://performedmusicontology.org/ontology/MediumOfPerformance
:MediumOfPerformance rdf:type owl:Class ;
                     rdfs:label "Medium of performance"^^xsd:string ;
                     skos:definition "An individual instrument, voice, ensemble, or instrumental group (e.g., percussion)."^^xsd:string ;
                     skos:example "guitar; er hu; alto voice; percussion; orchestra"^^xsd:string .


###  http://performedmusicontology.org/ontology/Mode
:Mode rdf:type owl:Class ;
      rdfs:label "Music mode"^^xsd:string ;
      skos:definition "Mode (not associated with a key) of a musical work"^^xsd:string ;
      skos:example "Dorian; Dhaivata"^^xsd:string .


###  http://performedmusicontology.org/ontology/MusicBrainzId
:MusicBrainzId rdf:type owl:Class ;
               rdfs:subClassOf <http://id.loc.gov/ontologies/bibframe/Identifier> ;
               rdfs:label "MusicBrainz ID"^^xsd:string ;
               skos:definition "An identifier from MusicBrainz"^^xsd:string .


###  http://performedmusicontology.org/ontology/OpusNumber
:OpusNumber rdf:type owl:Class ;
            rdfs:subClassOf <http://id.loc.gov/ontologies/bibframe/Identifier> ;
            rdfs:label "Opus number"^^xsd:string ;
            skos:definition "An opus number assigned to a musical work."^^xsd:string ;
            skos:example "Op. 45, no. 1; Op. 135a"^^xsd:string .


###  http://performedmusicontology.org/ontology/RismNumber
:RismNumber rdf:type owl:Class ;
            rdfs:subClassOf <http://id.loc.gov/ontologies/bibframe/Identifier> ;
            rdfs:label "RISM number"^^xsd:string ;
            skos:definition "A number from the Repertoire Internationale des Sources Musicales (RISM) online version."^^xsd:string .


###  http://performedmusicontology.org/ontology/Tempo
:Tempo rdf:type owl:Class ;
       rdfs:label "Tempo"^^xsd:string ;
       skos:definition "The speed or pace of a music work, whether declared (in a score) or performed."^^xsd:string ;
       skos:example "80 quarter notes per minute; 100 bpm; Piano roll speed=120"^^xsd:string .


###  http://performedmusicontology.org/ontology/ThematicCatalogNumber
:ThematicCatalogNumber rdf:type owl:Class ;
                       rdfs:subClassOf <http://id.loc.gov/ontologies/bibframe/Identifier> ;
                       rdfs:label "Thematic catalog number"^^xsd:string ;
                       skos:definition "A numeric or alphanumeric designation of a musical work as found in a thematic index or catalog."^^xsd:string ;
                       skos:example "BWV 485; TWV 52:d1"^^xsd:string .


###  http://performedmusicontology.org/ontology/VideogamePlatformIdentifier
:VideogamePlatformIdentifier rdf:type owl:Class ;
                             rdfs:subClassOf <http://id.loc.gov/ontologies/bibframe/Identifier> ;
                             rdfs:label "Videogame platform identifier"^^xsd:string ;
                             skos:definition "An identifier assigned to a video game platform."^^xsd:string ;
                             skos:example "CUSA 54321 (a PlayStation 4 number)"^^xsd:string .


###  Generated by the OWL API (version 4.5.9.2019-02-01T07:24:44Z) https://github.com/owlcs/owlapi
