@prefix skos: <http://www.w3.org/2004/02/skos/core#> .
@prefix rdfs: <http://www.w3.org/2000/01/rdf-schema#> .
@prefix dc: <http://purl.org/dc/terms/> .
@prefix rdf: <http://www.w3.org/1999/02/22-rdf-syntax-ns#> .

<http://performedmusicontology.org/ontologies/vocabularies/encoding_format/>
  a skos:ConceptScheme ;
  rdfs:label "PMO Encoding Format Vocabulary"@en ;
  dc:title "PMO Encoding Format Vocabulary"@en ;
  skos:definition "The PMO Encoding Format Vocabulary is a controlled vocabulary for stating encoding formats of audio recordings. It was developed for the Performed Music Ontology, but may be used with other ontologies."@en .

<http://performedmusicontology.org/ontologies/vocabularies/encoding_format/Aac>
  a skos:Concept ;
  skos:prefLabel "AAC"@en ;
  skos:altLabel "Advanced Audio Recording format"@en ;
  skos:definition "Advanced Audio Coding format, a proprietary audio coding standard for lossy digital audio compression."@en ;
  skos:inScheme <http://performedmusicontology.org/ontologies/vocabularies/encoding_format/> ;
  skos:changeNote [
    rdf:value "NEW" ;
    dc:date "2018-07-01"
  ] .

<http://performedmusicontology.org/ontologies/vocabularies/encoding_format/Aiff>
  a skos:Concept ;
  skos:prefLabel "AIFF"@en ;
  skos:definition "Standard audio file format used by Apple."@en ;
  skos:inScheme <http://performedmusicontology.org/ontologies/vocabularies/encoding_format/> ;
  skos:changeNote [
    rdf:value "NEW" ;
    dc:date "2018-07-01"
  ] .

<http://performedmusicontology.org/ontologies/vocabularies/encoding_format/Flac>
  a skos:Concept ;
  skos:prefLabel "FLAC"@en ;
  skos:altLabel "Free Lossless Audio Codec"@en ;
  skos:definition "An open audio coding format for lossless compression of digital audio."@en ;
  skos:inScheme <http://performedmusicontology.org/ontologies/vocabularies/encoding_format/> ;
  skos:changeNote [
    rdf:value "NEW" ;
    dc:date "2018-07-01"
  ] .

<http://performedmusicontology.org/ontologies/vocabularies/encoding_format/Mp3>
  a skos:Concept ;
  skos:prefLabel "MP3"@en ;
  skos:definition "MPEG Layer III Audio, an audio encoding format for digital audio."@en ;
  skos:inScheme <http://performedmusicontology.org/ontologies/vocabularies/encoding_format/> ;
  skos:changeNote [
    rdf:value "NEW" ;
    dc:date "2018-07-01"
  ] .