<?xml version="1.0"?>
<rdf:RDF xmlns="http://performedmusicontology.org/ontology/"
     xml:base="http://performedmusicontology.org/ontology/"
     xmlns:rdakit="http://metadataregistry.org/uri/profile/rdakit/"
     xmlns:rdf="http://www.w3.org/1999/02/22-rdf-syntax-ns#"
     xmlns:terms="http://purl.org/dc/terms/"
     xmlns:owl="http://www.w3.org/2002/07/owl#"
     xmlns:xml="http://www.w3.org/XML/1998/namespace"
     xmlns:regap="http://metadataregistry.org/uri/profile/regap/"
     xmlns:xsd="http://www.w3.org/2001/XMLSchema#"
     xmlns:skos="http://www.w3.org/2004/02/skos/core#"
     xmlns:rdfs="http://www.w3.org/2000/01/rdf-schema#"
     xmlns:vann="http://purl.org/vocab/vann/"
     xmlns:dc="http://purl.org/dc/elements/1.1/">
    <owl:Ontology rdf:about="http://performedmusicontology.org/ontology/">
        <owl:versionIRI rdf:resource="http://performedmusicontology.org/ontology/"/>
    </owl:Ontology>
    


    <!-- 
    ///////////////////////////////////////////////////////////////////////////////////////
    //
    // Annotation properties
    //
    ///////////////////////////////////////////////////////////////////////////////////////
     -->

    


    <!-- http://metadataregistry.org/uri/profile/rdakit/toolkitDefinition -->

    <owl:AnnotationProperty rdf:about="http://metadataregistry.org/uri/profile/rdakit/toolkitDefinition"/>
    


    <!-- http://metadataregistry.org/uri/profile/rdakit/toolkitLabel -->

    <owl:AnnotationProperty rdf:about="http://metadataregistry.org/uri/profile/rdakit/toolkitLabel"/>
    


    <!-- http://metadataregistry.org/uri/profile/regap/identifier -->

    <owl:AnnotationProperty rdf:about="http://metadataregistry.org/uri/profile/regap/identifier"/>
    


    <!-- http://purl.org/dc/elements/1.1/title -->

    <owl:AnnotationProperty rdf:about="http://purl.org/dc/elements/1.1/title"/>
    


    <!-- http://www.w3.org/2004/02/skos/core#altLabel -->

    <owl:AnnotationProperty rdf:about="http://www.w3.org/2004/02/skos/core#altLabel"/>
    


    <!-- http://www.w3.org/2004/02/skos/core#broader -->

    <owl:AnnotationProperty rdf:about="http://www.w3.org/2004/02/skos/core#broader"/>
    


    <!-- http://www.w3.org/2004/02/skos/core#definition -->

    <owl:AnnotationProperty rdf:about="http://www.w3.org/2004/02/skos/core#definition"/>
    


    <!-- http://www.w3.org/2004/02/skos/core#inScheme -->

    <owl:AnnotationProperty rdf:about="http://www.w3.org/2004/02/skos/core#inScheme"/>
    


    <!-- http://www.w3.org/2004/02/skos/core#narrower -->

    <owl:AnnotationProperty rdf:about="http://www.w3.org/2004/02/skos/core#narrower"/>
    


    <!-- http://www.w3.org/2004/02/skos/core#prefLabel -->

    <owl:AnnotationProperty rdf:about="http://www.w3.org/2004/02/skos/core#prefLabel"/>
    


    <!-- http://www.w3.org/2004/02/skos/core#scopeNote -->

    <owl:AnnotationProperty rdf:about="http://www.w3.org/2004/02/skos/core#scopeNote"/>
    


    <!-- 
    ///////////////////////////////////////////////////////////////////////////////////////
    //
    // Object Properties
    //
    ///////////////////////////////////////////////////////////////////////////////////////
     -->

    


    <!-- http://id.loc.gov/ontologies/bibframe/eventContent -->

    <owl:ObjectProperty rdf:about="http://id.loc.gov/ontologies/bibframe/eventContent"/>
    


    <!-- http://id.loc.gov/ontologies/bibframe/eventContentOf -->

    <owl:ObjectProperty rdf:about="http://id.loc.gov/ontologies/bibframe/eventContentOf"/>
    


    <!-- http://id.loc.gov/ontologies/bibframe/relatedTo -->

    <owl:ObjectProperty rdf:about="http://id.loc.gov/ontologies/bibframe/relatedTo"/>
    


    <!-- http://performedmusicontology.org/ontology/asMemberOf -->

    <owl:ObjectProperty rdf:about="http://performedmusicontology.org/ontology/asMemberOf">
        <rdfs:domain rdf:resource="http://id.loc.gov/ontologies/bibframe/Contribution"/>
        <rdfs:range rdf:resource="http://id.loc.gov/ontologies/bibframe/Organization"/>
        <rdfs:label>as Member of</rdfs:label>
        <skos:definition>Organization through which a person makes a contribution to a work or instance.</skos:definition>
    </owl:ObjectProperty>
    


    <!-- http://performedmusicontology.org/ontology/associatedWith -->

    <owl:ObjectProperty rdf:about="http://performedmusicontology.org/ontology/associatedWith">
        <rdfs:subPropertyOf rdf:resource="http://id.loc.gov/ontologies/bibframe/relatedTo"/>
        <rdf:type rdf:resource="http://www.w3.org/2002/07/owl#SymmetricProperty"/>
        <rdfs:label>associated with</rdfs:label>
        <skos:definition>Event or Work that is associated in a general way with another event or work, instance or item, e.g., the Bible used at a presidential inauguration.</skos:definition>
    </owl:ObjectProperty>
    


    <!-- http://performedmusicontology.org/ontology/composedOf -->

    <owl:ObjectProperty rdf:about="http://performedmusicontology.org/ontology/composedOf">
        <rdfs:label>composed of</rdfs:label>
        <skos:definition>Portion of a multi-level identifier, such as a prefix, e.g., BWV of BWV 464, or a hierarchical number, e.g., 2, of op. 45, no. 2.</skos:definition>
    </owl:ObjectProperty>
    


    <!-- http://performedmusicontology.org/ontology/createdFor -->

    <owl:ObjectProperty rdf:about="http://performedmusicontology.org/ontology/createdFor">
        <rdfs:subPropertyOf rdf:resource="http://id.loc.gov/ontologies/bibframe/relatedTo"/>
        <rdfs:domain rdf:resource="http://id.loc.gov/ontologies/bibframe/Work"/>
        <rdfs:range rdf:resource="http://id.loc.gov/ontologies/bibframe/Event"/>
        <rdfs:label>created for</rdfs:label>
        <skos:definition>Event a work is created for, e.g., a motet celebrating the inauguration of a pope.</skos:definition>
    </owl:ObjectProperty>
    


    <!-- http://performedmusicontology.org/ontology/hasCompiledWork -->

    <owl:ObjectProperty rdf:about="http://performedmusicontology.org/ontology/hasCompiledWork">
        <rdfs:domain rdf:resource="http://id.loc.gov/ontologies/bibframe/Work"/>
        <rdfs:range rdf:resource="http://id.loc.gov/ontologies/bibframe/Work"/>
        <rdfs:label>has Compiled Work</rdfs:label>
        <skos:definition>Property connecting a bf:Work or its subclasses to a bf:Work that is exactly the same except that it is in an instance of a compilation.</skos:definition>
    </owl:ObjectProperty>
    


    <!-- http://performedmusicontology.org/ontology/hasDoublingMediumOfPerformance -->

    <owl:ObjectProperty rdf:about="http://performedmusicontology.org/ontology/hasDoublingMediumOfPerformance">
        <rdfs:range rdf:resource="http://performedmusicontology.org/ontology/MediumOfPerformance"/>
        <rdfs:label>has Doubling Medium of Performance</rdfs:label>
        <skos:definition>2 (or more) mediums of performance intended to be performed alternately by a single performer</skos:definition>
    </owl:ObjectProperty>
    


    <!-- http://performedmusicontology.org/ontology/hasDramaticRole -->

    <owl:ObjectProperty rdf:about="http://performedmusicontology.org/ontology/hasDramaticRole">
        <rdfs:range rdf:resource="http://performedmusicontology.org/ontology/DramaticRole"/>
        <rdfs:label>has Dramatic Role</rdfs:label>
        <skos:definition>Property connecting a bf:Contribution to the character of a performer in a dramatic work (e.g., an opera, play, video), e.g., &quot;Carmen&quot; in the opera or video &quot;Carmen&quot;.</skos:definition>
    </owl:ObjectProperty>
    


    <!-- http://performedmusicontology.org/ontology/hasEventName -->

    <owl:ObjectProperty rdf:about="http://performedmusicontology.org/ontology/hasEventName">
        <rdfs:subPropertyOf rdf:resource="http://www.w3.org/2002/07/owl#topObjectProperty"/>
        <rdfs:domain rdf:resource="http://id.loc.gov/ontologies/bibframe/Event"/>
        <rdfs:label>has Event Name</rdfs:label>
        <skos:definition>Name of an event, whether formal or created for metadata purposes</skos:definition>
    </owl:ObjectProperty>
    


    <!-- http://performedmusicontology.org/ontology/hasInspiration -->

    <owl:ObjectProperty rdf:about="http://performedmusicontology.org/ontology/hasInspiration">
        <rdfs:subPropertyOf rdf:resource="http://id.loc.gov/ontologies/bibframe/relatedTo"/>
        <owl:inverseOf rdf:resource="http://performedmusicontology.org/ontology/inspirationFor"/>
        <rdfs:label>has as Inspiration</rdfs:label>
        <skos:definition>Event that inspired the creation of a work.</skos:definition>
    </owl:ObjectProperty>
    


    <!-- http://performedmusicontology.org/ontology/hasKeyMode -->

    <owl:ObjectProperty rdf:about="http://performedmusicontology.org/ontology/hasKeyMode">
        <rdfs:range rdf:resource="http://performedmusicontology.org/ontology/KeyMode"/>
        <rdfs:label>has Key and Mode</rdfs:label>
        <skos:definition>Property linking Work to KeyMode.</skos:definition>
    </owl:ObjectProperty>
    


    <!-- http://performedmusicontology.org/ontology/hasMedium -->

    <owl:ObjectProperty rdf:about="http://performedmusicontology.org/ontology/hasMedium">
        <rdfs:domain rdf:resource="http://id.loc.gov/ontologies/bibframe/Work"/>
        <rdfs:label>has Medium</rdfs:label>
        <skos:definition>Property that links a Work or Performance to the declared or performed medium.</skos:definition>
    </owl:ObjectProperty>
    


    <!-- http://performedmusicontology.org/ontology/hasMediumOfPerformance -->

    <owl:ObjectProperty rdf:about="http://performedmusicontology.org/ontology/hasMediumOfPerformance">
        <rdfs:range rdf:resource="http://performedmusicontology.org/ontology/MediumOfPerformance"/>
        <rdfs:label>has Medium Of Performance</rdfs:label>
        <skos:definition>Specific medium of performance, e.g., bass guitar.</skos:definition>
    </owl:ObjectProperty>
    


    <!-- http://performedmusicontology.org/ontology/hasMediumPart -->

    <owl:ObjectProperty rdf:about="http://performedmusicontology.org/ontology/hasMediumPart">
        <rdfs:range rdf:resource="http://performedmusicontology.org/ontology/MediumPart"/>
        <rdfs:label>has Medium Part</rdfs:label>
        <skos:definition>Specific element within an overall declared or performed medium, e.g., er hu, mixed chorus.</skos:definition>
    </owl:ObjectProperty>
    


    <!-- http://performedmusicontology.org/ontology/hasMediumPartType -->

    <owl:ObjectProperty rdf:about="http://performedmusicontology.org/ontology/hasMediumPartType">
        <rdfs:subPropertyOf rdf:resource="http://www.w3.org/2002/07/owl#topObjectProperty"/>
        <rdfs:domain rdf:resource="http://performedmusicontology.org/ontology/MediumPart"/>
        <rdfs:range rdf:resource="http://performedmusicontology.org/ontology/MediumPartType"/>
        <rdfs:label>has Medium Part Type</rdfs:label>
        <skos:definition>Property that links a a pmo:MediumPart to a specific role or type of part, e.g., solo, ad lib, optional, offstage, amplified.</skos:definition>
    </owl:ObjectProperty>
    


    <!-- http://performedmusicontology.org/ontology/hasMode -->

    <owl:ObjectProperty rdf:about="http://performedmusicontology.org/ontology/hasMode">
        <rdfs:range rdf:resource="http://performedmusicontology.org/ontology/Mode"/>
        <rdfs:label>has Mode</rdfs:label>
        <skos:definition>Property linking Work to Mode.</skos:definition>
    </owl:ObjectProperty>
    


    <!-- http://performedmusicontology.org/ontology/hasMusicPart -->

    <owl:ObjectProperty rdf:about="http://performedmusicontology.org/ontology/hasMusicPart">
        <rdfs:range rdf:resource="http://performedmusicontology.org/ontology/MusicPart"/>
        <rdfs:label>has Music Part</rdfs:label>
        <skos:definition>Property linking MediumPart or bf:Contribution to the specific music parts within a single medium part e.g., Violin 1, Clarinet 2.</skos:definition>
    </owl:ObjectProperty>
    


    <!-- http://performedmusicontology.org/ontology/hasPerformance -->

    <owl:ObjectProperty rdf:about="http://performedmusicontology.org/ontology/hasPerformance">
        <rdfs:subPropertyOf rdf:resource="http://id.loc.gov/ontologies/bibframe/eventContentOf"/>
        <owl:inverseOf rdf:resource="http://performedmusicontology.org/ontology/performanceOf"/>
        <rdfs:domain rdf:resource="http://id.loc.gov/ontologies/bibframe/Work"/>
        <rdfs:range rdf:resource="http://performedmusicontology.org/ontology/Performance"/>
        <rdfs:label>has Performance</rdfs:label>
        <skos:definition>Event that is a performance of a work</skos:definition>
    </owl:ObjectProperty>
    


    <!-- http://performedmusicontology.org/ontology/hasRecording -->

    <owl:ObjectProperty rdf:about="http://performedmusicontology.org/ontology/hasRecording">
        <rdfs:subPropertyOf rdf:resource="http://id.loc.gov/ontologies/bibframe/eventContent"/>
        <owl:inverseOf rdf:resource="http://performedmusicontology.org/ontology/recordingOf"/>
        <rdfs:domain rdf:resource="http://id.loc.gov/ontologies/bibframe/Event"/>
        <rdfs:range rdf:resource="http://id.loc.gov/ontologies/bibframe/Work"/>
        <rdfs:label>has Recording</rdfs:label>
        <skos:definition>Audio or video work created from the recording of event content.</skos:definition>
    </owl:ObjectProperty>
    


    <!-- http://performedmusicontology.org/ontology/hasTempo -->

    <owl:ObjectProperty rdf:about="http://performedmusicontology.org/ontology/hasTempo">
        <rdfs:range rdf:resource="http://performedmusicontology.org/ontology/Tempo"/>
        <rdfs:label>has Tempo</rdfs:label>
    </owl:ObjectProperty>
    


    <!-- http://performedmusicontology.org/ontology/hasTonalCenter -->

    <owl:ObjectProperty rdf:about="http://performedmusicontology.org/ontology/hasTonalCenter">
        <rdfs:range rdf:resource="http://performedmusicontology.org/ontology/TonalCenter"/>
        <rdfs:label>has Tonal Center</rdfs:label>
        <skos:definition>Property linking Work to Tonal Center</skos:definition>
    </owl:ObjectProperty>
    


    <!-- http://performedmusicontology.org/ontology/inspirationFor -->

    <owl:ObjectProperty rdf:about="http://performedmusicontology.org/ontology/inspirationFor">
        <rdfs:subPropertyOf rdf:resource="http://id.loc.gov/ontologies/bibframe/relatedTo"/>
        <rdfs:label>Inspiration for</rdfs:label>
        <skos:definition>Work that is inspired by an event.</skos:definition>
    </owl:ObjectProperty>
    


    <!-- http://performedmusicontology.org/ontology/performanceOf -->

    <owl:ObjectProperty rdf:about="http://performedmusicontology.org/ontology/performanceOf">
        <rdfs:subPropertyOf rdf:resource="http://id.loc.gov/ontologies/bibframe/eventContent"/>
        <rdfs:domain rdf:resource="http://performedmusicontology.org/ontology/Performance"/>
        <rdfs:range rdf:resource="http://id.loc.gov/ontologies/bibframe/Work"/>
        <rdfs:label>Performance of</rdfs:label>
        <skos:definition>Work that is realized through a performance.</skos:definition>
    </owl:ObjectProperty>
    


    <!-- http://performedmusicontology.org/ontology/recordingOf -->

    <owl:ObjectProperty rdf:about="http://performedmusicontology.org/ontology/recordingOf">
        <rdfs:subPropertyOf rdf:resource="http://id.loc.gov/ontologies/bibframe/eventContentOf"/>
        <rdfs:domain rdf:resource="http://id.loc.gov/ontologies/bibframe/Work"/>
        <rdfs:range rdf:resource="http://id.loc.gov/ontologies/bibframe/Event"/>
        <rdfs:label>Recording of</rdfs:label>
        <skos:definition>Event content of an audio or video work.</skos:definition>
    </owl:ObjectProperty>
    


    <!-- 
    ///////////////////////////////////////////////////////////////////////////////////////
    //
    // Data properties
    //
    ///////////////////////////////////////////////////////////////////////////////////////
     -->

    


    <!-- http://id.loc.gov/ontologies/bibframe/date -->

    <owl:DatatypeProperty rdf:about="http://id.loc.gov/ontologies/bibframe/date"/>
    


    <!-- http://performedmusicontology.org/ontology/hasDistinctPartCount -->

    <owl:DatatypeProperty rdf:about="http://performedmusicontology.org/ontology/hasDistinctPartCount">
        <rdfs:comment>has Distinct Part Count</rdfs:comment>
        <skos:definition>Number of distinct music parts in a performed or declared medium, or medium part that is not a named ensemble, e.g, a performed work for 2 flutes and bassoon has a count of “3”.</skos:definition>
    </owl:DatatypeProperty>
    


    <!-- http://performedmusicontology.org/ontology/hasEnsembleCount -->

    <owl:DatatypeProperty rdf:about="http://performedmusicontology.org/ontology/hasEnsembleCount">
        <rdfs:comment>has Ensemble Count</rdfs:comment>
        <skos:definition>Number of named ensembles in a specified declared or performed medium, e.g., a string quartet has a count of “1”; a jazz combo has a count of “1”; a work for 2 choruses and orchestra has a count of “3”.</skos:definition>
    </owl:DatatypeProperty>
    


    <!-- http://performedmusicontology.org/ontology/hasNumberOfHands -->

    <owl:DatatypeProperty rdf:about="http://performedmusicontology.org/ontology/hasNumberOfHands">
        <rdfs:comment>has Number of Hands</rdfs:comment>
        <skos:definition>Number of hands required for performance in works where more than one performer shares an instrument (e.g., piano, 4 hands) or where an atypical number of hands is specified (e.g., viola, 1 hand).</skos:definition>
    </owl:DatatypeProperty>
    


    <!-- http://performedmusicontology.org/ontology/hasOrder -->

    <owl:DatatypeProperty rdf:about="http://performedmusicontology.org/ontology/hasOrder">
        <rdfs:comment>Order a compiled work has in a compilation.</rdfs:comment>
    </owl:DatatypeProperty>
    


    <!-- http://performedmusicontology.org/ontology/hasPerformerCount -->

    <owl:DatatypeProperty rdf:about="http://performedmusicontology.org/ontology/hasPerformerCount">
        <rdfs:comment>has Performer Count</rdfs:comment>
        <skos:definition>Actual number of performers participating in a performed music event or work, e.g., a quartet for 4 serpents, performed by 8 bassoons, has a count of &quot;8&quot;.</skos:definition>
    </owl:DatatypeProperty>
    


    <!-- http://performedmusicontology.org/ontology/hasRequiredPerformerCount -->

    <owl:DatatypeProperty rdf:about="http://performedmusicontology.org/ontology/hasRequiredPerformerCount">
        <rdfs:comment>has Suggested Performer Count</rdfs:comment>
        <skos:definition>Minimum or suggested number of performers required to perform a declared medium, e.g., a work for a percussion ensemble for 3 performers has a a count of “3”.</skos:definition>
    </owl:DatatypeProperty>
    


    <!-- http://performedmusicontology.org/ontology/hasTrackNumber -->

    <owl:DatatypeProperty rdf:about="http://performedmusicontology.org/ontology/hasTrackNumber">
        <rdfs:comment>Track number(s) of a compiled audio work on a sound recording.</rdfs:comment>
    </owl:DatatypeProperty>
    


    <!-- http://performedmusicontology.org/ontology/phonogramCopyrightDate -->

    <owl:DatatypeProperty rdf:about="http://performedmusicontology.org/ontology/phonogramCopyrightDate">
        <rdfs:subPropertyOf rdf:resource="http://id.loc.gov/ontologies/bibframe/date"/>
        <rdfs:comment>Phonogram Copyright Date</rdfs:comment>
        <skos:definition>Phonogram copyright date for a sound recording. Indicated by a &quot;p&quot; or a &quot;p&quot; in a circle.</skos:definition>
    </owl:DatatypeProperty>
    


    <!-- 
    ///////////////////////////////////////////////////////////////////////////////////////
    //
    // Classes
    //
    ///////////////////////////////////////////////////////////////////////////////////////
     -->

    


    <!-- http://erlangen-crm.org/efrbroo/F31_Performance -->

    <owl:Class rdf:about="http://erlangen-crm.org/efrbroo/F31_Performance"/>
    


    <!-- http://id.loc.gov/ontologies/bibframe/Carrier -->

    <owl:Class rdf:about="http://id.loc.gov/ontologies/bibframe/Carrier"/>
    


    <!-- http://id.loc.gov/ontologies/bibframe/Contribution -->

    <owl:Class rdf:about="http://id.loc.gov/ontologies/bibframe/Contribution"/>
    


    <!-- http://id.loc.gov/ontologies/bibframe/EncodingFormat -->

    <owl:Class rdf:about="http://id.loc.gov/ontologies/bibframe/EncodingFormat"/>
    


    <!-- http://id.loc.gov/ontologies/bibframe/Event -->

    <owl:Class rdf:about="http://id.loc.gov/ontologies/bibframe/Event"/>
    


    <!-- http://id.loc.gov/ontologies/bibframe/Identifier -->

    <owl:Class rdf:about="http://id.loc.gov/ontologies/bibframe/Identifier"/>
    


    <!-- http://id.loc.gov/ontologies/bibframe/Organization -->

    <owl:Class rdf:about="http://id.loc.gov/ontologies/bibframe/Organization"/>
    


    <!-- http://id.loc.gov/ontologies/bibframe/PlayingSpeed -->

    <owl:Class rdf:about="http://id.loc.gov/ontologies/bibframe/PlayingSpeed"/>
    


    <!-- http://id.loc.gov/ontologies/bibframe/SoundCharacteristic -->

    <owl:Class rdf:about="http://id.loc.gov/ontologies/bibframe/SoundCharacteristic"/>
    


    <!-- http://id.loc.gov/ontologies/bibframe/TapeConfig -->

    <owl:Class rdf:about="http://id.loc.gov/ontologies/bibframe/TapeConfig"/>
    


    <!-- http://id.loc.gov/ontologies/bibframe/Work -->

    <owl:Class rdf:about="http://id.loc.gov/ontologies/bibframe/Work"/>
    


    <!-- http://performedmusicontology.org/ontology/Audition -->

    <owl:Class rdf:about="http://performedmusicontology.org/ontology/Audition">
        <rdfs:subClassOf rdf:resource="http://id.loc.gov/ontologies/bibframe/Event"/>
        <skos:definition>Event in which a performer or actor is applying for a position in an ensemble, cast, film, etc.</skos:definition>
    </owl:Class>
    


    <!-- http://performedmusicontology.org/ontology/BenefitConcert -->

    <owl:Class rdf:about="http://performedmusicontology.org/ontology/BenefitConcert">
        <rdfs:subClassOf rdf:resource="http://performedmusicontology.org/ontology/Concert"/>
        <skos:definition>Concert held for charitable purposes, i.e., to raise funds or awareness</skos:definition>
    </owl:Class>
    


    <!-- http://performedmusicontology.org/ontology/Ceremony -->

    <owl:Class rdf:about="http://performedmusicontology.org/ontology/Ceremony">
        <rdfs:subClassOf rdf:resource="http://id.loc.gov/ontologies/bibframe/Event"/>
        <skos:definition>Ritual event, performed on special occasions (e.g., death, baptism, wedding, graduation, equinox, coronation, victory)</skos:definition>
    </owl:Class>
    


    <!-- http://performedmusicontology.org/ontology/CommandPerformance -->

    <owl:Class rdf:about="http://performedmusicontology.org/ontology/CommandPerformance">
        <rdfs:subClassOf rdf:resource="http://performedmusicontology.org/ontology/Concert"/>
        <skos:definition>Performance done at the request of a monarch or other head of state.</skos:definition>
    </owl:Class>
    


    <!-- http://performedmusicontology.org/ontology/Concert -->

    <owl:Class rdf:about="http://performedmusicontology.org/ontology/Concert">
        <rdfs:subClassOf rdf:resource="http://id.loc.gov/ontologies/bibframe/Event"/>
        <skos:definition>Live musical performance of one or more works in front of an audience</skos:definition>
    </owl:Class>
    


    <!-- http://performedmusicontology.org/ontology/ConcertSeries -->

    <owl:Class rdf:about="http://performedmusicontology.org/ontology/ConcertSeries">
        <rdfs:subClassOf rdf:resource="http://id.loc.gov/ontologies/bibframe/Event"/>
        <skos:definition>Group of concerts in the same geographic area by a single performer or brought together by a common theme, usually available for sale as a package. e.g., an orchestra concert season, a series featuring chamber ensembles.</skos:definition>
    </owl:Class>
    


    <!-- http://performedmusicontology.org/ontology/ConcertTour -->

    <owl:Class rdf:about="http://performedmusicontology.org/ontology/ConcertTour">
        <rdfs:subClassOf rdf:resource="http://id.loc.gov/ontologies/bibframe/Event"/>
        <skos:definition>Series of concerts by a performer or group of performers in different cities, countries, or locations.</skos:definition>
    </owl:Class>
    


    <!-- http://performedmusicontology.org/ontology/DeclaredMedium -->

    <owl:Class rdf:about="http://performedmusicontology.org/ontology/DeclaredMedium">
        <rdfs:label>Declared medium</rdfs:label>
        <skos:definition>Intended overall medium of performance of a musical work, as declared by the composer, a reference source, or other source.</skos:definition>
    </owl:Class>
    


    <!-- http://performedmusicontology.org/ontology/DiscCutting -->

    <owl:Class rdf:about="http://performedmusicontology.org/ontology/DiscCutting">
        <rdfs:subClassOf rdf:resource="http://id.loc.gov/ontologies/bibframe/SoundCharacteristic"/>
        <rdfs:label>Disc cutting process</rdfs:label>
        <skos:definition>Recording process in which a stylus cuts a vertical or lateral groove into an audio disc.</skos:definition>
    </owl:Class>
    


    <!-- http://performedmusicontology.org/ontology/Discogs -->

    <owl:Class rdf:about="http://performedmusicontology.org/ontology/Discogs">
        <rdfs:subClassOf rdf:resource="http://id.loc.gov/ontologies/bibframe/Identifier"/>
        <rdfs:label>Discogs ID</rdfs:label>
        <skos:definition>Identifier from Discogs.</skos:definition>
    </owl:Class>
    


    <!-- http://performedmusicontology.org/ontology/DramaticRole -->

    <owl:Class rdf:about="http://performedmusicontology.org/ontology/DramaticRole">
        <rdfs:label>Dramatic role</rdfs:label>
        <skos:definition>Character of a performer in a dramatic work (e.g., an opera, play, video), e.g., &quot;Carmen&quot; in the opera or video &quot;Carmen&quot;.</skos:definition>
    </owl:Class>
    


    <!-- http://performedmusicontology.org/ontology/EnsembleMediumOfPerformance -->

    <owl:Class rdf:about="http://performedmusicontology.org/ontology/EnsembleMediumOfPerformance">
        <rdfs:subClassOf rdf:resource="http://performedmusicontology.org/ontology/MediumOfPerformance"/>
        <skos:definition>Named group of like or unlike mediums of performance intended to be played by multiple performers, e.g., orchestra, jazz combo, string quartet, percussion ensemble.</skos:definition>
    </owl:Class>
    


    <!-- http://performedmusicontology.org/ontology/EventName -->

    <owl:Class rdf:about="http://performedmusicontology.org/ontology/EventName">
        <rdfs:label>Event name</rdfs:label>
        <skos:definition>Name given to an event.</skos:definition>
    </owl:Class>
    


    <!-- http://performedmusicontology.org/ontology/FirstPerformance -->

    <owl:Class rdf:about="http://performedmusicontology.org/ontology/FirstPerformance">
        <rdfs:subClassOf rdf:resource="http://performedmusicontology.org/ontology/Performance"/>
        <skos:definition>The world premiere performance of a work.</skos:definition>
    </owl:Class>
    


    <!-- http://performedmusicontology.org/ontology/IndividualMediumOfPerformance -->

    <owl:Class rdf:about="http://performedmusicontology.org/ontology/IndividualMediumOfPerformance">
        <rdfs:subClassOf rdf:resource="http://performedmusicontology.org/ontology/MediumOfPerformance"/>
        <rdfs:comment>Individual musical instrument, voice, or other object used as a medium of performance (e.g., flute, keyboards, pi pa, drinking glass, typewriter).</rdfs:comment>
    </owl:Class>
    


    <!-- http://performedmusicontology.org/ontology/KeyMode -->

    <owl:Class rdf:about="http://performedmusicontology.org/ontology/KeyMode">
        <rdfs:label>Music key and mode</rdfs:label>
        <skos:definition>Key and mode of a music work when used in combination, e.g., C major, B-flat major.</skos:definition>
    </owl:Class>
    


    <!-- http://performedmusicontology.org/ontology/LivePerformance -->

    <owl:Class rdf:about="http://performedmusicontology.org/ontology/LivePerformance">
        <rdfs:subClassOf rdf:resource="http://performedmusicontology.org/ontology/Performance"/>
        <skos:definition>Performance that is recorded at a concert.</skos:definition>
    </owl:Class>
    


    <!-- http://performedmusicontology.org/ontology/MasterClass -->

    <owl:Class rdf:about="http://performedmusicontology.org/ontology/MasterClass">
        <rdfs:subClassOf rdf:resource="http://id.loc.gov/ontologies/bibframe/Event"/>
        <skos:definition>Event in which a recognized performer critiques the performances of one or more other performers.</skos:definition>
    </owl:Class>
    


    <!-- http://performedmusicontology.org/ontology/MediumOfPerformance -->

    <owl:Class rdf:about="http://performedmusicontology.org/ontology/MediumOfPerformance">
        <rdfs:label>Medium of performance</rdfs:label>
        <skos:definition>Instruments, voices, ensembles, choruses, and other participants (actors, dancers, etc.) required for, or performing in, an event or work, including electronics, computers, installations, etc.</skos:definition>
    </owl:Class>
    


    <!-- http://performedmusicontology.org/ontology/MediumPart -->

    <owl:Class rdf:about="http://performedmusicontology.org/ontology/MediumPart">
        <rdfs:comment>Use with DeclaredMedium, PerformedMedium</rdfs:comment>
        <rdfs:label>Medium part</rdfs:label>
        <skos:definition>Medium of performance, type, etc., of a specific part of the declared or performed medium.</skos:definition>
    </owl:Class>
    


    <!-- http://performedmusicontology.org/ontology/MediumPartType -->

    <owl:Class rdf:about="http://performedmusicontology.org/ontology/MediumPartType">
        <rdfs:label>Part type</rdfs:label>
        <skos:definition>Specific role or type of a medium part, e.g., solo, ad lib, optional, offstage, amplified</skos:definition>
    </owl:Class>
    


    <!-- http://performedmusicontology.org/ontology/Mode -->

    <owl:Class rdf:about="http://performedmusicontology.org/ontology/Mode">
        <rdfs:label>Music mode</rdfs:label>
        <skos:definition>Musical mode of a music work, e.g., Dorian, Dhaivata.</skos:definition>
    </owl:Class>
    


    <!-- http://performedmusicontology.org/ontology/MusicBrainz -->

    <owl:Class rdf:about="http://performedmusicontology.org/ontology/MusicBrainz">
        <rdfs:subClassOf rdf:resource="http://id.loc.gov/ontologies/bibframe/Identifier"/>
        <rdfs:label>MusicBrainz ID</rdfs:label>
        <skos:definition>Identifier from MusicBrainz</skos:definition>
    </owl:Class>
    


    <!-- http://performedmusicontology.org/ontology/MusicPart -->

    <owl:Class rdf:about="http://performedmusicontology.org/ontology/MusicPart">
        <rdfs:label>Music part</rdfs:label>
        <skos:definition>Specific element within an overall declared or performed medium, e.g., Violin 1, Trumpet 2.</skos:definition>
    </owl:Class>
    


    <!-- http://performedmusicontology.org/ontology/OpenMicPerformance -->

    <owl:Class rdf:about="http://performedmusicontology.org/ontology/OpenMicPerformance">
        <rdfs:subClassOf rdf:resource="http://performedmusicontology.org/ontology/Performance"/>
        <skos:definition>Live performance at a coffee house, night club, or other venue by amateur performers.</skos:definition>
    </owl:Class>
    


    <!-- http://performedmusicontology.org/ontology/OpusNumber -->

    <owl:Class rdf:about="http://performedmusicontology.org/ontology/OpusNumber">
        <rdfs:subClassOf rdf:resource="http://id.loc.gov/ontologies/bibframe/Identifier"/>
        <rdfs:label>Opus number</rdfs:label>
        <skos:definition>Opus number for a   musical work, e.g. “45” of Op. 45. No. 1</skos:definition>
    </owl:Class>
    


    <!-- http://performedmusicontology.org/ontology/OpusNumberPart -->

    <owl:Class rdf:about="http://performedmusicontology.org/ontology/OpusNumberPart">
        <rdfs:subClassOf rdf:resource="http://id.loc.gov/ontologies/bibframe/Identifier"/>
        <rdfs:label>Opus number part</rdfs:label>
        <skos:definition>Number for a   portion of an opus number, e.g., no. 1   of Op. 45, no. 1.</skos:definition>
    </owl:Class>
    


    <!-- http://performedmusicontology.org/ontology/OpusNumberStatement -->

    <owl:Class rdf:about="http://performedmusicontology.org/ontology/OpusNumberStatement">
        <rdfs:subClassOf rdf:resource="http://id.loc.gov/ontologies/bibframe/Identifier"/>
        <rdfs:label>Opus number statement</rdfs:label>
        <skos:definition>Statement about the opus number for a musical work.</skos:definition>
    </owl:Class>
    


    <!-- http://performedmusicontology.org/ontology/Performance -->

    <owl:Class rdf:about="http://performedmusicontology.org/ontology/Performance">
        <rdfs:subClassOf rdf:resource="http://erlangen-crm.org/efrbroo/F31_Performance"/>
        <rdfs:subClassOf rdf:resource="http://id.loc.gov/ontologies/bibframe/Event"/>
        <skos:definition>Event in which a performer or group of performers present a work to an audience or in a recording studio.</skos:definition>
    </owl:Class>
    


    <!-- http://performedmusicontology.org/ontology/PerformedMedium -->

    <owl:Class rdf:about="http://performedmusicontology.org/ontology/PerformedMedium">
        <rdfs:label>Performed medium</rdfs:label>
        <skos:definition>The overall medium of performance used in the performance of a musical work. This may or may not be the same as the declared medium of performance.</skos:definition>
    </owl:Class>
    


    <!-- http://performedmusicontology.org/ontology/RecordingSession -->

    <owl:Class rdf:about="http://performedmusicontology.org/ontology/RecordingSession">
        <rdfs:subClassOf rdf:resource="http://id.loc.gov/ontologies/bibframe/Event"/>
        <skos:definition>Event in which one or more performances are recorded with the aim of producing a recording for issue.</skos:definition>
    </owl:Class>
    


    <!-- http://performedmusicontology.org/ontology/Rehearsal -->

    <owl:Class rdf:about="http://performedmusicontology.org/ontology/Rehearsal">
        <rdfs:subClassOf rdf:resource="http://id.loc.gov/ontologies/bibframe/Event"/>
        <skos:definition>Event in which a performer or group of performers prepare for a performance in a concert.</skos:definition>
    </owl:Class>
    


    <!-- http://performedmusicontology.org/ontology/RismNumber -->

    <owl:Class rdf:about="http://performedmusicontology.org/ontology/RismNumber">
        <rdfs:subClassOf rdf:resource="http://id.loc.gov/ontologies/bibframe/Identifier"/>
        <rdfs:label>RISM number</rdfs:label>
        <skos:definition>Number from the Repertoire Internationale des Sources Musicales (RISM) online version.</skos:definition>
    </owl:Class>
    


    <!-- http://performedmusicontology.org/ontology/Tempo -->

    <owl:Class rdf:about="http://performedmusicontology.org/ontology/Tempo">
        <rdfs:label>Tempo</rdfs:label>
        <skos:definition>The speed or pace of a music work, whether declared (in a score) or performed.</skos:definition>
    </owl:Class>
    


    <!-- http://performedmusicontology.org/ontology/ThematicCatalogNumber -->

    <owl:Class rdf:about="http://performedmusicontology.org/ontology/ThematicCatalogNumber">
        <rdfs:subClassOf rdf:resource="http://id.loc.gov/ontologies/bibframe/Identifier"/>
        <rdfs:label>Thematic catalog number</rdfs:label>
        <skos:definition>Numeric or alphanumericdesignation of a   musical work as found in a thematic index for the composer.</skos:definition>
    </owl:Class>
    


    <!-- http://performedmusicontology.org/ontology/ThematicCatalogPrefix -->

    <owl:Class rdf:about="http://performedmusicontology.org/ontology/ThematicCatalogPrefix">
        <rdfs:subClassOf rdf:resource="http://id.loc.gov/ontologies/bibframe/Identifier"/>
        <rdfs:label>Thematic catalog prefix</rdfs:label>
        <skos:definition>Prefix assigned to a   thematic catalog number denoting thework from which the number originated, e.g., BWV for Bach, M.S. for Paganini.</skos:definition>
    </owl:Class>
    


    <!-- http://performedmusicontology.org/ontology/ThematicCatalogStatement -->

    <owl:Class rdf:about="http://performedmusicontology.org/ontology/ThematicCatalogStatement">
        <rdfs:subClassOf rdf:resource="http://id.loc.gov/ontologies/bibframe/Identifier"/>
        <rdfs:label>Thematic catalog number statement</rdfs:label>
        <skos:definition>Statement about the thematic catalog number for a musical work.</skos:definition>
    </owl:Class>
    


    <!-- http://performedmusicontology.org/ontology/TonalCenter -->

    <owl:Class rdf:about="http://performedmusicontology.org/ontology/TonalCenter">
        <rdfs:label>Tonal center</rdfs:label>
        <skos:definition>The tonal center of a music work, without mode, e.g., D, C##.</skos:definition>
    </owl:Class>
    


    <!-- http://performedmusicontology.org/ontology/VideogamePlatformIdentifier -->

    <owl:Class rdf:about="http://performedmusicontology.org/ontology/VideogamePlatformIdentifier">
        <rdfs:subClassOf rdf:resource="http://id.loc.gov/ontologies/bibframe/Identifier"/>
        <rdfs:label>Videogame platform identifier</rdfs:label>
        <skos:definition>Identifier assigned to a video game platform, e.g., CUSA 54321 (a PlayStation 4 number).</skos:definition>
    </owl:Class>
    


    <!-- http://performedmusicontology.org/ontology/WorkComponent -->

    <owl:Class rdf:about="http://performedmusicontology.org/ontology/WorkComponent">
        <rdfs:subClassOf rdf:resource="http://id.loc.gov/ontologies/bibframe/Work"/>
        <rdfs:label>Work component</rdfs:label>
        <skos:definition>A work that is an integral part of another work, even when separated from it, e.g., a movement of a symphony, a chapter of a novel.</skos:definition>
    </owl:Class>
    


    <!-- http://www.w3.org/2004/02/skos/core#Concept -->

    <owl:Class rdf:about="http://www.w3.org/2004/02/skos/core#Concept"/>
    


    <!-- http://www.w3.org/2004/02/skos/core#ConceptScheme -->

    <owl:Class rdf:about="http://www.w3.org/2004/02/skos/core#ConceptScheme"/>
    


    <!-- 
    ///////////////////////////////////////////////////////////////////////////////////////
    //
    // Individuals
    //
    ///////////////////////////////////////////////////////////////////////////////////////
     -->

    


    <!-- http://performedmusicontology.org/FPM12 -->

    <owl:NamedIndividual rdf:about="http://performedmusicontology.org/FPM12">
        <rdf:type rdf:resource="http://id.loc.gov/ontologies/bibframe/PlayingSpeed"/>
        <rdfs:comment>Traditional way of describing the speed of audio cylinders.</rdfs:comment>
        <rdfs:label rdf:datatype="http://www.w3.org/2001/XMLSchema#integer">120</rdfs:label>
        <skos:definition>Playing speed of 12 feet per minute x 10.</skos:definition>
    </owl:NamedIndividual>
    


    <!-- http://performedmusicontology.org/Laserdisc -->

    <owl:NamedIndividual rdf:about="http://performedmusicontology.org/Laserdisc">
        <rdf:type rdf:resource="http://id.loc.gov/ontologies/bibframe/Carrier"/>
        <rdfs:label>Laser disc</rdfs:label>
        <skos:broader rdf:resource="http://rdaregistry.info/termList/RDACarrierType/1060"/>
        <skos:definition>Optical video disc, 30 cm (12 in.) in diameter. It was the first commercial optical disc storage medium.</skos:definition>
    </owl:NamedIndividual>
    


    <!-- http://performedmusicontology.org/adLib -->

    <owl:NamedIndividual rdf:about="http://performedmusicontology.org/adLib">
        <rdf:type rdf:resource="http://performedmusicontology.org/ontology/MediumPartType"/>
        <rdfs:comment>For mediums of performance marked &quot;ad lib&quot; or &quot;ad libitum&quot; in a score or otherwise.</rdfs:comment>
        <rdfs:label>ad lib</rdfs:label>
        <skos:altLabel>ad libitum</skos:altLabel>
    </owl:NamedIndividual>
    


    <!-- http://performedmusicontology.org/offstage -->

    <owl:NamedIndividual rdf:about="http://performedmusicontology.org/offstage">
        <rdf:type rdf:resource="http://performedmusicontology.org/ontology/MediumPartType"/>
        <rdfs:label>offstage</rdfs:label>
        <skos:definition>A declared or performed medium that is to be performed or is performed offstage, i.e., out of sight of the audience.</skos:definition>
    </owl:NamedIndividual>
    


    <!-- http://performedmusicontology.org/optional -->

    <owl:NamedIndividual rdf:about="http://performedmusicontology.org/optional">
        <rdf:type rdf:resource="http://performedmusicontology.org/ontology/MediumPartType"/>
        <rdfs:label>optional</rdfs:label>
        <skos:definition>For mediums of performance marked &quot;optional&quot; in a score or otherwise.</skos:definition>
    </owl:NamedIndividual>
    


    <!-- http://performedmusicontology.org/solo -->

    <owl:NamedIndividual rdf:about="http://performedmusicontology.org/solo">
        <rdf:type rdf:resource="http://performedmusicontology.org/ontology/MediumPartType"/>
        <rdfs:label>solo</rdfs:label>
        <skos:definition>For mediums of performance marked &quot;solo&quot; in a score or is clearly a solo part in the context of the work, e.g., a concerto for oboe and orchestra.</skos:definition>
    </owl:NamedIndividual>
    


    <!-- http://performedmusicontology.org/45 -->

    <owl:NamedIndividual rdf:about="http://performedmusicontology.org/45">
        <rdf:type rdf:resource="http://id.loc.gov/ontologies/bibframe/Carrier"/>
        <rdfs:label>45 recording</rdfs:label>
        <skos:broader rdf:resource="http://rdaregistry.info/termList/RDACarrierType/1004"/>
        <skos:definition>Colloquial term representing 7&quot; diameter vinyl audio discs with a playing speed of 45 rpm. The term does not necessarily accurately describe the carrier.</skos:definition>
    </owl:NamedIndividual>
    


    <!-- http://performedmusicontology.org/78recording -->

    <owl:NamedIndividual rdf:about="http://performedmusicontology.org/78recording">
        <rdf:type rdf:resource="http://id.loc.gov/ontologies/bibframe/Carrier"/>
        <rdfs:label>78 recording</rdfs:label>
        <skos:broader rdf:resource="http://rdaregistry.info/termList/RDACarrierType/1004"/>
        <skos:definition>Colloquial term representing audio discs from the 78 rpm disc era, with actual playing speeds ranging from around 60 rpm to 130 rpm.The term does not necessarily accurately describe the carrier.</skos:definition>
    </owl:NamedIndividual>
    


    <!-- http://performedmusicontology.org/ontology/AAC -->

    <owl:NamedIndividual rdf:about="http://performedmusicontology.org/ontology/AAC">
        <rdf:type rdf:resource="http://id.loc.gov/ontologies/bibframe/EncodingFormat"/>
        <rdfs:label>AAC</rdfs:label>
        <skos:definition>Advanced Audio Coding format, a proprietary audio coding standard for lossy digital audio compression.</skos:definition>
    </owl:NamedIndividual>
    


    <!-- http://performedmusicontology.org/ontology/AIFF -->

    <owl:NamedIndividual rdf:about="http://performedmusicontology.org/ontology/AIFF">
        <rdf:type rdf:resource="http://id.loc.gov/ontologies/bibframe/EncodingFormat"/>
        <rdfs:label>AIFF</rdfs:label>
        <skos:definition>Standard audio file format used by Apple.</skos:definition>
    </owl:NamedIndividual>
    


    <!-- http://performedmusicontology.org/ontology/CdAudio -->

    <owl:NamedIndividual rdf:about="http://performedmusicontology.org/ontology/CdAudio">
        <rdf:type rdf:resource="http://id.loc.gov/ontologies/bibframe/Carrier"/>
        <rdfs:label>CD Audio</rdfs:label>
        <skos:broader rdf:resource="http://rdaregistry.info/termList/RDACarrierType/1004"/>
        <skos:definition>Optical discs that use the standard compact disc format for audio. They are 12 cm (4 3/4 in.) in diameter, and encoded as 2-channel signed 16-bit Linear PCM sampled at 44,100 Hz.</skos:definition>
    </owl:NamedIndividual>
    


    <!-- http://performedmusicontology.org/ontology/DAT -->

    <owl:NamedIndividual rdf:about="http://performedmusicontology.org/ontology/DAT">
        <rdf:type rdf:resource="http://id.loc.gov/ontologies/bibframe/Carrier"/>
        <rdfs:label>DAT (Digital Audio Tape)</rdfs:label>
        <skos:broader rdf:resource="http://rdaregistry.info/termList/RDACarrierType/1007"/>
        <skos:definition>Sony&apos;s proprietary Digital Audio Tape format, characterized by magnetic media enclosed in a protective shell, with the dimensions of 8 x 6 cm, 4 mm tape or 2 7/8 x 2 1/8 in., 1/8 in. tape</skos:definition>
    </owl:NamedIndividual>
    


    <!-- http://performedmusicontology.org/ontology/DvdAudio -->

    <owl:NamedIndividual rdf:about="http://performedmusicontology.org/ontology/DvdAudio">
        <rdf:type rdf:resource="http://id.loc.gov/ontologies/bibframe/Carrier"/>
        <rdfs:label>DVD Audio</rdfs:label>
        <skos:altLabel>DVD-A</skos:altLabel>
        <skos:broader rdf:resource="http://rdaregistry.info/termList/RDACarrierType/1004"/>
        <skos:definition>DVD optical discs that use the the DVD audio format. Different bit depth/sampling rate/channel combinations can be used on a single disc.</skos:definition>
    </owl:NamedIndividual>
    


    <!-- http://performedmusicontology.org/ontology/DvdVideo -->

    <owl:NamedIndividual rdf:about="http://performedmusicontology.org/ontology/DvdVideo">
        <rdf:type rdf:resource="http://id.loc.gov/ontologies/bibframe/Carrier"/>
        <rdfs:label>DVD Video</rdfs:label>
        <skos:broader rdf:resource="http://rdaregistry.info/termList/RDACarrierType/1060"/>
        <skos:definition>DVD optical discs that use the DVD format to store digital video. From 2003, it has been the dominant consumer video format.</skos:definition>
    </owl:NamedIndividual>
    


    <!-- http://performedmusicontology.org/ontology/EightTrack -->

    <owl:NamedIndividual rdf:about="http://performedmusicontology.org/ontology/EightTrack">
        <rdf:type rdf:resource="http://id.loc.gov/ontologies/bibframe/TapeConfig"/>
        <rdfs:label>8-track</rdfs:label>
        <skos:definition>Magnetic tape divided into 8 audio tracks that run parallel with each other, on which sound and other electro-acoustic signals are captured.</skos:definition>
    </owl:NamedIndividual>
    


    <!-- http://performedmusicontology.org/ontology/EnhancedCdAudio -->

    <owl:NamedIndividual rdf:about="http://performedmusicontology.org/ontology/EnhancedCdAudio">
        <rdf:type rdf:resource="http://id.loc.gov/ontologies/bibframe/Carrier"/>
        <rdfs:label>Enhanced CD Audio</rdfs:label>
        <skos:broader rdf:resource="http://rdaregistry.info/termList/RDACarrierType/1004"/>
        <skos:definition>An optical disc containing a combination of audio and computer data for use in both CD and CD-ROM players. Usually music CDs combined with short videos or other content.</skos:definition>
    </owl:NamedIndividual>
    


    <!-- http://performedmusicontology.org/ontology/EpRecord -->

    <owl:NamedIndividual rdf:about="http://performedmusicontology.org/ontology/EpRecord">
        <rdf:type rdf:resource="http://id.loc.gov/ontologies/bibframe/Carrier"/>
        <rdfs:label>EP (Extended play)</rdfs:label>
        <skos:broader rdf:resource="http://rdaregistry.info/termList/RDACarrierType/1004"/>
        <skos:definition>A music disc that contains more tracks than a single but not as many as on a typical album/LP/disc.</skos:definition>
    </owl:NamedIndividual>
    


    <!-- http://performedmusicontology.org/ontology/FLAC -->

    <owl:NamedIndividual rdf:about="http://performedmusicontology.org/ontology/FLAC">
        <rdf:type rdf:resource="http://id.loc.gov/ontologies/bibframe/EncodingFormat"/>
        <rdfs:label>FLAC</rdfs:label>
        <skos:definition>Free Lossless Audio Codec, an open audio coding format for lossless compression of digital audio.</skos:definition>
    </owl:NamedIndividual>
    


    <!-- http://performedmusicontology.org/ontology/FullTrack -->

    <owl:NamedIndividual rdf:about="http://performedmusicontology.org/ontology/FullTrack">
        <rdf:type rdf:resource="http://id.loc.gov/ontologies/bibframe/TapeConfig"/>
        <rdfs:label>full track</rdfs:label>
        <skos:definition>Magnetic tape with 1 audio track on which sound and other electro-acoustic signals are captured.</skos:definition>
    </owl:NamedIndividual>
    


    <!-- http://performedmusicontology.org/ontology/HalfTrack -->

    <owl:NamedIndividual rdf:about="http://performedmusicontology.org/ontology/HalfTrack">
        <rdf:type rdf:resource="http://id.loc.gov/ontologies/bibframe/TapeConfig"/>
        <rdfs:label>half track</rdfs:label>
        <skos:definition>Magnetic tape divided into 2 audio tracks that run parallel with each other, on which sound and other electro-acoustic signals are captured.</skos:definition>
    </owl:NamedIndividual>
    


    <!-- http://performedmusicontology.org/ontology/HybridSacd -->

    <owl:NamedIndividual rdf:about="http://performedmusicontology.org/ontology/HybridSacd">
        <rdf:type rdf:resource="http://id.loc.gov/ontologies/bibframe/Carrier"/>
        <rdfs:label>Hybrid SACD</rdfs:label>
        <skos:broader rdf:resource="http://rdaregistry.info/termList/RDACarrierType/1004"/>
        <skos:definition>An SACD that also is also encoded with a PCM audio layer readable by compact disc players.</skos:definition>
    </owl:NamedIndividual>
    


    <!-- http://performedmusicontology.org/ontology/IPS.9 -->

    <owl:NamedIndividual rdf:about="http://performedmusicontology.org/ontology/IPS.9">
        <rdf:type rdf:resource="http://id.loc.gov/ontologies/bibframe/PlayingSpeed"/>
        <rdfs:comment>Speed occurs on half-speed mini-cassettes used in small portable recorders.</rdfs:comment>
        <rdfs:label>15/16 ips</rdfs:label>
        <skos:definition>Playing speed of 15/16 inches per second.</skos:definition>
    </owl:NamedIndividual>
    


    <!-- http://performedmusicontology.org/ontology/IPS1.8 -->

    <owl:NamedIndividual rdf:about="http://performedmusicontology.org/ontology/IPS1.8">
        <rdf:type rdf:resource="http://id.loc.gov/ontologies/bibframe/PlayingSpeed"/>
        <rdfs:comment>Speed occurs on standard audiocassettes.</rdfs:comment>
        <rdfs:label>1 7/8 ips</rdfs:label>
        <skos:definition>Playing speed of 1 7/8 inches per second.</skos:definition>
    </owl:NamedIndividual>
    


    <!-- http://performedmusicontology.org/ontology/IPS15 -->

    <owl:NamedIndividual rdf:about="http://performedmusicontology.org/ontology/IPS15">
        <rdf:type rdf:resource="http://id.loc.gov/ontologies/bibframe/PlayingSpeed"/>
        <rdfs:comment>Occcurs on reel-to-reel, studio tapes.</rdfs:comment>
        <rdfs:label>15 ips</rdfs:label>
        <skos:definition>Playing speed of 15 inches per second.</skos:definition>
    </owl:NamedIndividual>
    


    <!-- http://performedmusicontology.org/ontology/IPS3.75 -->

    <owl:NamedIndividual rdf:about="http://performedmusicontology.org/ontology/IPS3.75">
        <rdf:type rdf:resource="http://id.loc.gov/ontologies/bibframe/PlayingSpeed"/>
        <rdfs:comment>Speed occurs on consumer and nonprofessional reel-to-reel tapes, cartridges and very unusual cassette tapes.</rdfs:comment>
        <rdfs:label>3.75 ips</rdfs:label>
        <skos:definition>Playing speed of 3.75 inches per second</skos:definition>
    </owl:NamedIndividual>
    


    <!-- http://performedmusicontology.org/ontology/IPS30 -->

    <owl:NamedIndividual rdf:about="http://performedmusicontology.org/ontology/IPS30">
        <rdf:type rdf:resource="http://id.loc.gov/ontologies/bibframe/PlayingSpeed"/>
        <rdfs:comment>Occurs on reel-to-reel, studio tapes, but is rarely used.</rdfs:comment>
        <rdfs:label>30 ips</rdfs:label>
        <skos:definition>Playing speed of 30 inches per second.</skos:definition>
    </owl:NamedIndividual>
    


    <!-- http://performedmusicontology.org/ontology/IPS7.5 -->

    <owl:NamedIndividual rdf:about="http://performedmusicontology.org/ontology/IPS7.5">
        <rdf:type rdf:resource="http://id.loc.gov/ontologies/bibframe/PlayingSpeed"/>
        <rdfs:comment>Speed occurs in reel-to-reel, nonprofessional, and studio tapes.</rdfs:comment>
        <rdfs:label>7.5 ips</rdfs:label>
        <skos:definition>Playing speed of 7.5 inches per second.</skos:definition>
    </owl:NamedIndividual>
    


    <!-- http://performedmusicontology.org/ontology/LP -->

    <owl:NamedIndividual rdf:about="http://performedmusicontology.org/ontology/LP">
        <rdf:type rdf:resource="http://id.loc.gov/ontologies/bibframe/Carrier"/>
        <rdfs:label>LP/Vinyl</rdfs:label>
        <skos:broader rdf:resource="http://rdaregistry.info/termList/RDACarrierType/1004"/>
        <skos:definition>Colloquial term representing 12&quot; diameter vinyl audio discs with a playing speed of 33 1/3 rpm. The term does not necessarily accurately describe the carrier.</skos:definition>
    </owl:NamedIndividual>
    


    <!-- http://performedmusicontology.org/ontology/LateralCut -->

    <owl:NamedIndividual rdf:about="http://performedmusicontology.org/ontology/LateralCut">
        <rdf:type rdf:resource="http://performedmusicontology.org/ontology/DiscCutting"/>
        <rdfs:label>Lateral cut</rdfs:label>
        <skos:definition>Recording process in which a stylus cuts a side-to-side groove into a phonograph record.</skos:definition>
    </owl:NamedIndividual>
    


    <!-- http://performedmusicontology.org/ontology/MP3 -->

    <owl:NamedIndividual rdf:about="http://performedmusicontology.org/ontology/MP3">
        <rdf:type rdf:resource="http://id.loc.gov/ontologies/bibframe/EncodingFormat"/>
        <rdfs:comment>MPEG Layer III Audio, and audio encoding format for digital audio.</rdfs:comment>
        <rdfs:label>MP3</rdfs:label>
    </owl:NamedIndividual>
    


    <!-- http://performedmusicontology.org/ontology/MPS1.4 -->

    <owl:NamedIndividual rdf:about="http://performedmusicontology.org/ontology/MPS1.4">
        <rdf:type rdf:resource="http://id.loc.gov/ontologies/bibframe/PlayingSpeed"/>
        <rdfs:comment>Speed is calculated from the distance the playback mechanism covers on the surface of the disc per second, and not the number of revolutions of the disc. It is associated with compact discs (CDs)</rdfs:comment>
        <rdfs:label>1.4 mps</rdfs:label>
        <skos:definition>Playing speed of 1.4 meters per second.</skos:definition>
    </owl:NamedIndividual>
    


    <!-- http://performedmusicontology.org/ontology/OrganRoll -->

    <owl:NamedIndividual rdf:about="http://performedmusicontology.org/ontology/OrganRoll">
        <rdf:type rdf:resource="http://id.loc.gov/ontologies/bibframe/Carrier"/>
        <rdfs:label>Organ roll</rdfs:label>
        <skos:broader rdf:resource="http://rdaregistry.info/termList/RDACarrierType/1006"/>
        <skos:definition>An audio roll used to operate a player piano or reproducing organ.</skos:definition>
    </owl:NamedIndividual>
    


    <!-- http://performedmusicontology.org/ontology/PianoRoll -->

    <owl:NamedIndividual rdf:about="http://performedmusicontology.org/ontology/PianoRoll">
        <rdf:type rdf:resource="http://id.loc.gov/ontologies/bibframe/Carrier"/>
        <rdfs:label>Piano roll</rdfs:label>
        <skos:broader rdf:resource="http://rdaregistry.info/termList/RDACarrierType/1006"/>
        <skos:definition>Audio roll used to operate a player piano or reproducing piano.</skos:definition>
    </owl:NamedIndividual>
    


    <!-- http://performedmusicontology.org/ontology/QuarterTrack -->

    <owl:NamedIndividual rdf:about="http://performedmusicontology.org/ontology/QuarterTrack">
        <rdf:type rdf:resource="http://id.loc.gov/ontologies/bibframe/TapeConfig"/>
        <rdfs:label>quarter track</rdfs:label>
        <skos:definition>Magnetic tape divided into 4 audio tracks that run parallel with each other, in which sound and other electro-acoustic signals are captured.</skos:definition>
    </owl:NamedIndividual>
    


    <!-- http://performedmusicontology.org/ontology/RPM16 -->

    <owl:NamedIndividual rdf:about="http://performedmusicontology.org/ontology/RPM16">
        <rdf:type rdf:resource="http://id.loc.gov/ontologies/bibframe/PlayingSpeed"/>
        <rdfs:comment>For audio discs</rdfs:comment>
        <rdfs:label>16 rpm</rdfs:label>
        <skos:definition>Playing speed of 16 revolutions per minute.</skos:definition>
    </owl:NamedIndividual>
    


    <!-- http://performedmusicontology.org/ontology/RPM33 -->

    <owl:NamedIndividual rdf:about="http://performedmusicontology.org/ontology/RPM33">
        <rdf:type rdf:resource="http://id.loc.gov/ontologies/bibframe/PlayingSpeed"/>
        <rdfs:comment>For audio discs.</rdfs:comment>
        <rdfs:label>33 1/3 rpm</rdfs:label>
        <skos:definition>Playing speed of 33 1/3 revolutions per minute. Often shortened to &quot;33&quot;.</skos:definition>
    </owl:NamedIndividual>
    


    <!-- http://performedmusicontology.org/ontology/RPM45 -->

    <owl:NamedIndividual rdf:about="http://performedmusicontology.org/ontology/RPM45">
        <rdf:type rdf:resource="http://id.loc.gov/ontologies/bibframe/PlayingSpeed"/>
        <rdfs:comment>For audio discs.</rdfs:comment>
        <rdfs:label>45 rpm</rdfs:label>
        <skos:definition>Playing speed of 45 revolutions per minute.</skos:definition>
    </owl:NamedIndividual>
    


    <!-- http://performedmusicontology.org/ontology/RPM78 -->

    <owl:NamedIndividual rdf:about="http://performedmusicontology.org/ontology/RPM78">
        <rdf:type rdf:resource="http://id.loc.gov/ontologies/bibframe/PlayingSpeed"/>
        <rdfs:comment>For audio discs</rdfs:comment>
        <rdfs:label>78 rpm</rdfs:label>
        <skos:definition>Playing speed of 78 revolutions per minute.</skos:definition>
    </owl:NamedIndividual>
    


    <!-- http://performedmusicontology.org/ontology/RPM8 -->

    <owl:NamedIndividual rdf:about="http://performedmusicontology.org/ontology/RPM8">
        <rdf:type rdf:resource="http://id.loc.gov/ontologies/bibframe/PlayingSpeed"/>
        <rdfs:comment>For audio discs</rdfs:comment>
        <rdfs:label>8 rpm</rdfs:label>
        <skos:definition>Playing speed of 8 revolutions per minute.</skos:definition>
    </owl:NamedIndividual>
    


    <!-- http://performedmusicontology.org/ontology/Sacd -->

    <owl:NamedIndividual rdf:about="http://performedmusicontology.org/ontology/Sacd">
        <rdf:type rdf:resource="http://id.loc.gov/ontologies/bibframe/Carrier"/>
        <rdfs:label>SACD</rdfs:label>
        <skos:altLabel>Super audio compact disc</skos:altLabel>
        <skos:broader rdf:resource="http://rdaregistry.info/termList/RDACarrierType/1004"/>
        <skos:definition>Optical audio disc with more channels and longer playing time than a conventional CD.</skos:definition>
    </owl:NamedIndividual>
    


    <!-- http://performedmusicontology.org/ontology/SixteenTrack -->

    <owl:NamedIndividual rdf:about="http://performedmusicontology.org/ontology/SixteenTrack">
        <rdf:type rdf:resource="http://id.loc.gov/ontologies/bibframe/TapeConfig"/>
        <rdfs:label>16-track</rdfs:label>
        <skos:definition>Magnetic tape divided into 16 audio tracks that run parallel with each other, on which sound and other electro-acoustic signals are captured.</skos:definition>
    </owl:NamedIndividual>
    


    <!-- http://performedmusicontology.org/ontology/TwelveTrack -->

    <owl:NamedIndividual rdf:about="http://performedmusicontology.org/ontology/TwelveTrack">
        <rdf:type rdf:resource="http://id.loc.gov/ontologies/bibframe/TapeConfig"/>
        <rdfs:label>12-track</rdfs:label>
        <skos:definition>Magnetic tape divided into 12 audio tracks that run parallel with each other, on which sound and other electro-acoustic signals are captured.</skos:definition>
    </owl:NamedIndividual>
    


    <!-- http://performedmusicontology.org/ontology/Vertical -->

    <owl:NamedIndividual rdf:about="http://performedmusicontology.org/ontology/Vertical">
        <rdf:type rdf:resource="http://performedmusicontology.org/ontology/DiscCutting"/>
        <rdfs:label>Vertical cut</rdfs:label>
        <skos:altLabel>Hill and dale</skos:altLabel>
        <skos:definition>Recording process in which a stylus cuts a vertical groove into a phonograph record.</skos:definition>
    </owl:NamedIndividual>
    


    <!-- http://performedmusicontology.org/ontology/amplified -->

    <owl:NamedIndividual rdf:about="http://performedmusicontology.org/ontology/amplified">
        <rdf:type rdf:resource="http://performedmusicontology.org/ontology/MediumPartType"/>
        <rdfs:comment>For mediums of performance marked &quot;amplified&quot; in a score or otherwise.</rdfs:comment>
    </owl:NamedIndividual>
    


    <!-- http://performedmusicontology.org/ontology/obligato -->

    <owl:NamedIndividual rdf:about="http://performedmusicontology.org/ontology/obligato">
        <rdf:type rdf:resource="http://performedmusicontology.org/ontology/MediumPartType"/>
        <rdfs:label>obligato</rdfs:label>
        <skos:definition>For mediums of performance marked &quot;obligato&quot; in a score or otherwise.</skos:definition>
    </owl:NamedIndividual>
    


    <!-- http://rdaregistry.info/termList/RDACarrierType -->

    <owl:NamedIndividual rdf:about="http://rdaregistry.info/termList/RDACarrierType">
        <rdf:type rdf:resource="http://www.w3.org/2004/02/skos/core#ConceptScheme"/>
        <dc:title>RDA Carrier Type</dc:title>
    </owl:NamedIndividual>
    


    <!-- http://rdaregistry.info/termList/RDACarrierType/1003 -->

    <owl:NamedIndividual rdf:about="http://rdaregistry.info/termList/RDACarrierType/1003">
        <rdf:type rdf:resource="http://www.w3.org/2004/02/skos/core#Concept"/>
        <rdakit:toolkitDefinition xml:lang="en">A carrier type consisting of a roller-shaped object on which sound waves are incised or indented in a continuous circular groove.</rdakit:toolkitDefinition>
        <rdakit:toolkitDefinition xml:lang="da">Bærertype, der består af et rulleformet genstand, hvorpå lydbølger er indskåret eller indtrykt i en uafbrudt cirkulær rille.</rdakit:toolkitDefinition>
        <rdakit:toolkitDefinition xml:lang="nl">Een rolvormig object waarop geluidsgolven worden ingesneden of ingesprongen in een continue cirkelvormige groef.</rdakit:toolkitDefinition>
        <rdakit:toolkitDefinition xml:lang="de">Ein Datenträgertyp, der aus einem rollenförmigen Objekt besteht, auf dem Schallwellen in einer fortlaufend gewundenen Rille graviert oder eingeprägt sind.</rdakit:toolkitDefinition>
        <rdakit:toolkitDefinition xml:lang="no">En bærertype som består av en sylinderformet gjenstand der lydopptak er gravert inn i et uavbrutt, sirkulært spor.</rdakit:toolkitDefinition>
        <rdakit:toolkitDefinition xml:lang="vi">Loại hộp chứa gồm có vật thể hình trục lăn trên đó sóng âm được vạch hoặc rập trong đường rãnh xoắn ốc liên tục.</rdakit:toolkitDefinition>
        <rdakit:toolkitDefinition xml:lang="es">Objeto con forma de rollo en el cual se han hecho incisiones o muescas en un surco circular continuo.</rdakit:toolkitDefinition>
        <rdakit:toolkitDefinition xml:lang="fi">Rullamuotoinen tallennetyyppi, johon ääniaallot on kaiverrettu tai uurrettu yhtenäisenä pyöreänä urana.</rdakit:toolkitDefinition>
        <rdakit:toolkitDefinition xml:lang="ca">Tipus de suport físic que consisteix en un objecte en forma de rotlle en el qual s’han gravat ones sonores per mitjà d’incisions o marques tot creant un solc circular continu.</rdakit:toolkitDefinition>
        <rdakit:toolkitDefinition xml:lang="fr">Type de support matériel qui consiste en un objet en forme de rouleau sur lequel des ondulations sonores ont été gravées au moyen d’une entaille ou d’empreintes en créant un sillon circulaire continu.</rdakit:toolkitDefinition>
        <rdakit:toolkitDefinition xml:lang="zh">通过刻痕或连续的螺旋式纹槽在其上记录声波的滚筒形物体，包括蜡滚筒、金属丝滚筒等。</rdakit:toolkitDefinition>
        <rdakit:toolkitLabel xml:lang="de">Phonographenzylinder</rdakit:toolkitLabel>
        <rdakit:toolkitLabel xml:lang="en">audio cylinder</rdakit:toolkitLabel>
        <rdakit:toolkitLabel xml:lang="nl">audiocilinder</rdakit:toolkitLabel>
        <rdakit:toolkitLabel xml:lang="ca">cilindre àudio</rdakit:toolkitLabel>
        <rdakit:toolkitLabel xml:lang="it">cilindro audio</rdakit:toolkitLabel>
        <rdakit:toolkitLabel xml:lang="es">cilindro sonoro</rdakit:toolkitLabel>
        <rdakit:toolkitLabel xml:lang="fr">cylindre audio</rdakit:toolkitLabel>
        <rdakit:toolkitLabel xml:lang="no">fonografrull</rdakit:toolkitLabel>
        <rdakit:toolkitLabel xml:lang="sv">ljudcylinder</rdakit:toolkitLabel>
        <rdakit:toolkitLabel xml:lang="da">lydvalse</rdakit:toolkitLabel>
        <rdakit:toolkitLabel xml:lang="vi">trục lăn audio</rdakit:toolkitLabel>
        <rdakit:toolkitLabel xml:lang="fi">äänisylinteri</rdakit:toolkitLabel>
        <rdakit:toolkitLabel xml:lang="zh">录音筒</rdakit:toolkitLabel>
        <regap:identifier rdf:resource="http://metadataregistry.org/concepts/535"/>
        <rdfs:label>audio cylinder</rdfs:label>
        <skos:definition xml:lang="en">A carrier type consisting of a roller-shaped object on which sound waves are incised or indented in a continuous circular groove.</skos:definition>
        <skos:definition xml:lang="da">Bærertype, der består af et rulleformet genstand, hvorpå lydbølger er indskåret eller indtrykt i en uafbrudt cirkulær rille.</skos:definition>
        <skos:definition xml:lang="nl">Een rolvormig object waarop geluidsgolven worden ingesneden of ingesprongen in een continue cirkelvormige groef.</skos:definition>
        <skos:definition xml:lang="de">Ein Datenträgertyp, der aus einem rollenförmigen Objekt besteht, auf dem Schallwellen in einer fortlaufend gewundenen Rille graviert oder eingeprägt sind.</skos:definition>
        <skos:definition xml:lang="no">En bærertype som består av en sylinderformet gjenstand der lydopptak er gravert inn i et uavbrutt, sirkulært spor.</skos:definition>
        <skos:definition xml:lang="vi">Loại hộp chứa gồm có vật thể hình trục lăn trên đó sóng âm được vạch hoặc rập trong đường rãnh xoắn ốc liên tục.</skos:definition>
        <skos:definition xml:lang="es">Objeto con forma de rollo en el cual se han hecho incisiones o muescas en un surco circular continuo.</skos:definition>
        <skos:definition xml:lang="fi">Rullamuotoinen tallennetyyppi, johon ääniaallot on kaiverrettu tai uurrettu yhtenäisenä pyöreänä urana.</skos:definition>
        <skos:definition xml:lang="ca">Tipus de suport físic que consisteix en un objecte en forma de rotlle en el qual s’han gravat ones sonores per mitjà d’incisions o marques tot creant un solc circular continu.</skos:definition>
        <skos:definition xml:lang="fr">Type de support matériel qui consiste en un objet en forme de rouleau sur lequel des ondulations sonores ont été gravées au moyen d’une entaille ou d’empreintes en créant un sillon circulaire continu.</skos:definition>
        <skos:definition xml:lang="zh">通过刻痕或连续的螺旋式纹槽在其上记录声波的滚筒形物体，包括蜡滚筒、金属丝滚筒等。</skos:definition>
        <skos:inScheme rdf:resource="http://rdaregistry.info/termList/RDACarrierType"/>
        <skos:prefLabel xml:lang="de">Phonographenzylinder</skos:prefLabel>
        <skos:prefLabel xml:lang="en">audio cylinder</skos:prefLabel>
        <skos:prefLabel xml:lang="nl">audiocilinder</skos:prefLabel>
        <skos:prefLabel xml:lang="ca">cilindre àudio</skos:prefLabel>
        <skos:prefLabel xml:lang="it">cilindro audio</skos:prefLabel>
        <skos:prefLabel xml:lang="es">cilindro sonoro</skos:prefLabel>
        <skos:prefLabel xml:lang="fr">cylindre audio</skos:prefLabel>
        <skos:prefLabel xml:lang="no">fonografrull</skos:prefLabel>
        <skos:prefLabel xml:lang="sv">ljudcylinder</skos:prefLabel>
        <skos:prefLabel xml:lang="da">lydvalse</skos:prefLabel>
        <skos:prefLabel xml:lang="vi">trục lăn audio</skos:prefLabel>
        <skos:prefLabel xml:lang="fi">äänisylinteri</skos:prefLabel>
        <skos:prefLabel xml:lang="ar">أسطوانة سمعية</skos:prefLabel>
        <skos:prefLabel xml:lang="zh">录音筒</skos:prefLabel>
        <skos:scopeNote xml:lang="fr">Comprend les cylindres de cire, cylindres de fil, etc.</skos:scopeNote>
        <skos:scopeNote xml:lang="de">Dazu gehören Wachszylinder, Drahtzylinder usw.</skos:scopeNote>
        <skos:scopeNote xml:lang="fi">Esim. vahasylinteri, vaijerisylinteri.</skos:scopeNote>
        <skos:scopeNote xml:lang="ca">Inclou cilindres de cera, de filferro, etc.</skos:scopeNote>
        <skos:scopeNote xml:lang="es">Incluye cilindros de cera, cilindros metálicos, etc.</skos:scopeNote>
        <skos:scopeNote xml:lang="vi">Trục lăn sáp, trục lăn dây, v.v..., được bao gồm</skos:scopeNote>
        <skos:scopeNote xml:lang="no">Vokssylindre, sylindre med metalltråd, etc. er inkludert.</skos:scopeNote>
        <skos:scopeNote xml:lang="en">Wax cylinders, wire cylinders, etc., are included.</skos:scopeNote>
        <skos:scopeNote xml:lang="zh">包括腊筒、线筒等</skos:scopeNote>
    </owl:NamedIndividual>
    


    <!-- http://rdaregistry.info/termList/RDACarrierType/1004 -->

    <owl:NamedIndividual rdf:about="http://rdaregistry.info/termList/RDACarrierType/1004">
        <rdf:type rdf:resource="http://www.w3.org/2004/02/skos/core#Concept"/>
        <rdakit:toolkitDefinition xml:lang="en">A carrier type consisting of a disc on which sound waves, recorded as modulations, pulses, etc., are incised or indented in a continuous spiral groove.</rdakit:toolkitDefinition>
        <rdakit:toolkitDefinition xml:lang="da">Bærertype, der består af en disc eller plade, hvorpå lydbølger optaget som modulationer, rytmer etc. er ridset eller indtrykt i en uafbrudt cirkulær rille.</rdakit:toolkitDefinition>
        <rdakit:toolkitDefinition xml:lang="es">Disco en el que las ondas sonoras, registradas como modulaciones, pulsos, etc., se registraron mediante incisiones o muescas en un surco en espiral continua.</rdakit:toolkitDefinition>
        <rdakit:toolkitDefinition xml:lang="nl">Een disc waarop geluidsgolven, opgeslagen als modulaties, pulsen etc., ingesneden of ingesprongen zijn in een continue spiraalvormige groef.</rdakit:toolkitDefinition>
        <rdakit:toolkitDefinition xml:lang="de">Ein Datenträgertyp, der aus einer Disk besteht, auf der als Modulation, Pulse usw. aufgenommene Schallwellen in einer fortlaufend gewundenen Rille graviert oder eingeprägt sind.</rdakit:toolkitDefinition>
        <rdakit:toolkitDefinition xml:lang="no">En bærertype som består av en plate der lydbølger, registrert som modulasjoner, pulser, etc. er gravert inn i et uavbrutt, spiralformet spor.</rdakit:toolkitDefinition>
        <rdakit:toolkitDefinition xml:lang="fi">Levy, jolle on kaiverrettu tai uurrettu modulaatioiksi tai pulsseiksi tallennettuja äänisignaaleja yhtenäiseksi spiraalimaiseksi uraksi.</rdakit:toolkitDefinition>
        <rdakit:toolkitDefinition xml:lang="vi">Loại hộp chứa gồm có đĩa trên đó sóng âm ghi lại như là chuyển giọng, nhịp điệu, vv... được vạch hoặc rập trong đường rãnh xoắn ốc liên tục.</rdakit:toolkitDefinition>
        <rdakit:toolkitDefinition xml:lang="ca">Tipus de suport físic que consisteix en un disc en el qual s’han gravat ones sonores, enregistrades com a modulacions, impulsos, etc., per mitjà d’incisions o marques en un solc continu en espiral.</rdakit:toolkitDefinition>
        <rdakit:toolkitDefinition xml:lang="fr">Type de support matériel qui consiste en un disque sur lequel des ondulations sonores, enregistrées sous forme de modulations, d’impulsions, etc., ont été gravées au moyen d’une entaille ou d’empreintes en créant un sillon continu en spirale.</rdakit:toolkitDefinition>
        <rdakit:toolkitDefinition xml:lang="zh">通过刻痕或连续的螺旋式纹槽在其上将声波记录为音调、节奏等的盘片。</rdakit:toolkitDefinition>
        <rdakit:toolkitLabel xml:lang="de">Audiodisk</rdakit:toolkitLabel>
        <rdakit:toolkitLabel xml:lang="en">audio disc</rdakit:toolkitLabel>
        <rdakit:toolkitLabel xml:lang="nl">audiodisc</rdakit:toolkitLabel>
        <rdakit:toolkitLabel xml:lang="ca">disc àudio</rdakit:toolkitLabel>
        <rdakit:toolkitLabel xml:lang="it">disco audio</rdakit:toolkitLabel>
        <rdakit:toolkitLabel xml:lang="es">disco sonoro</rdakit:toolkitLabel>
        <rdakit:toolkitLabel xml:lang="fr">disque audio</rdakit:toolkitLabel>
        <rdakit:toolkitLabel xml:lang="no">grammofonplate</rdakit:toolkitLabel>
        <rdakit:toolkitLabel xml:lang="sv">ljudskiva</rdakit:toolkitLabel>
        <rdakit:toolkitLabel xml:lang="da">lyddisc</rdakit:toolkitLabel>
        <rdakit:toolkitLabel xml:lang="fi">äänilevy</rdakit:toolkitLabel>
        <rdakit:toolkitLabel xml:lang="vi">đĩa audio</rdakit:toolkitLabel>
        <rdakit:toolkitLabel xml:lang="zh">录音盘</rdakit:toolkitLabel>
        <regap:identifier rdf:resource="http://metadataregistry.org/concepts/536"/>
        <rdfs:label>audio disc</rdfs:label>
        <skos:altLabel xml:lang="da">audiodisc</skos:altLabel>
        <skos:altLabel xml:lang="ca">disc sonor</skos:altLabel>
        <skos:altLabel xml:lang="es">disco de audio</skos:altLabel>
        <skos:altLabel xml:lang="fr">disque sonore</skos:altLabel>
        <skos:altLabel xml:lang="en">sound disc</skos:altLabel>
        <skos:altLabel xml:lang="vi">đĩa âm thanh</skos:altLabel>
        <skos:altLabel xml:lang="zh">声音盘</skos:altLabel>
        <skos:definition xml:lang="en">A carrier type consisting of a disc on which sound waves, recorded as modulations, pulses, etc., are incised or indented in a continuous spiral groove.</skos:definition>
        <skos:definition xml:lang="da">Bærertype, der består af en disc eller plade, hvorpå lydbølger optaget som modulationer, rytmer etc. er ridset eller indtrykt i en uafbrudt cirkulær rille.</skos:definition>
        <skos:definition xml:lang="es">Disco en el que las ondas sonoras, registradas como modulaciones, pulsos, etc., se registraron mediante incisiones o muescas en un surco en espiral continua.</skos:definition>
        <skos:definition xml:lang="nl">Een disc waarop geluidsgolven, opgeslagen als modulaties, pulsen etc., ingesneden of ingesprongen zijn in een continue spiraalvormige groef.</skos:definition>
        <skos:definition xml:lang="de">Ein Datenträgertyp, der aus einer Disk besteht, auf der als Modulation, Pulse usw. aufgenommene Schallwellen in einer fortlaufend gewundenen Rille graviert oder eingeprägt sind.</skos:definition>
        <skos:definition xml:lang="no">En bærertype som består av en plate der lydbølger, registrert som modulasjoner, pulser, etc. er gravert inn i et uavbrutt, spiralformet spor.</skos:definition>
        <skos:definition xml:lang="fi">Levy, jolle on kaiverrettu tai uurrettu modulaatioiksi tai pulsseiksi tallennettuja äänisignaaleja yhtenäiseksi spiraalimaiseksi uraksi.</skos:definition>
        <skos:definition xml:lang="vi">Loại hộp chứa gồm có đĩa trên đó sóng âm ghi lại như là chuyển giọng, nhịp điệu, vv... được vạch hoặc rập trong đường rãnh xoắn ốc liên tục.</skos:definition>
        <skos:definition xml:lang="ca">Tipus de suport físic que consisteix en un disc en el qual s’han gravat ones sonores, enregistrades com a modulacions, impulsos, etc., per mitjà d’incisions o marques en un solc continu en espiral.</skos:definition>
        <skos:definition xml:lang="fr">Type de support matériel qui consiste en un disque sur lequel des ondulations sonores, enregistrées sous forme de modulations, d’impulsions, etc., ont été gravées au moyen d’une entaille ou d’empreintes en créant un sillon continu en spirale.</skos:definition>
        <skos:definition xml:lang="zh">通过刻痕或连续的螺旋式纹槽在其上将声波记录为音调、节奏等的盘片。</skos:definition>
        <skos:inScheme rdf:resource="http://rdaregistry.info/termList/RDACarrierType"/>
        <skos:narrower rdf:resource="http://performedmusicontology.org/45"/>
        <skos:narrower rdf:resource="http://performedmusicontology.org/78recording"/>
        <skos:narrower rdf:resource="http://performedmusicontology.org/ontology/CdAudio"/>
        <skos:narrower rdf:resource="http://performedmusicontology.org/ontology/DvdAudio"/>
        <skos:narrower rdf:resource="http://performedmusicontology.org/ontology/EnhancedCdAudio"/>
        <skos:narrower rdf:resource="http://performedmusicontology.org/ontology/EpRecord"/>
        <skos:narrower rdf:resource="http://performedmusicontology.org/ontology/HybridSacd"/>
        <skos:narrower rdf:resource="http://performedmusicontology.org/ontology/Sacd"/>
        <skos:prefLabel xml:lang="de">Audiodisk</skos:prefLabel>
        <skos:prefLabel xml:lang="en">audio disc</skos:prefLabel>
        <skos:prefLabel xml:lang="nl">audiodisc</skos:prefLabel>
        <skos:prefLabel xml:lang="ca">disc àudio</skos:prefLabel>
        <skos:prefLabel xml:lang="it">disco audio</skos:prefLabel>
        <skos:prefLabel xml:lang="es">disco sonoro</skos:prefLabel>
        <skos:prefLabel xml:lang="fr">disque audio</skos:prefLabel>
        <skos:prefLabel xml:lang="no">grammofonplate</skos:prefLabel>
        <skos:prefLabel xml:lang="sv">ljudskiva</skos:prefLabel>
        <skos:prefLabel xml:lang="da">lyddisc</skos:prefLabel>
        <skos:prefLabel xml:lang="fi">äänilevy</skos:prefLabel>
        <skos:prefLabel xml:lang="vi">đĩa audio</skos:prefLabel>
        <skos:prefLabel xml:lang="ar">قرص صوتي</skos:prefLabel>
        <skos:prefLabel xml:lang="zh">录音盘</skos:prefLabel>
    </owl:NamedIndividual>
    


    <!-- http://rdaregistry.info/termList/RDACarrierType/1006 -->

    <owl:NamedIndividual rdf:about="http://rdaregistry.info/termList/RDACarrierType/1006">
        <rdf:type rdf:resource="http://www.w3.org/2004/02/skos/core#Concept"/>
        <rdakit:toolkitDefinition xml:lang="en">A carrier type consisting of a roll of paper on which musical notes are represented by perforations, designed to mechanically reproduce the music when used in a player piano, player organ, etc.</rdakit:toolkitDefinition>
        <rdakit:toolkitDefinition xml:lang="da">Bærertype, der består af en papirrulle, hvorpå musiknoder repræsenteres af huller skabt til at gengive musikken mekanisk, når rullen bruges i et pianola, mekanisk klaver etc.</rdakit:toolkitDefinition>
        <rdakit:toolkitDefinition xml:lang="nl">Een rol papier waarop muzieknoten voorgesteld worden door perforaties, ontworpen om mechanisch de muziek weer te geven wanneer deze gebruikt wordt in een pianola e.d.</rdakit:toolkitDefinition>
        <rdakit:toolkitDefinition xml:lang="de">Ein Datenträgertyp, der aus einer Papierrolle besteht, auf der Musiknoten in Form von Perforationen repräsentiert werden und die konzipiert ist, um Musik in einem mechanischen Klavier, einer mechanischen Orgel usw. wiederzugeben.</rdakit:toolkitDefinition>
        <rdakit:toolkitDefinition xml:lang="no">En bærertype som består av en papirrull der musikknoter representeres av hull, utformet for å gjengi musikken mekanisk ved bruk i pianola og lignende mekaniske instrumenter.</rdakit:toolkitDefinition>
        <rdakit:toolkitDefinition xml:lang="vi">Loại hộp chứa gồm có cuốn giấy trên đó nốt nhạc được trình bày bởi các lỗ răng cưa để tái tạo một cách cơ học âm nhạc khi dùng với piano tự động, organ tự động, vv...</rdakit:toolkitDefinition>
        <rdakit:toolkitDefinition xml:lang="fi">Paperirulla, jossa olevat rei’itykset edustavat toistettavia säveliä. Suunniteltu toistamaan musiikkia mekaanisesti automaattipianon, automaattiurkujen yms. avulla.</rdakit:toolkitDefinition>
        <rdakit:toolkitDefinition xml:lang="es">Rollo de papel en el que las notas musicales están representadas mediante perforaciones, diseñado para reproducir en forma mecánica la música cuando se utiliza en una pianola, órgano mecánico, etc.</rdakit:toolkitDefinition>
        <rdakit:toolkitDefinition xml:lang="ca">Tipus de suport físic que consisteix en un rotlle de paper sobre el qual es representen les notes musicals amb perforacions, concebut per reproduir la música mecànicament quan s’usa en una pianola, un orgue mecànic, etc.</rdakit:toolkitDefinition>
        <rdakit:toolkitDefinition xml:lang="fr">Type de support matériel qui consiste en un rouleau de papier sur lequel les notes de musique sont représentées par des perforations, destiné à reproduire mécaniquement la musique lorsqu’il est utilisé avec un piano mécanique, un orgue mécanique, etc.</rdakit:toolkitDefinition>
        <rdakit:toolkitDefinition xml:lang="zh">通过穿孔方式表示音符的纸卷，用于钢琴、风琴等时，以机械方式重现音乐。</rdakit:toolkitDefinition>
        <rdakit:toolkitLabel xml:lang="de">Notenrolle</rdakit:toolkitLabel>
        <rdakit:toolkitLabel xml:lang="en">audio roll</rdakit:toolkitLabel>
        <rdakit:toolkitLabel xml:lang="nl">audiorol</rdakit:toolkitLabel>
        <rdakit:toolkitLabel xml:lang="vi">cuốn audio</rdakit:toolkitLabel>
        <rdakit:toolkitLabel xml:lang="sv">ljudrulle</rdakit:toolkitLabel>
        <rdakit:toolkitLabel xml:lang="da">lydrulle</rdakit:toolkitLabel>
        <rdakit:toolkitLabel xml:lang="no">pianorull</rdakit:toolkitLabel>
        <rdakit:toolkitLabel xml:lang="es">rollo sonoro</rdakit:toolkitLabel>
        <rdakit:toolkitLabel xml:lang="ca">rotlle àudio</rdakit:toolkitLabel>
        <rdakit:toolkitLabel xml:lang="fr">rouleau audio</rdakit:toolkitLabel>
        <rdakit:toolkitLabel xml:lang="it">rullo audio</rdakit:toolkitLabel>
        <rdakit:toolkitLabel xml:lang="fi">äänirulla</rdakit:toolkitLabel>
        <rdakit:toolkitLabel xml:lang="zh">录音卷</rdakit:toolkitLabel>
        <regap:identifier rdf:resource="http://metadataregistry.org/concepts/538"/>
        <rdfs:label>audio roll</rdfs:label>
        <skos:altLabel xml:lang="vi">cuốn piano</skos:altLabel>
        <skos:altLabel xml:lang="en">piano roll</skos:altLabel>
        <skos:altLabel xml:lang="da">pianolarulle</skos:altLabel>
        <skos:altLabel xml:lang="fi">pianorulla</skos:altLabel>
        <skos:altLabel xml:lang="es">rollo de piano</skos:altLabel>
        <skos:altLabel xml:lang="fr">rouleau pour piano</skos:altLabel>
        <skos:altLabel xml:lang="zh">钢琴滚筒</skos:altLabel>
        <skos:definition xml:lang="en">A carrier type consisting of a roll of paper on which musical notes are represented by perforations, designed to mechanically reproduce the music when used in a player piano, player organ, etc.</skos:definition>
        <skos:definition xml:lang="da">Bærertype, der består af en papirrulle, hvorpå musiknoder repræsenteres af huller skabt til at gengive musikken mekanisk, når rullen bruges i et pianola, mekanisk klaver etc.</skos:definition>
        <skos:definition xml:lang="nl">Een rol papier waarop muzieknoten voorgesteld worden door perforaties, ontworpen om mechanisch de muziek weer te geven wanneer deze gebruikt wordt in een pianola e.d.</skos:definition>
        <skos:definition xml:lang="de">Ein Datenträgertyp, der aus einer Papierrolle besteht, auf der Musiknoten in Form von Perforationen repräsentiert werden und die konzipiert ist, um Musik in einem mechanischen Klavier, einer mechanischen Orgel usw. wiederzugeben.</skos:definition>
        <skos:definition xml:lang="no">En bærertype som består av en papirrull der musikknoter representeres av hull, utformet for å gjengi musikken mekanisk ved bruk i pianola og lignende mekaniske instrumenter.</skos:definition>
        <skos:definition xml:lang="vi">Loại hộp chứa gồm có cuốn giấy trên đó nốt nhạc được trình bày bởi các lỗ răng cưa để tái tạo một cách cơ học âm nhạc khi dùng với piano tự động, organ tự động, vv...</skos:definition>
        <skos:definition xml:lang="fi">Paperirulla, jossa olevat rei’itykset edustavat toistettavia säveliä. Suunniteltu toistamaan musiikkia mekaanisesti automaattipianon, automaattiurkujen yms. avulla.</skos:definition>
        <skos:definition xml:lang="es">Rollo de papel en el que las notas musicales están representadas mediante perforaciones, diseñado para reproducir en forma mecánica la música cuando se utiliza en una pianola, órgano mecánico, etc.</skos:definition>
        <skos:definition xml:lang="ca">Tipus de suport físic que consisteix en un rotlle de paper sobre el qual es representen les notes musicals amb perforacions, concebut per reproduir la música mecànicament quan s’usa en una pianola, un orgue mecànic, etc.</skos:definition>
        <skos:definition xml:lang="fr">Type de support matériel qui consiste en un rouleau de papier sur lequel les notes de musique sont représentées par des perforations, destiné à reproduire mécaniquement la musique lorsqu’il est utilisé avec un piano mécanique, un orgue mécanique, etc.</skos:definition>
        <skos:definition xml:lang="zh">通过穿孔方式表示音符的纸卷，用于钢琴、风琴等时，以机械方式重现音乐。</skos:definition>
        <skos:inScheme rdf:resource="http://rdaregistry.info/termList/RDACarrierType"/>
        <skos:narrower rdf:resource="http://performedmusicontology.org/ontology/OrganRoll"/>
        <skos:narrower rdf:resource="http://performedmusicontology.org/ontology/PianoRoll"/>
        <skos:prefLabel xml:lang="de">Notenrolle</skos:prefLabel>
        <skos:prefLabel xml:lang="en">audio roll</skos:prefLabel>
        <skos:prefLabel xml:lang="nl">audiorol</skos:prefLabel>
        <skos:prefLabel xml:lang="vi">cuốn audio</skos:prefLabel>
        <skos:prefLabel xml:lang="sv">ljudrulle</skos:prefLabel>
        <skos:prefLabel xml:lang="da">lydrulle</skos:prefLabel>
        <skos:prefLabel xml:lang="no">pianorull</skos:prefLabel>
        <skos:prefLabel xml:lang="es">rollo sonoro</skos:prefLabel>
        <skos:prefLabel xml:lang="ca">rotlle àudio</skos:prefLabel>
        <skos:prefLabel xml:lang="fr">rouleau audio</skos:prefLabel>
        <skos:prefLabel xml:lang="it">rullo audio</skos:prefLabel>
        <skos:prefLabel xml:lang="fi">äänirulla</skos:prefLabel>
        <skos:prefLabel xml:lang="ar">لفافة سمعية</skos:prefLabel>
        <skos:prefLabel xml:lang="zh">录音卷</skos:prefLabel>
        <skos:scopeNote xml:lang="es">Incluye rollos de pianola, etc.</skos:scopeNote>
        <skos:scopeNote xml:lang="zh">用于钢琴滚筒等。</skos:scopeNote>
    </owl:NamedIndividual>
    


    <!-- http://rdaregistry.info/termList/RDACarrierType/1007 -->

    <owl:NamedIndividual rdf:about="http://rdaregistry.info/termList/RDACarrierType/1007">
        <rdf:type rdf:resource="http://www.w3.org/2004/02/skos/core#Concept"/>
        <rdakit:toolkitDefinition xml:lang="en">A carrier type consisting of a cassette containing an audiotape.</rdakit:toolkitDefinition>
        <rdakit:toolkitDefinition xml:lang="da">Bærertype, der består af en kassette, der indeholder et lydbånd.</rdakit:toolkitDefinition>
        <rdakit:toolkitDefinition xml:lang="es">Casete que contiene una cinta de audio.</rdakit:toolkitDefinition>
        <rdakit:toolkitDefinition xml:lang="nl">Een cassette die een audiotape bevat.</rdakit:toolkitDefinition>
        <rdakit:toolkitDefinition xml:lang="de">Ein Datenträgertyp, der aus einer Kassette besteht, die ein Tonband enthält.</rdakit:toolkitDefinition>
        <rdakit:toolkitDefinition xml:lang="no">En bærertype som består av en kassett som inneholder et lydbånd.</rdakit:toolkitDefinition>
        <rdakit:toolkitDefinition xml:lang="fi">Kasetti, joka sisältää ääninauhan.</rdakit:toolkitDefinition>
        <rdakit:toolkitDefinition xml:lang="vi">Loại hộp chứa gồm có cassette chứa một băng audio.</rdakit:toolkitDefinition>
        <rdakit:toolkitDefinition xml:lang="ca">Tipus de suport físic que consisteix en una casset que conté una cinta àudio.</rdakit:toolkitDefinition>
        <rdakit:toolkitDefinition xml:lang="fr">Type de support matériel qui consiste en une cassette contenant une bande audio.</rdakit:toolkitDefinition>
        <rdakit:toolkitDefinition xml:lang="zh">装在双轴盒中的录音带。</rdakit:toolkitDefinition>
        <rdakit:toolkitLabel xml:lang="de">Audiokassette</rdakit:toolkitLabel>
        <rdakit:toolkitLabel xml:lang="es">audiocasete</rdakit:toolkitLabel>
        <rdakit:toolkitLabel xml:lang="it">audiocassetta</rdakit:toolkitLabel>
        <rdakit:toolkitLabel xml:lang="en">audiocassette</rdakit:toolkitLabel>
        <rdakit:toolkitLabel xml:lang="nl">audiocassette</rdakit:toolkitLabel>
        <rdakit:toolkitLabel xml:lang="vi">audiocassette</rdakit:toolkitLabel>
        <rdakit:toolkitLabel xml:lang="ca">casset àudio</rdakit:toolkitLabel>
        <rdakit:toolkitLabel xml:lang="fr">cassette audio</rdakit:toolkitLabel>
        <rdakit:toolkitLabel xml:lang="da">kassettebånd</rdakit:toolkitLabel>
        <rdakit:toolkitLabel xml:lang="sv">ljudkassett</rdakit:toolkitLabel>
        <rdakit:toolkitLabel xml:lang="no">lydkassett</rdakit:toolkitLabel>
        <rdakit:toolkitLabel xml:lang="fi">äänikasetti</rdakit:toolkitLabel>
        <rdakit:toolkitLabel xml:lang="zh">卡式录音带</rdakit:toolkitLabel>
        <regap:identifier rdf:resource="http://metadataregistry.org/concepts/539"/>
        <rdfs:label>audiocassette</rdfs:label>
        <skos:definition xml:lang="en">A carrier type consisting of a cassette containing an audiotape.</skos:definition>
        <skos:definition xml:lang="da">Bærertype, der består af en kassette, der indeholder et lydbånd.</skos:definition>
        <skos:definition xml:lang="es">Casete que contiene una cinta de audio.</skos:definition>
        <skos:definition xml:lang="nl">Een cassette die een audiotape bevat.</skos:definition>
        <skos:definition xml:lang="de">Ein Datenträgertyp, der aus einer Kassette besteht, die ein Tonband enthält.</skos:definition>
        <skos:definition xml:lang="no">En bærertype som består av en kassett som inneholder et lydbånd.</skos:definition>
        <skos:definition xml:lang="fi">Kasetti, joka sisältää ääninauhan.</skos:definition>
        <skos:definition xml:lang="vi">Loại hộp chứa gồm có cassette chứa một băng audio.</skos:definition>
        <skos:definition xml:lang="ca">Tipus de suport físic que consisteix en una casset que conté una cinta àudio.</skos:definition>
        <skos:definition xml:lang="fr">Type de support matériel qui consiste en une cassette contenant une bande audio.</skos:definition>
        <skos:definition xml:lang="zh">装在双轴盒中的录音带。</skos:definition>
        <skos:inScheme rdf:resource="http://rdaregistry.info/termList/RDACarrierType"/>
        <skos:narrower rdf:resource="http://performedmusicontology.org/ontology/DAT"/>
        <skos:prefLabel xml:lang="de">Audiokassette</skos:prefLabel>
        <skos:prefLabel xml:lang="es">audiocasete</skos:prefLabel>
        <skos:prefLabel xml:lang="it">audiocassetta</skos:prefLabel>
        <skos:prefLabel xml:lang="en">audiocassette</skos:prefLabel>
        <skos:prefLabel xml:lang="nl">audiocassette</skos:prefLabel>
        <skos:prefLabel xml:lang="vi">audiocassette</skos:prefLabel>
        <skos:prefLabel xml:lang="ca">casset àudio</skos:prefLabel>
        <skos:prefLabel xml:lang="fr">cassette audio</skos:prefLabel>
        <skos:prefLabel xml:lang="da">kassettebånd</skos:prefLabel>
        <skos:prefLabel xml:lang="sv">ljudkassett</skos:prefLabel>
        <skos:prefLabel xml:lang="no">lydkassett</skos:prefLabel>
        <skos:prefLabel xml:lang="fi">äänikasetti</skos:prefLabel>
        <skos:prefLabel xml:lang="ar">كاسيت صوتي</skos:prefLabel>
        <skos:prefLabel xml:lang="zh">卡式录音带</skos:prefLabel>
    </owl:NamedIndividual>
    


    <!-- http://rdaregistry.info/termList/RDACarrierType/1060 -->

    <owl:NamedIndividual rdf:about="http://rdaregistry.info/termList/RDACarrierType/1060">
        <rdf:type rdf:resource="http://www.w3.org/2004/02/skos/core#Concept"/>
        <rdakit:toolkitDefinition xml:lang="en">A carrier type consisting of a disc on which video signals, with or without sound, are recorded.</rdakit:toolkitDefinition>
        <rdakit:toolkitDefinition xml:lang="da">Bærertype, der består af en disc, hvorpå der er optaget videosignaler med eller uden lyd.</rdakit:toolkitDefinition>
        <rdakit:toolkitDefinition xml:lang="es">Disco sobre el que se han grabado señales de video, con o sin sonido.</rdakit:toolkitDefinition>
        <rdakit:toolkitDefinition xml:lang="nl">Een disc waarop videosignalen, met of zonder geluid, worden opgenomen.</rdakit:toolkitDefinition>
        <rdakit:toolkitDefinition xml:lang="de">Ein Datenträgertyp, der aus eine Disk besteht, auf der Video-Signale mit oder ohne Ton aufgezeichnet sind.</rdakit:toolkitDefinition>
        <rdakit:toolkitDefinition xml:lang="no">En bærertype som består av en plate der videosignaler med eller uten lyd registreres.</rdakit:toolkitDefinition>
        <rdakit:toolkitDefinition xml:lang="fi">Levy, jolle tallennetaan videosignaaleja, sisältäen ääntä tai ilman ääntä.</rdakit:toolkitDefinition>
        <rdakit:toolkitDefinition xml:lang="vi">Loại hộp chứa gồm có đĩa trên đó tín hiệu video, có hoặc không có âm thanh, được ghi lại.</rdakit:toolkitDefinition>
        <rdakit:toolkitDefinition xml:lang="ca">Tipus de suport físic que consisteix en un disc en el qual hi ha enregistrats senyals de vídeo, amb o sense so.</rdakit:toolkitDefinition>
        <rdakit:toolkitDefinition xml:lang="fr">Type de support matériel qui consiste en un disque sur lequel des signaux vidéo, accompagnés ou non de son, sont enregistrés.</rdakit:toolkitDefinition>
        <rdakit:toolkitDefinition xml:lang="zh">记录视频信号的盘片，有无声音均可。</rdakit:toolkitDefinition>
        <rdakit:toolkitLabel xml:lang="de">Videodisk</rdakit:toolkitLabel>
        <rdakit:toolkitLabel xml:lang="ca">videodisc</rdakit:toolkitLabel>
        <rdakit:toolkitLabel xml:lang="da">videodisc</rdakit:toolkitLabel>
        <rdakit:toolkitLabel xml:lang="en">videodisc</rdakit:toolkitLabel>
        <rdakit:toolkitLabel xml:lang="nl">videodisc</rdakit:toolkitLabel>
        <rdakit:toolkitLabel xml:lang="es">videodisco</rdakit:toolkitLabel>
        <rdakit:toolkitLabel xml:lang="it">videodisco</rdakit:toolkitLabel>
        <rdakit:toolkitLabel xml:lang="no">videodisk</rdakit:toolkitLabel>
        <rdakit:toolkitLabel xml:lang="fi">videolevy</rdakit:toolkitLabel>
        <rdakit:toolkitLabel xml:lang="sv">videoskiva</rdakit:toolkitLabel>
        <rdakit:toolkitLabel xml:lang="fr">vidéodisque</rdakit:toolkitLabel>
        <rdakit:toolkitLabel xml:lang="vi">đĩa video</rdakit:toolkitLabel>
        <rdakit:toolkitLabel xml:lang="zh">视盘</rdakit:toolkitLabel>
        <regap:identifier rdf:resource="http://metadataregistry.org/concepts/1113"/>
        <rdfs:label>videodisc</rdfs:label>
        <skos:definition xml:lang="en">A carrier type consisting of a disc on which video signals, with or without sound, are recorded.</skos:definition>
        <skos:definition xml:lang="da">Bærertype, der består af en disc, hvorpå der er optaget videosignaler med eller uden lyd.</skos:definition>
        <skos:definition xml:lang="es">Disco sobre el que se han grabado señales de video, con o sin sonido.</skos:definition>
        <skos:definition xml:lang="nl">Een disc waarop videosignalen, met of zonder geluid, worden opgenomen.</skos:definition>
        <skos:definition xml:lang="de">Ein Datenträgertyp, der aus eine Disk besteht, auf der Video-Signale mit oder ohne Ton aufgezeichnet sind.</skos:definition>
        <skos:definition xml:lang="no">En bærertype som består av en plate der videosignaler med eller uten lyd registreres.</skos:definition>
        <skos:definition xml:lang="fi">Levy, jolle tallennetaan videosignaaleja, sisältäen ääntä tai ilman ääntä.</skos:definition>
        <skos:definition xml:lang="vi">Loại hộp chứa gồm có đĩa trên đó tín hiệu video, có hoặc không có âm thanh, được ghi lại.</skos:definition>
        <skos:definition xml:lang="ca">Tipus de suport físic que consisteix en un disc en el qual hi ha enregistrats senyals de vídeo, amb o sense so.</skos:definition>
        <skos:definition xml:lang="fr">Type de support matériel qui consiste en un disque sur lequel des signaux vidéo, accompagnés ou non de son, sont enregistrés.</skos:definition>
        <skos:definition xml:lang="zh">记录视频信号的盘片，有无声音均可。</skos:definition>
        <skos:inScheme rdf:resource="http://rdaregistry.info/termList/RDACarrierType"/>
        <skos:narrower rdf:resource="http://performedmusicontology.org/Laserdisc"/>
        <skos:narrower rdf:resource="http://performedmusicontology.org/ontology/DvdVideo"/>
        <skos:prefLabel xml:lang="de">Videodisk</skos:prefLabel>
        <skos:prefLabel xml:lang="ca">videodisc</skos:prefLabel>
        <skos:prefLabel xml:lang="da">videodisc</skos:prefLabel>
        <skos:prefLabel xml:lang="en">videodisc</skos:prefLabel>
        <skos:prefLabel xml:lang="nl">videodisc</skos:prefLabel>
        <skos:prefLabel xml:lang="es">videodisco</skos:prefLabel>
        <skos:prefLabel xml:lang="it">videodisco</skos:prefLabel>
        <skos:prefLabel xml:lang="no">videodisk</skos:prefLabel>
        <skos:prefLabel xml:lang="fi">videolevy</skos:prefLabel>
        <skos:prefLabel xml:lang="sv">videoskiva</skos:prefLabel>
        <skos:prefLabel xml:lang="fr">vidéodisque</skos:prefLabel>
        <skos:prefLabel xml:lang="vi">đĩa video</skos:prefLabel>
        <skos:prefLabel xml:lang="ar">قرص فيديو</skos:prefLabel>
        <skos:prefLabel xml:lang="zh">视盘</skos:prefLabel>
    </owl:NamedIndividual>
</rdf:RDF>



<!-- Generated by the OWL API (version 4.2.8.20170104-2310) https://github.com/owlcs/owlapi -->

